<?xml version="1.0" encoding="UTF-8"?>
<rdf:RDF
   xmlns:nen2660="https://w3id.org/nen2660/def#"
   xmlns:owl="http://www.w3.org/2002/07/owl#"
   xmlns:rdf="http://www.w3.org/1999/02/22-rdf-syntax-ns#"
   xmlns:rdfs="http://www.w3.org/2000/01/rdf-schema#"
   xmlns:sh="http://www.w3.org/ns/shacl#"
   xmlns:skos="http://www.w3.org/2004/02/skos/core#"
>
  <rdf:Description rdf:about="https://w3id.org/nen2660/def#overConnection">
    <rdf:type rdf:resource="http://www.w3.org/1999/02/22-rdf-syntax-ns#Property"/>
    <rdf:type rdf:resource="http://www.w3.org/2002/07/owl#ObjectProperty"/>
    <rdfs:domain rdf:resource="https://w3id.org/nen2660/def#Interaction"/>
    <rdfs:range rdf:resource="https://w3id.org/nen2660/def#Connection"/>
    <rdfs:seeAlso rdf:resource="https://w3id.org/nen2660/term#overConnection"/>
    <skos:definition xml:lang="en">The connection over which an interaction between physical objects takes place</skos:definition>
    <skos:prefLabel xml:lang="en">over connection</skos:prefLabel>
  </rdf:Description>
  <rdf:Description rdf:about="https://w3id.org/nen2660/shacl/def">
    <rdf:type rdf:resource="http://www.w3.org/2002/07/owl#Ontology"/>
    <owl:imports rdf:resource="http://qudt.org/2.1/schema/qudt"/>
    <owl:imports rdf:resource="http://qudt.org/2.1/vocab/quantitykind"/>
    <owl:imports rdf:resource="http://qudt.org/2.1/vocab/unit"/>
    <owl:imports rdf:resource="http://www.w3.org/2004/02/skos/core"/>
    <owl:imports rdf:resource="http://www.w3.org/2006/time"/>
    <owl:imports rdf:resource="http://www.w3.org/ns/shacl"/>
    <owl:imports rdf:resource="https://w3id.org/nen2660/rdfs/def"/>
  </rdf:Description>
  <rdf:Description rdf:about="https://w3id.org/nen2660/term#hasUnit">
    <rdf:type rdf:resource="http://www.w3.org/2004/02/skos/core#Concept"/>
    <skos:definition xml:lang="nl">Het hebben van een eenheid</skos:definition>
    <skos:definition xml:lang="en">The possession of a unit</skos:definition>
    <skos:prefLabel xml:lang="en">has unit</skos:prefLabel>
    <skos:prefLabel xml:lang="nl">heeft eenheid</skos:prefLabel>
  </rdf:Description>
  <rdf:Description rdf:about="https://w3id.org/nen2660/term#HeterogeneousMixture">
    <rdf:type rdf:resource="http://www.w3.org/2004/02/skos/core#Concept"/>
    <skos:broader rdf:resource="https://w3id.org/nen2660/term#Mixture"/>
    <skos:definition xml:lang="en">A mixture that is separated into different regions or phases that have different compositions or properties</skos:definition>
    <skos:definition xml:lang="nl">Een mengsel dat is opgedeeld in verschillende regio's of fasen met verschillende samenstellingen of eigenschappen</skos:definition>
    <skos:prefLabel xml:lang="nl">Heterogeneen mengsel</skos:prefLabel>
    <skos:prefLabel xml:lang="en">Heterogeneous mixture</skos:prefLabel>
  </rdf:Description>
  <rdf:Description rdf:about="https://w3id.org/nen2660/term#ChemicalElement">
    <rdf:type rdf:resource="http://www.w3.org/2004/02/skos/core#Concept"/>
    <skos:broader rdf:resource="https://w3id.org/nen2660/term#PureSubstance"/>
    <skos:definition xml:lang="en">Pure substance that is made up of atoms with the same atomic number. A chemical element cannot be decomposed through chemical reactions</skos:definition>
    <skos:definition xml:lang="nl">Zuivere stof die is opgebouwd uit atomen met hetzelfde atoomnummer. Een chemisch element kan niet worden ontleed door middel van chemische reacties</skos:definition>
    <skos:prefLabel xml:lang="en">Chemical element</skos:prefLabel>
    <skos:prefLabel xml:lang="nl">Chemisch element</skos:prefLabel>
  </rdf:Description>
  <rdf:Description rdf:about="https://w3id.org/nen2660/def#aggregationStateType">
    <rdf:type rdf:resource="http://www.w3.org/1999/02/22-rdf-syntax-ns#Property"/>
    <rdf:type rdf:resource="http://www.w3.org/2002/07/owl#ObjectProperty"/>
    <rdfs:domain rdf:resource="https://w3id.org/nen2660/def#Matter"/>
    <rdfs:range rdf:resource="https://w3id.org/nen2660/def#AggregationStateType"/>
    <rdfs:seeAlso rdf:resource="https://w3id.org/nen2660/term#aggregationStateType"/>
    <skos:definition xml:lang="en">The possession of an aggregation state type</skos:definition>
    <skos:prefLabel xml:lang="en">aggregation state type</skos:prefLabel>
  </rdf:Description>
  <rdf:Description rdf:about="https://w3id.org/nen2660/def#InformationObject">
    <rdf:type rdf:resource="http://www.w3.org/2000/01/rdf-schema#Class"/>
    <rdf:type rdf:resource="http://www.w3.org/2002/07/owl#Class"/>
    <rdfs:seeAlso rdf:resource="https://w3id.org/nen2660/term#InformationObject"/>
    <rdfs:subClassOf rdf:resource="https://w3id.org/nen2660/def#Object"/>
    <skos:definition xml:lang="en">Object which describes a thing in reality</skos:definition>
    <skos:prefLabel xml:lang="en">Information object</skos:prefLabel>
  </rdf:Description>
  <rdf:Description rdf:about="https://w3id.org/nen2660/def#executes">
    <rdf:type rdf:resource="http://www.w3.org/1999/02/22-rdf-syntax-ns#Property"/>
    <rdf:type rdf:resource="http://www.w3.org/2002/07/owl#ObjectProperty"/>
    <rdfs:domain rdf:resource="https://w3id.org/nen2660/def#PhysicalObject"/>
    <rdfs:range rdf:resource="https://w3id.org/nen2660/def#Activity"/>
    <rdfs:seeAlso rdf:resource="https://w3id.org/nen2660/term#executes"/>
    <skos:definition xml:lang="en">The activity executed by a physical object</skos:definition>
    <skos:prefLabel xml:lang="en">executes</skos:prefLabel>
  </rdf:Description>
  <rdf:Description rdf:about="https://w3id.org/nen2660/term#Port">
    <rdf:type rdf:resource="http://www.w3.org/2004/02/skos/core#Concept"/>
    <skos:broader rdf:resource="https://w3id.org/nen2660/term#PhysicalObject"/>
    <skos:definition xml:lang="en">A physical or logical point of interaction as part of a physical object where, through a connection or interface, an interaction can take place</skos:definition>
    <skos:definition xml:lang="nl">Een fysiek of logisch interactiepunt als deel van een fysiek object waar, via een verbinding of raakvlak, een interactie kan plaatsvinden</skos:definition>
    <skos:prefLabel xml:lang="nl">Poort</skos:prefLabel>
    <skos:prefLabel xml:lang="en">Port</skos:prefLabel>
  </rdf:Description>
  <rdf:Description rdf:nodeID="n87801b7bffed4f059b3dda9335adfc9ab68">
    <sh:path rdf:resource="https://w3id.org/nen2660/def#requirementSourceType"/>
    <sh:class rdf:resource="https://w3id.org/nen2660/def#RequirementSourceType"/>
  </rdf:Description>
  <rdf:Description rdf:about="https://w3id.org/nen2660/term#aggregationStateType">
    <rdf:type rdf:resource="http://www.w3.org/2004/02/skos/core#Concept"/>
    <skos:definition xml:lang="nl">Het hebben van een aggregatietoestandtype</skos:definition>
    <skos:definition xml:lang="en">The possession of an aggregation state type</skos:definition>
    <skos:prefLabel xml:lang="nl">aggregatietoestandtype</skos:prefLabel>
    <skos:prefLabel xml:lang="en">aggregation state type</skos:prefLabel>
  </rdf:Description>
  <rdf:Description rdf:about="https://w3id.org/nen2660/term#abbreviation">
    <rdf:type rdf:resource="http://www.w3.org/2004/02/skos/core#Concept"/>
    <skos:broader rdf:resource="http://www.w3.org/2004/02/skos/core#altLabel"/>
    <skos:definition xml:lang="nl">Acroniem of eerste woord als speciaal geval van een naam</skos:definition>
    <skos:definition xml:lang="en">Acronym or initial word as special case of a name</skos:definition>
    <skos:prefLabel xml:lang="en">abbreviation</skos:prefLabel>
    <skos:prefLabel xml:lang="nl">afkorting</skos:prefLabel>
  </rdf:Description>
  <rdf:Description rdf:about="https://w3id.org/nen2660/term#TemporalEntity">
    <rdf:type rdf:resource="http://www.w3.org/2004/02/skos/core#Concept"/>
    <skos:broader rdf:resource="https://w3id.org/nen2660/term#Representation"/>
    <skos:definition xml:lang="en">A temporal interval or instant</skos:definition>
    <skos:definition xml:lang="nl">Een tijdsinterval of -moment</skos:definition>
    <skos:prefLabel xml:lang="en">Temporal entity</skos:prefLabel>
    <skos:prefLabel xml:lang="nl">Temporele entiteit</skos:prefLabel>
  </rdf:Description>
  <rdf:Description rdf:about="https://w3id.org/nen2660/def#AllDisjointClassesShape">
    <rdf:type rdf:resource="http://www.w3.org/ns/shacl#NodeShape"/>
    <sh:targetSubjectsOf rdf:resource="http://www.w3.org/1999/02/22-rdf-syntax-ns#type"/>
    <sh:property rdf:nodeID="n87801b7bffed4f059b3dda9335adfc9ab90"/>
    <sh:property rdf:nodeID="n87801b7bffed4f059b3dda9335adfc9ab100"/>
    <sh:property rdf:nodeID="n87801b7bffed4f059b3dda9335adfc9ab107"/>
    <sh:property rdf:nodeID="n87801b7bffed4f059b3dda9335adfc9ab114"/>
  </rdf:Description>
  <rdf:Description rdf:about="https://w3id.org/nen2660/def#Activity">
    <rdf:type rdf:resource="http://www.w3.org/2000/01/rdf-schema#Class"/>
    <rdf:type rdf:resource="http://www.w3.org/ns/shacl#NodeShape"/>
    <rdf:type rdf:resource="http://www.w3.org/2002/07/owl#Class"/>
    <rdfs:seeAlso rdf:resource="https://w3id.org/nen2660/term#Activity"/>
    <rdfs:subClassOf rdf:resource="https://w3id.org/nen2660/def#Entity"/>
    <rdfs:subClassOf rdf:nodeID="n29315767620c4c949118ed89a344f3a5b1"/>
    <skos:definition xml:lang="en">Entity that takes place or can take place in a concrete space-time. An activity transforms objects, and is executed by an object</skos:definition>
    <skos:prefLabel xml:lang="en">Activity</skos:prefLabel>
    <sh:property rdf:nodeID="n87801b7bffed4f059b3dda9335adfc9ab1"/>
    <sh:property rdf:nodeID="n87801b7bffed4f059b3dda9335adfc9ab2"/>
    <sh:property rdf:nodeID="n87801b7bffed4f059b3dda9335adfc9ab3"/>
    <sh:property rdf:nodeID="n87801b7bffed4f059b3dda9335adfc9ab4"/>
    <sh:property rdf:nodeID="n87801b7bffed4f059b3dda9335adfc9ab5"/>
  </rdf:Description>
  <rdf:Description rdf:about="https://w3id.org/nen2660/def#MatterPortion">
    <rdf:type rdf:resource="http://www.w3.org/2000/01/rdf-schema#Class"/>
    <rdf:type rdf:resource="http://www.w3.org/ns/shacl#NodeShape"/>
    <rdf:type rdf:resource="http://www.w3.org/2002/07/owl#Class"/>
    <rdfs:seeAlso rdf:resource="https://w3id.org/nen2660/term#MatterPortion"/>
    <rdfs:subClassOf rdf:resource="https://w3id.org/nen2660/def#RelationReference"/>
    <rdfs:subClassOf rdf:nodeID="n29315767620c4c949118ed89a344f3a5b19"/>
    <rdfs:subClassOf rdf:nodeID="n29315767620c4c949118ed89a344f3a5b20"/>
    <skos:definition xml:lang="en">An objectified relation reference for the consists of relation</skos:definition>
    <skos:prefLabel xml:lang="en">Matter portion</skos:prefLabel>
    <sh:property rdf:nodeID="n87801b7bffed4f059b3dda9335adfc9ab32"/>
  </rdf:Description>
  <rdf:Description rdf:about="https://w3id.org/nen2660/def#connectsPort">
    <rdf:type rdf:resource="http://www.w3.org/1999/02/22-rdf-syntax-ns#Property"/>
    <rdf:type rdf:resource="http://www.w3.org/2002/07/owl#ObjectProperty"/>
    <rdfs:range rdf:resource="https://w3id.org/nen2660/def#Port"/>
    <rdfs:seeAlso rdf:resource="https://w3id.org/nen2660/term#connectsPort"/>
    <skos:definition xml:lang="en">The ports (as part of physical objects) connected by a connection or interface</skos:definition>
    <skos:prefLabel xml:lang="en">connects port</skos:prefLabel>
    <rdfs:domain rdf:nodeID="n29315767620c4c949118ed89a344f3a5b55"/>
  </rdf:Description>
  <rdf:Description rdf:about="https://w3id.org/nen2660/def#Connection">
    <rdf:type rdf:resource="http://www.w3.org/2000/01/rdf-schema#Class"/>
    <rdf:type rdf:resource="http://www.w3.org/ns/shacl#NodeShape"/>
    <rdf:type rdf:resource="http://www.w3.org/2002/07/owl#Class"/>
    <rdfs:seeAlso rdf:resource="https://w3id.org/nen2660/term#Connection"/>
    <rdfs:subClassOf rdf:resource="https://w3id.org/nen2660/def#PhysicalObject"/>
    <skos:definition xml:lang="en">A physical object (real object or spatial area) that connects two other physical objects and over which interaction takes place, namely the transfer of matter, energy, information or forces</skos:definition>
    <skos:prefLabel xml:lang="en">Connection</skos:prefLabel>
    <sh:property rdf:nodeID="n87801b7bffed4f059b3dda9335adfc9ab15"/>
    <sh:property rdf:nodeID="n87801b7bffed4f059b3dda9335adfc9ab16"/>
  </rdf:Description>
  <rdf:Description rdf:nodeID="n87801b7bffed4f059b3dda9335adfc9ab54">
    <sh:path rdf:resource="https://w3id.org/nen2660/def#consistsOf"/>
    <sh:or rdf:nodeID="n87801b7bffed4f059b3dda9335adfc9ab57"/>
  </rdf:Description>
  <rdf:Description rdf:about="https://w3id.org/nen2660/def#QuantityValue">
    <rdf:type rdf:resource="http://www.w3.org/2000/01/rdf-schema#Class"/>
    <rdf:type rdf:resource="http://www.w3.org/ns/shacl#NodeShape"/>
    <rdf:type rdf:resource="http://www.w3.org/2002/07/owl#Class"/>
    <rdfs:seeAlso rdf:resource="https://w3id.org/nen2660/term#QuantityValue"/>
    <rdfs:subClassOf rdf:resource="https://w3id.org/nen2660/def#Objectification"/>
    <rdfs:subClassOf rdf:nodeID="n29315767620c4c949118ed89a344f3a5b29"/>
    <skos:definition xml:lang="en">The objectification of a value of a quantity (typically involving a quantity kind and a unit) having a complex value like a simple value sec combined with other metadata or just a combination of simple values</skos:definition>
    <skos:prefLabel xml:lang="en">Quantity value</skos:prefLabel>
    <sh:property rdf:nodeID="n87801b7bffed4f059b3dda9335adfc9ab47"/>
  </rdf:Description>
  <rdf:Description rdf:about="https://w3id.org/nen2660/def#PhysicalObject">
    <rdf:type rdf:resource="http://www.w3.org/2000/01/rdf-schema#Class"/>
    <rdf:type rdf:resource="http://www.w3.org/ns/shacl#NodeShape"/>
    <rdf:type rdf:resource="http://www.w3.org/2002/07/owl#Class"/>
    <rdfs:seeAlso rdf:resource="https://w3id.org/nen2660/term#PhysicalObject"/>
    <rdfs:subClassOf rdf:resource="https://w3id.org/nen2660/def#Object"/>
    <skos:definition xml:lang="en">Object that exists or may exist within physical 4D space-time. A physical object forms a manifestation and a demarcation of matter and/or energy, and is (in)directly perceptible by the senses</skos:definition>
    <skos:prefLabel xml:lang="en">Physical object</skos:prefLabel>
    <sh:property rdf:nodeID="n87801b7bffed4f059b3dda9335adfc9ab40"/>
    <sh:property rdf:nodeID="n87801b7bffed4f059b3dda9335adfc9ab41"/>
    <sh:property rdf:nodeID="n87801b7bffed4f059b3dda9335adfc9ab42"/>
    <sh:property rdf:nodeID="n87801b7bffed4f059b3dda9335adfc9ab43"/>
  </rdf:Description>
  <rdf:Description rdf:about="https://w3id.org/nen2660/def#contains">
    <rdf:type rdf:resource="http://www.w3.org/1999/02/22-rdf-syntax-ns#Property"/>
    <rdf:type rdf:resource="http://www.w3.org/2002/07/owl#ObjectProperty"/>
    <rdfs:domain rdf:resource="https://w3id.org/nen2660/def#SpatialRegion"/>
    <rdfs:range rdf:resource="https://w3id.org/nen2660/def#RealObject"/>
    <rdfs:seeAlso rdf:resource="https://w3id.org/nen2660/term#contains"/>
    <skos:definition xml:lang="en">The real objects located in a spatial region, typically the gaseous amount of bulk matter present in that region</skos:definition>
    <skos:prefLabel xml:lang="en">contains</skos:prefLabel>
  </rdf:Description>
  <rdf:Description rdf:about="https://w3id.org/nen2660/def#isPlanFor">
    <rdf:type rdf:resource="http://www.w3.org/1999/02/22-rdf-syntax-ns#Property"/>
    <rdf:type rdf:resource="http://www.w3.org/2002/07/owl#ObjectProperty"/>
    <rdfs:domain rdf:resource="https://w3id.org/nen2660/def#PlannedEntity"/>
    <rdfs:range rdf:resource="https://w3id.org/nen2660/def#RealizedEntity"/>
    <rdfs:seeAlso rdf:resource="https://w3id.org/nen2660/term#isPlanFor"/>
    <skos:definition xml:lang="en">A potentially realized entity according to this planned entity</skos:definition>
    <skos:prefLabel xml:lang="en">is plan for</skos:prefLabel>
  </rdf:Description>
  <rdf:Description rdf:about="https://w3id.org/nen2660/term#PhysicalObject">
    <rdf:type rdf:resource="http://www.w3.org/2004/02/skos/core#Concept"/>
    <skos:broader rdf:resource="https://w3id.org/nen2660/term#Object"/>
    <skos:definition xml:lang="nl">Object dat bestaat of kan bestaan binnen de fysieke 4D ruimte-tijd. Een fysiek object vormt een manifestatie en een afbakening van materie en/of energie, en is (in)direct waarneembaar door de zintuigen</skos:definition>
    <skos:definition xml:lang="en">Object that exists or may exist within physical 4D space-time. A physical object forms a manifestation and a demarcation of matter and/or energy, and is (in)directly perceptible by the senses</skos:definition>
    <skos:prefLabel xml:lang="nl">Fysiek object</skos:prefLabel>
    <skos:prefLabel xml:lang="en">Physical object</skos:prefLabel>
  </rdf:Description>
  <rdf:Description rdf:nodeID="n87801b7bffed4f059b3dda9335adfc9ab29">
    <sh:path rdf:resource="https://w3id.org/nen2660/def#connectsPort"/>
    <sh:class rdf:resource="https://w3id.org/nen2660/def#Port"/>
  </rdf:Description>
  <rdf:Description rdf:nodeID="n29315767620c4c949118ed89a344f3a5b50">
    <rdf:first rdf:resource="https://w3id.org/nen2660/def#InformationFlow"/>
    <rdf:rest rdf:nodeID="n29315767620c4c949118ed89a344f3a5b51"/>
  </rdf:Description>
  <rdf:Description rdf:nodeID="n87801b7bffed4f059b3dda9335adfc9ab102">
    <rdf:first rdf:resource="http://www.w3.org/1999/02/22-rdf-syntax-ns#type"/>
    <rdf:rest rdf:nodeID="n87801b7bffed4f059b3dda9335adfc9ab103"/>
  </rdf:Description>
  <rdf:Description rdf:nodeID="n87801b7bffed4f059b3dda9335adfc9ab21">
    <sh:path rdf:resource="https://w3id.org/nen2660/def#hasPart"/>
    <sh:class rdf:resource="https://w3id.org/nen2660/def#Event"/>
  </rdf:Description>
  <rdf:Description rdf:about="https://w3id.org/nen2660/term#Mixture">
    <rdf:type rdf:resource="http://www.w3.org/2004/02/skos/core#Concept"/>
    <skos:broader rdf:resource="https://w3id.org/nen2660/term#Matter"/>
    <skos:definition xml:lang="nl">De combinatie van twee of meer verschillende zuivere stoffen zonder dat daarbij de moleculen hun identiteit verliezen</skos:definition>
    <skos:definition xml:lang="en">The combination of two or more different pure substances without the molecules losing their identity</skos:definition>
    <skos:prefLabel xml:lang="nl">Mengsel</skos:prefLabel>
    <skos:prefLabel xml:lang="en">Mixture</skos:prefLabel>
  </rdf:Description>
  <rdf:Description rdf:about="https://w3id.org/nen2660/def#Solid">
    <rdf:type rdf:resource="https://w3id.org/nen2660/def#AggregationStateType"/>
    <rdfs:seeAlso rdf:resource="https://w3id.org/nen2660/term#Solid"/>
    <skos:definition xml:lang="en">Matter that can be picked up or held, having a texture, and usually firm. Unlike a liquid, gas or plasma</skos:definition>
    <skos:prefLabel xml:lang="en">Solid</skos:prefLabel>
  </rdf:Description>
  <rdf:Description rdf:nodeID="n29315767620c4c949118ed89a344f3a5b51">
    <rdf:first rdf:resource="https://w3id.org/nen2660/def#Force"/>
    <rdf:rest rdf:resource="http://www.w3.org/1999/02/22-rdf-syntax-ns#nil"/>
  </rdf:Description>
  <rdf:Description rdf:about="https://w3id.org/nen2660/term#TechnicalEntity">
    <rdf:type rdf:resource="http://www.w3.org/2004/02/skos/core#Concept"/>
    <skos:broader rdf:resource="https://w3id.org/nen2660/term#Entity"/>
    <skos:definition xml:lang="en">An entity concerned with technical properties and relations that implements or plays functional entities</skos:definition>
    <skos:definition xml:lang="nl">Een entiteit waarbij het gaat om technische eigenschappen en relaties die functionele entiteiten implementeert of speelt</skos:definition>
    <skos:prefLabel xml:lang="en">Technical entity</skos:prefLabel>
    <skos:prefLabel xml:lang="nl">Technische entiteit</skos:prefLabel>
  </rdf:Description>
  <rdf:Description rdf:about="https://w3id.org/nen2660/term#Object">
    <rdf:type rdf:resource="http://www.w3.org/2004/02/skos/core#Concept"/>
    <skos:broader rdf:resource="https://w3id.org/nen2660/term#Entity"/>
    <skos:definition xml:lang="nl">Entiteit die bestaat of kan bestaan binnen een concrete ruimte-tijd. Een object voert een activiteit uit, en wordt getransformeerd door een activiteit</skos:definition>
    <skos:definition xml:lang="en">Entity that exists or can exist within a concrete space-time. An object executes an activity, and is transformed by an activity</skos:definition>
    <skos:prefLabel xml:lang="en">Object</skos:prefLabel>
    <skos:prefLabel xml:lang="nl">Object</skos:prefLabel>
  </rdf:Description>
  <rdf:Description rdf:about="https://w3id.org/nen2660/def#hasUnit">
    <rdf:type rdf:resource="http://www.w3.org/1999/02/22-rdf-syntax-ns#Property"/>
    <rdf:type rdf:resource="http://www.w3.org/2002/07/owl#ObjectProperty"/>
    <rdfs:range rdf:resource="http://qudt.org/schema/qudt/Unit"/>
    <rdfs:seeAlso rdf:resource="https://w3id.org/nen2660/term#hasUnit"/>
    <skos:definition xml:lang="en">The possession of a unit</skos:definition>
    <skos:prefLabel xml:lang="en">has unit</skos:prefLabel>
  </rdf:Description>
  <rdf:Description rdf:about="https://w3id.org/nen2660/term#overInterface">
    <rdf:type rdf:resource="http://www.w3.org/2004/02/skos/core#Concept"/>
    <skos:definition xml:lang="nl">Het raakvlak waarover een interactie tussen fysieke objecten plaatsvindt</skos:definition>
    <skos:definition xml:lang="en">The interface over which an interaction between physical objects takes place</skos:definition>
    <skos:prefLabel xml:lang="en">over interface</skos:prefLabel>
    <skos:prefLabel xml:lang="nl">over raakvlak</skos:prefLabel>
  </rdf:Description>
  <rdf:Description rdf:about="https://w3id.org/nen2660/def#isImplementedBy">
    <rdf:type rdf:resource="http://www.w3.org/1999/02/22-rdf-syntax-ns#Property"/>
    <rdf:type rdf:resource="http://www.w3.org/2002/07/owl#ObjectProperty"/>
    <rdfs:domain rdf:resource="https://w3id.org/nen2660/def#FunctionalEntity"/>
    <rdfs:range rdf:resource="https://w3id.org/nen2660/def#TechnicalEntity"/>
    <rdfs:seeAlso rdf:resource="https://w3id.org/nen2660/term#isImplementedBy"/>
    <rdfs:subPropertyOf rdf:resource="https://w3id.org/nen2660/def#hasSolution"/>
    <skos:definition xml:lang="en">The technical entity that implements a functional entity</skos:definition>
    <skos:prefLabel xml:lang="en">is implemented by</skos:prefLabel>
  </rdf:Description>
  <rdf:Description rdf:nodeID="n29315767620c4c949118ed89a344f3a5b33">
    <rdf:first rdf:resource="http://www.w3.org/2001/XMLSchema#double"/>
    <rdf:rest rdf:nodeID="n29315767620c4c949118ed89a344f3a5b34"/>
  </rdf:Description>
  <rdf:Description rdf:nodeID="n87801b7bffed4f059b3dda9335adfc9ab8">
    <rdf:first rdf:resource="https://w3id.org/nen2660/def#Gas"/>
    <rdf:rest rdf:nodeID="n87801b7bffed4f059b3dda9335adfc9ab9"/>
  </rdf:Description>
  <rdf:Description rdf:nodeID="n29315767620c4c949118ed89a344f3a5b34">
    <rdf:first rdf:resource="http://www.w3.org/2001/XMLSchema#integer"/>
    <rdf:rest rdf:resource="http://www.w3.org/1999/02/22-rdf-syntax-ns#nil"/>
  </rdf:Description>
  <rdf:Description rdf:about="https://w3id.org/nen2660/term#transforms">
    <rdf:type rdf:resource="http://www.w3.org/2004/02/skos/core#Concept"/>
    <skos:definition xml:lang="nl">Het object getransformeerd door een activiteit</skos:definition>
    <skos:definition xml:lang="en">The object transformed by an activity</skos:definition>
    <skos:prefLabel xml:lang="nl">transformeert</skos:prefLabel>
    <skos:prefLabel xml:lang="en">transforms</skos:prefLabel>
  </rdf:Description>
  <rdf:Description rdf:nodeID="n29315767620c4c949118ed89a344f3a5b29">
    <rdf:type rdf:resource="http://www.w3.org/2002/07/owl#Restriction"/>
    <owl:allValuesFrom rdf:nodeID="n29315767620c4c949118ed89a344f3a5b30"/>
    <owl:onProperty rdf:resource="http://www.w3.org/1999/02/22-rdf-syntax-ns#value"/>
  </rdf:Description>
  <rdf:Description rdf:about="https://w3id.org/nen2660/term#SpatialRegion">
    <rdf:type rdf:resource="http://www.w3.org/2004/02/skos/core#Concept"/>
    <skos:broader rdf:resource="https://w3id.org/nen2660/term#PhysicalObject"/>
    <skos:definition xml:lang="en">A physical object that encloses a particular area such as a room, roadway and river, that is bounded by real objects or other spatial areas (e.g., by usage or convention) and that contains primarily liquid or gaseous amount of matter</skos:definition>
    <skos:definition xml:lang="nl">Een fysiek object dat een bepaald gebied omsluit zoals een vertrek, rijbaan en rivier, en dat wordt begrensd door reële objecten of andere ruimtelijke gebieden (bijvoorbeeld op basis van gebruik of conventie) en dat voornamelijk vloeibare of gasvormige hoeveelheid materie bevat</skos:definition>
    <skos:prefLabel xml:lang="nl">Ruimtelijk gebied</skos:prefLabel>
    <skos:prefLabel xml:lang="en">Spatial region</skos:prefLabel>
  </rdf:Description>
  <rdf:Description rdf:about="https://w3id.org/nen2660/def#triggers">
    <rdf:type rdf:resource="http://www.w3.org/1999/02/22-rdf-syntax-ns#Property"/>
    <rdf:type rdf:resource="http://www.w3.org/2002/07/owl#ObjectProperty"/>
    <rdfs:domain rdf:resource="https://w3id.org/nen2660/def#Entity"/>
    <rdfs:range rdf:resource="https://w3id.org/nen2660/def#Event"/>
    <rdfs:seeAlso rdf:resource="https://w3id.org/nen2660/term#triggers"/>
    <skos:definition xml:lang="en">The event triggert by an entity</skos:definition>
    <skos:prefLabel xml:lang="en">triggers</skos:prefLabel>
  </rdf:Description>
  <rdf:Description rdf:about="https://w3id.org/nen2660/term#Interaction">
    <rdf:type rdf:resource="http://www.w3.org/2004/02/skos/core#Concept"/>
    <skos:broader rdf:resource="https://w3id.org/nen2660/term#Activity"/>
    <skos:definition xml:lang="nl">De activiteit zijnde een combinatie van subactiviteiten uitgevoerd door fysieke objecten waartussen een overdracht van materie, informatie, energie of kracht plaatsvindt, typisch over een verbinding of raakvlak (direct of via poorten)</skos:definition>
    <skos:definition xml:lang="en">The activity being a combination of sub-activities performed by physical objects between which a transfer of matter, information, energy or force takes place, typically over a connection or interface (directly or through ports)</skos:definition>
    <skos:prefLabel xml:lang="nl">Interactie</skos:prefLabel>
    <skos:prefLabel xml:lang="en">Interaction</skos:prefLabel>
  </rdf:Description>
  <rdf:Description rdf:nodeID="n29315767620c4c949118ed89a344f3a5b31">
    <rdf:first rdf:resource="http://www.w3.org/2001/XMLSchema#decimal"/>
    <rdf:rest rdf:nodeID="n29315767620c4c949118ed89a344f3a5b32"/>
  </rdf:Description>
  <rdf:Description rdf:about="https://w3id.org/nen2660/def#transforms">
    <rdf:type rdf:resource="http://www.w3.org/1999/02/22-rdf-syntax-ns#Property"/>
    <rdf:type rdf:resource="http://www.w3.org/2002/07/owl#ObjectProperty"/>
    <rdfs:domain rdf:resource="https://w3id.org/nen2660/def#Activity"/>
    <rdfs:range rdf:resource="https://w3id.org/nen2660/def#Object"/>
    <rdfs:seeAlso rdf:resource="https://w3id.org/nen2660/term#transforms"/>
    <skos:definition xml:lang="en">The object transformed by an activity</skos:definition>
    <skos:prefLabel xml:lang="en">transforms</skos:prefLabel>
  </rdf:Description>
  <rdf:Description rdf:about="https://w3id.org/nen2660/def#isRealizedBy">
    <rdf:type rdf:resource="http://www.w3.org/1999/02/22-rdf-syntax-ns#Property"/>
    <rdf:type rdf:resource="http://www.w3.org/2002/07/owl#ObjectProperty"/>
    <rdfs:domain rdf:resource="https://w3id.org/nen2660/def#PlannedEntity"/>
    <rdfs:range rdf:resource="https://w3id.org/nen2660/def#RealizedEntity"/>
    <rdfs:seeAlso rdf:resource="https://w3id.org/nen2660/term#isRealizedBy"/>
    <skos:definition xml:lang="en">The realized entity that realizes a planned entity</skos:definition>
    <rdfs:subPropertyOf rdf:resource="https://w3id.org/nen2660/def#isPlanFor"/>
    <skos:prefLabel xml:lang="en">is realized by</skos:prefLabel>
  </rdf:Description>
  <rdf:Description rdf:about="https://w3id.org/nen2660/owl/def">
    <rdf:type rdf:resource="http://www.w3.org/2002/07/owl#Ontology"/>
    <owl:imports rdf:resource="http://qudt.org/2.1/schema/qudt"/>
    <owl:imports rdf:resource="http://qudt.org/2.1/vocab/quantitykind"/>
    <owl:imports rdf:resource="http://qudt.org/2.1/vocab/unit"/>
    <owl:imports rdf:resource="http://www.w3.org/2004/02/skos/core"/>
    <owl:imports rdf:resource="http://www.w3.org/2006/time"/>
    <owl:imports rdf:resource="http://www.w3.org/ns/shacl"/>
    <owl:imports rdf:resource="https://w3id.org/nen2660/rdfs/def"/>
  </rdf:Description>
  <rdf:Description rdf:nodeID="n87801b7bffed4f059b3dda9335adfc9ab53">
    <rdf:first rdf:nodeID="n87801b7bffed4f059b3dda9335adfc9ab50"/>
    <rdf:rest rdf:resource="http://www.w3.org/1999/02/22-rdf-syntax-ns#nil"/>
  </rdf:Description>
  <rdf:Description rdf:about="https://w3id.org/nen2660/def#Matter">
    <rdf:type rdf:resource="http://www.w3.org/2000/01/rdf-schema#Class"/>
    <rdf:type rdf:resource="http://www.w3.org/ns/shacl#NodeShape"/>
    <rdf:type rdf:resource="http://www.w3.org/2002/07/owl#Class"/>
    <rdfs:seeAlso rdf:resource="https://w3id.org/nen2660/term#Matter"/>
    <rdfs:subClassOf rdf:resource="https://w3id.org/nen2660/def#PhysicalObject"/>
    <skos:definition xml:lang="en">A pure chemical substance, chemical compound or mixture from which real objects are made</skos:definition>
    <skos:prefLabel xml:lang="en">Matter</skos:prefLabel>
    <sh:property rdf:nodeID="n87801b7bffed4f059b3dda9335adfc9ab30"/>
    <sh:property rdf:nodeID="n87801b7bffed4f059b3dda9335adfc9ab31"/>
  </rdf:Description>
  <rdf:Description rdf:about="https://w3id.org/nen2660/term#QualityValue">
    <rdf:type rdf:resource="http://www.w3.org/2004/02/skos/core#Concept"/>
    <skos:broader rdf:resource="https://w3id.org/nen2660/term#Objectification"/>
    <skos:definition xml:lang="nl">De objectivering van een waarde van een kwaliteit met een complexe waarde zoals een eenvoudige waarde sec gecombineerd met andere metadata of alleen een combinatie van eenvoudige waarden</skos:definition>
    <skos:definition xml:lang="en">The objectification of a value of a quality having a complex value like a simple value sec combined with other metadata or just a combination of simple values</skos:definition>
    <skos:prefLabel xml:lang="nl">Kwaliteitwaarde</skos:prefLabel>
    <skos:prefLabel xml:lang="en">Quality value</skos:prefLabel>
  </rdf:Description>
  <rdf:Description rdf:nodeID="n29315767620c4c949118ed89a344f3a5b18">
    <rdf:type rdf:resource="http://www.w3.org/2002/07/owl#Restriction"/>
    <owl:allValuesFrom rdf:resource="https://w3id.org/nen2660/def#Entity"/>
    <owl:onProperty rdf:resource="https://w3id.org/nen2660/def#hasPart"/>
  </rdf:Description>
  <rdf:Description rdf:nodeID="n87801b7bffed4f059b3dda9335adfc9ab91">
    <sh:zeroOrMorePath rdf:resource="http://www.w3.org/2000/01/rdf-schema#subClassOf"/>
  </rdf:Description>
  <rdf:Description rdf:about="https://w3id.org/nen2660/term#hasPart">
    <rdf:type rdf:resource="http://www.w3.org/2004/02/skos/core#Concept"/>
    <skos:definition xml:lang="en">A decomposition (hasPart) relation between concrete concepts</skos:definition>
    <skos:definition xml:lang="nl">Een decompositie (heeftDeel) relatie tussen concrete concepten</skos:definition>
    <skos:prefLabel xml:lang="en">has part</skos:prefLabel>
    <skos:prefLabel xml:lang="nl">heeft deel</skos:prefLabel>
  </rdf:Description>
  <rdf:Description rdf:about="https://w3id.org/nen2660/def#TransferType">
    <rdf:type rdf:resource="http://www.w3.org/2000/01/rdf-schema#Class"/>
    <rdf:type rdf:resource="https://w3id.org/nen2660/def#EnumerationType"/>
    <rdf:type rdf:resource="http://www.w3.org/ns/shacl#NodeShape"/>
    <rdf:type rdf:resource="http://www.w3.org/2002/07/owl#Class"/>
    <rdfs:seeAlso rdf:resource="https://w3id.org/nen2660/term#TransferType"/>
    <skos:definition xml:lang="en">The type of thing being transferred, here: material, information, energy or force</skos:definition>
    <skos:prefLabel xml:lang="en">Transfer type</skos:prefLabel>
    <sh:in rdf:nodeID="n87801b7bffed4f059b3dda9335adfc9ab86"/>
    <owl:oneOf rdf:nodeID="n29315767620c4c949118ed89a344f3a5b48"/>
  </rdf:Description>
  <rdf:Description rdf:about="https://w3id.org/nen2660/term#Unit">
    <rdf:type rdf:resource="http://www.w3.org/2004/02/skos/core#Concept"/>
    <skos:definition xml:lang="en">A particular quantity value that has been chosen as a scale for measuring other quantities the same kind</skos:definition>
    <skos:definition xml:lang="nl">Een bepaalde hoeveelheidswaarde die is gekozen als schaal voor het meten van andere hoeveelheden van dezelfde soort</skos:definition>
    <skos:prefLabel xml:lang="nl">Eenheid</skos:prefLabel>
    <skos:prefLabel xml:lang="en">Unit</skos:prefLabel>
  </rdf:Description>
  <rdf:Description rdf:nodeID="n87801b7bffed4f059b3dda9335adfc9ab67">
    <sh:path rdf:resource="https://w3id.org/nen2660/def#requirementSeverityType"/>
    <sh:class rdf:resource="https://w3id.org/nen2660/def#RequirementSeverityType"/>
  </rdf:Description>
  <rdf:Description rdf:about="http://qudt.org/schema/qudt/QuantityKind">
    <rdf:type rdf:resource="https://w3id.org/nen2660/def#EnumerationType"/>
    <rdfs:seeAlso rdf:resource="https://w3id.org/nen2660/term#QuantityKind"/>
    <skos:definition xml:lang="en">Any observable property that can be measured and quantified numerically</skos:definition>
    <skos:prefLabel xml:lang="en">Quantity kind</skos:prefLabel>
  </rdf:Description>
  <rdf:Description rdf:about="https://w3id.org/nen2660/term#Matter">
    <rdf:type rdf:resource="http://www.w3.org/2004/02/skos/core#Concept"/>
    <skos:altLabel xml:lang="en">Chemical substance</skos:altLabel>
    <skos:broader rdf:resource="https://w3id.org/nen2660/term#PhysicalObject"/>
    <skos:definition xml:lang="en">A pure chemical substance, chemical compound or mixture from which real objects are made</skos:definition>
    <skos:definition xml:lang="nl">Een pure chemische stof, chemische verbinding of mengsel waaruit reële objecten zijn gemaakt</skos:definition>
    <skos:prefLabel xml:lang="nl">Materie</skos:prefLabel>
    <skos:prefLabel xml:lang="en">Matter</skos:prefLabel>
  </rdf:Description>
  <rdf:Description rdf:about="https://w3id.org/nen2660/def#RequirementSourceType">
    <rdf:type rdf:resource="http://www.w3.org/2000/01/rdf-schema#Class"/>
    <rdf:type rdf:resource="https://w3id.org/nen2660/def#EnumerationType"/>
    <rdf:type rdf:resource="http://www.w3.org/2002/07/owl#Class"/>
    <rdfs:seeAlso rdf:resource="https://w3id.org/nen2660/term#RequirementSourceType"/>
    <skos:definition xml:lang="en">The type of source from which a requirement comes like a client, by definition, recommended by the sector or demanded by law/regulation</skos:definition>
    <skos:prefLabel xml:lang="en">Requirement source type</skos:prefLabel>
  </rdf:Description>
  <rdf:Description rdf:about="https://w3id.org/nen2660/term#Liquid">
    <rdf:type rdf:resource="http://www.w3.org/2004/02/skos/core#Concept"/>
    <skos:broader rdf:resource="https://w3id.org/nen2660/term#AggregationStateType"/>
    <skos:definition xml:lang="en">A liquid is a nearly incompressible fluid that conforms to the shape of its container but retains a (nearly) constant volume independent of pressure</skos:definition>
    <skos:definition xml:lang="nl">Een vloeistof is een bijna onsamendrukbare vloeistof die zich aanpast aan de vorm van de houder, maar een (bijna) constant volume behoudt, onafhankelijk van de druk</skos:definition>
    <skos:prefLabel xml:lang="en">Liquid</skos:prefLabel>
    <skos:prefLabel xml:lang="nl">Vloeistof</skos:prefLabel>
  </rdf:Description>
  <rdf:Description rdf:nodeID="n87801b7bffed4f059b3dda9335adfc9ab25">
    <sh:path rdf:resource="https://w3id.org/nen2660/def#overConnection"/>
    <sh:class rdf:resource="https://w3id.org/nen2660/def#Connection"/>
  </rdf:Description>
  <rdf:Description rdf:about="https://w3id.org/nen2660/def#Event">
    <rdf:type rdf:resource="http://www.w3.org/2000/01/rdf-schema#Class"/>
    <rdf:type rdf:resource="http://www.w3.org/ns/shacl#NodeShape"/>
    <rdf:type rdf:resource="http://www.w3.org/2002/07/owl#Class"/>
    <rdfs:seeAlso rdf:resource="https://w3id.org/nen2660/term#Event"/>
    <rdfs:subClassOf rdf:resource="https://w3id.org/nen2660/def#ConcreteConcept"/>
    <rdfs:subClassOf rdf:nodeID="n29315767620c4c949118ed89a344f3a5b17"/>
    <skos:definition xml:lang="en">Transition between two successive states of an entity (object or activity). An event is triggered in a state</skos:definition>
    <skos:prefLabel xml:lang="en">Event</skos:prefLabel>
    <sh:property rdf:nodeID="n87801b7bffed4f059b3dda9335adfc9ab19"/>
    <sh:property rdf:nodeID="n87801b7bffed4f059b3dda9335adfc9ab20"/>
    <sh:property rdf:nodeID="n87801b7bffed4f059b3dda9335adfc9ab21"/>
  </rdf:Description>
  <rdf:Description rdf:about="https://w3id.org/nen2660/def#SpatialRegion">
    <rdf:type rdf:resource="http://www.w3.org/2000/01/rdf-schema#Class"/>
    <rdf:type rdf:resource="http://www.w3.org/ns/shacl#NodeShape"/>
    <rdf:type rdf:resource="http://www.w3.org/2002/07/owl#Class"/>
    <rdfs:seeAlso rdf:resource="https://w3id.org/nen2660/term#SpatialRegion"/>
    <rdfs:subClassOf rdf:resource="https://w3id.org/nen2660/def#PhysicalObject"/>
    <rdfs:subClassOf rdf:nodeID="n29315767620c4c949118ed89a344f3a5b42"/>
    <skos:definition xml:lang="en">A physical object that encloses a particular area such as a room, roadway and river, that is bounded by real objects or other spatial areas (e.g., by usage or convention) and that contains primarily liquid or gaseous amount of matter</skos:definition>
    <skos:prefLabel xml:lang="en">Spatial region</skos:prefLabel>
    <sh:property rdf:nodeID="n87801b7bffed4f059b3dda9335adfc9ab70"/>
    <sh:property rdf:nodeID="n87801b7bffed4f059b3dda9335adfc9ab71"/>
    <sh:property rdf:nodeID="n87801b7bffed4f059b3dda9335adfc9ab76"/>
  </rdf:Description>
  <rdf:Description rdf:about="https://w3id.org/nen2660/term#portion">
    <rdf:type rdf:resource="http://www.w3.org/2004/02/skos/core#Concept"/>
    <skos:definition xml:lang="nl">Het relatieve deel van een materiedeel</skos:definition>
    <skos:definition xml:lang="en">The relative portion of a matter portion</skos:definition>
    <skos:prefLabel xml:lang="nl">aandeel</skos:prefLabel>
    <skos:prefLabel xml:lang="en">portion</skos:prefLabel>
  </rdf:Description>
  <rdf:Description rdf:about="https://w3id.org/nen2660/def#isDescribedBy">
    <rdf:type rdf:resource="http://www.w3.org/1999/02/22-rdf-syntax-ns#Property"/>
    <rdf:type rdf:resource="http://www.w3.org/2002/07/owl#ObjectProperty"/>
    <rdfs:domain rdf:resource="https://w3id.org/nen2660/def#TopConcept"/>
    <rdfs:range rdf:resource="https://w3id.org/nen2660/def#InformationObject"/>
    <rdfs:seeAlso rdf:resource="https://w3id.org/nen2660/term#isDescribedBy"/>
    <skos:definition xml:lang="en">The information object that describes something</skos:definition>
    <skos:prefLabel xml:lang="en">is described by</skos:prefLabel>
  </rdf:Description>
  <rdf:Description rdf:about="https://w3id.org/nen2660/term#Entity">
    <rdf:type rdf:resource="http://www.w3.org/2004/02/skos/core#Concept"/>
    <skos:broader rdf:resource="https://w3id.org/nen2660/term#ConcreteConcept"/>
    <skos:definition xml:lang="nl">Concept dat een manifestatie en een afbakening vormt in een concrete ruimte-tijd, en dat op ieder moment in de tijd een bepaalde toestand heeft. Een entiteit heeft een unieke identiteit die constant blijft gedurende de levenscyclus. De levenscyclus van een entiteit is opgebouwd uit de reeks van toestanden van die entiteit, die elkaar in de tijd opvolgen. Een entiteit is een object of een activiteit. Een object bestaat, een activiteit vindt plaats</skos:definition>
    <skos:definition xml:lang="en">Concept that forms a manifestation and a demarcation in a concrete space-time, and which has a certain state at any moment in time. An entity has a unique identity that remains constant throughout its life cycle. The life cycle of an entity is made up of the sequence of states of that entity, which follow each other in time. An entity is an object or an activity. An object exists, an activity takes place</skos:definition>
    <skos:prefLabel xml:lang="nl">Entiteit</skos:prefLabel>
    <skos:prefLabel xml:lang="en">Entity</skos:prefLabel>
  </rdf:Description>
  <rdf:Description rdf:about="https://w3id.org/nen2660/term#PureSubstance">
    <rdf:type rdf:resource="http://www.w3.org/2004/02/skos/core#Concept"/>
    <skos:broader rdf:resource="https://w3id.org/nen2660/term#Matter"/>
    <skos:definition xml:lang="nl">Een chemische stof die een gelijke chemische samenstelling en herkenbare uniforme en isotrope eigenschappen heeft</skos:definition>
    <skos:definition xml:lang="en">Chemical matter that has an equal chemical composition and recognizable uniform and isotropic properties</skos:definition>
    <skos:prefLabel xml:lang="en">Pure substance</skos:prefLabel>
    <skos:prefLabel xml:lang="nl">Zuivere stof</skos:prefLabel>
  </rdf:Description>
  <rdf:Description rdf:about="https://w3id.org/nen2660/def#transferType">
    <rdf:type rdf:resource="http://www.w3.org/1999/02/22-rdf-syntax-ns#Property"/>
    <rdf:type rdf:resource="http://www.w3.org/2002/07/owl#ObjectProperty"/>
    <rdfs:domain rdf:resource="https://w3id.org/nen2660/def#Interaction"/>
    <rdfs:range rdf:resource="https://w3id.org/nen2660/def#TransferType"/>
    <rdfs:seeAlso rdf:resource="https://w3id.org/nen2660/term#transferType"/>
    <skos:definition xml:lang="en">The possession of a transfer type by an interaction</skos:definition>
    <skos:prefLabel xml:lang="en">transfer type</skos:prefLabel>
  </rdf:Description>
  <rdf:Description rdf:about="https://w3id.org/nen2660/def#Type">
    <rdf:type rdf:resource="http://www.w3.org/2000/01/rdf-schema#Class"/>
    <rdf:type rdf:resource="http://www.w3.org/2002/07/owl#Class"/>
    <rdfs:seeAlso rdf:resource="https://w3id.org/nen2660/term#Type"/>
    <rdfs:subClassOf rdf:resource="https://w3id.org/nen2660/def#AbstractConcept"/>
    <skos:definition xml:lang="en">A meta-concept which instances are concepts (not individuals)</skos:definition>
    <skos:prefLabel xml:lang="en">Type</skos:prefLabel>
  </rdf:Description>
  <rdf:Description rdf:about="https://w3id.org/nen2660/term#GeometricEntity">
    <rdf:type rdf:resource="http://www.w3.org/2004/02/skos/core#Concept"/>
    <skos:broader rdf:resource="https://w3id.org/nen2660/term#Representation"/>
    <skos:definition xml:lang="nl">Benoemd concept, dat een daadwerkelijke of virtuele afbakening vormt in een concrete (fysieke, driedimensionale) ruimte, die we in de werkelijkheid ervaren</skos:definition>
    <skos:definition xml:lang="en">Named concept, which forms an actual or virtual demarcation in a concrete (physical, three-dimensional) space, which we experience in reality</skos:definition>
    <skos:prefLabel xml:lang="en">Geometric entity</skos:prefLabel>
    <skos:prefLabel xml:lang="nl">Geometrische entiteit</skos:prefLabel>
  </rdf:Description>
  <rdf:Description rdf:about="https://w3id.org/nen2660/term#Force">
    <rdf:type rdf:resource="http://www.w3.org/2004/02/skos/core#Concept"/>
    <skos:broader rdf:resource="https://w3id.org/nen2660/term#TransferType"/>
    <skos:definition xml:lang="nl">Natuurkundige grootheid die, uitgeoefend op een lichaam, daarin een spanning of druk doet ontstaan, of die het lichaam van beweging doet veranderen, doet versnellen</skos:definition>
    <skos:definition xml:lang="en">Physical quantity which, when exerted on a body, causes tension or pressure to arise therein, or which causes the body to change motion, accelerate</skos:definition>
    <skos:prefLabel xml:lang="en">Force</skos:prefLabel>
    <skos:prefLabel xml:lang="nl">Kracht</skos:prefLabel>
  </rdf:Description>
  <rdf:Description rdf:about="https://w3id.org/nen2660/def#connectsObject">
    <rdf:type rdf:resource="http://www.w3.org/1999/02/22-rdf-syntax-ns#Property"/>
    <rdf:type rdf:resource="http://www.w3.org/2002/07/owl#ObjectProperty"/>
    <rdfs:range rdf:resource="https://w3id.org/nen2660/def#PhysicalObject"/>
    <rdfs:seeAlso rdf:resource="https://w3id.org/nen2660/term#connectsObject"/>
    <skos:definition xml:lang="en">The physical objects connected by a connection or interface</skos:definition>
    <skos:prefLabel xml:lang="en">connects object</skos:prefLabel>
    <rdfs:domain rdf:nodeID="n29315767620c4c949118ed89a344f3a5b52"/>
  </rdf:Description>
  <rdf:Description rdf:about="https://w3id.org/nen2660/def#overInterface">
    <rdf:type rdf:resource="http://www.w3.org/1999/02/22-rdf-syntax-ns#Property"/>
    <rdf:type rdf:resource="http://www.w3.org/2002/07/owl#ObjectProperty"/>
    <rdfs:domain rdf:resource="https://w3id.org/nen2660/def#Interaction"/>
    <rdfs:range rdf:resource="https://w3id.org/nen2660/def#Interface"/>
    <rdfs:seeAlso rdf:resource="https://w3id.org/nen2660/term#overInterface"/>
    <skos:definition xml:lang="en">The interface over which an interaction between physical objects takes place</skos:definition>
    <skos:prefLabel xml:lang="en">over interface</skos:prefLabel>
  </rdf:Description>
  <rdf:Description rdf:about="https://w3id.org/nen2660/def#ConceptType">
    <rdf:type rdf:resource="http://www.w3.org/2000/01/rdf-schema#Class"/>
    <rdf:type rdf:resource="http://www.w3.org/2002/07/owl#Class"/>
    <rdfs:seeAlso rdf:resource="https://w3id.org/nen2660/term#ConceptType"/>
    <rdfs:subClassOf rdf:resource="https://w3id.org/nen2660/def#Type"/>
    <skos:definition xml:lang="en">A meta-concept having concepts as instances that can have attributes or relations</skos:definition>
    <skos:prefLabel xml:lang="en">Concept type</skos:prefLabel>
  </rdf:Description>
  <rdf:Description rdf:about="https://w3id.org/nen2660/term#hasState">
    <rdf:type rdf:resource="http://www.w3.org/2004/02/skos/core#Concept"/>
    <skos:definition xml:lang="nl">De toestand van een entiteit op een bepaald tijdstip of in een bepaalde periode</skos:definition>
    <skos:definition xml:lang="en">The state of an entity in a certain point or period of time</skos:definition>
    <skos:prefLabel xml:lang="en">has state</skos:prefLabel>
    <skos:prefLabel xml:lang="nl">heeft toestand</skos:prefLabel>
  </rdf:Description>
  <rdf:Description rdf:about="https://w3id.org/nen2660/term#isRealizedBy">
    <rdf:type rdf:resource="http://www.w3.org/2004/02/skos/core#Concept"/>
    <skos:broader rdf:resource="https://w3id.org/nen2660/term#isPlanFor"/>
    <skos:definition xml:lang="nl">De gerealiseerde entiteit die een geplande entiteit realiseert</skos:definition>
    <skos:definition xml:lang="en">The realized entity that realizes a planned entity</skos:definition>
    <skos:prefLabel xml:lang="nl">is gerealiseerd door</skos:prefLabel>
    <skos:prefLabel xml:lang="en">is realized by</skos:prefLabel>
  </rdf:Description>
  <rdf:Description rdf:about="https://w3id.org/nen2660/def#hasState">
    <rdf:type rdf:resource="http://www.w3.org/1999/02/22-rdf-syntax-ns#Property"/>
    <rdf:type rdf:resource="http://www.w3.org/2002/07/owl#ObjectProperty"/>
    <rdfs:domain rdf:resource="https://w3id.org/nen2660/def#Entity"/>
    <rdfs:range rdf:resource="https://w3id.org/nen2660/def#State"/>
    <rdfs:seeAlso rdf:resource="https://w3id.org/nen2660/term#hasState"/>
    <skos:definition xml:lang="en">The state of an entity in a certain point or period of time</skos:definition>
    <skos:prefLabel xml:lang="en">has state</skos:prefLabel>
  </rdf:Description>
  <rdf:Description rdf:nodeID="n29315767620c4c949118ed89a344f3a5b25">
    <rdf:type rdf:resource="http://www.w3.org/2002/07/owl#Class"/>
    <owl:unionOf rdf:nodeID="n29315767620c4c949118ed89a344f3a5b26"/>
  </rdf:Description>
  <rdf:Description rdf:about="https://w3id.org/nen2660/def#DiscreteObject">
    <rdf:type rdf:resource="http://www.w3.org/2000/01/rdf-schema#Class"/>
    <rdf:type rdf:resource="http://www.w3.org/2002/07/owl#Class"/>
    <rdfs:seeAlso rdf:resource="https://w3id.org/nen2660/term#DiscreteObject"/>
    <rdfs:subClassOf rdf:resource="https://w3id.org/nen2660/def#RealObject"/>
    <skos:definition xml:lang="en">A real object consisting of a contiguous amount of form-retaining matter, held together primarily by internal forces (gravity or electromagnetic force)</skos:definition>
    <skos:prefLabel xml:lang="en">Discrete object</skos:prefLabel>
  </rdf:Description>
  <rdf:Description rdf:about="https://w3id.org/nen2660/def#portion">
    <rdf:type rdf:resource="http://www.w3.org/1999/02/22-rdf-syntax-ns#Property"/>
    <rdf:type rdf:resource="http://www.w3.org/2002/07/owl#ObjectProperty"/>
    <rdfs:domain rdf:resource="https://w3id.org/nen2660/def#MatterPortion"/>
    <rdfs:range rdf:resource="https://w3id.org/nen2660/def#QuantityValue"/>
    <rdfs:seeAlso rdf:resource="https://w3id.org/nen2660/term#portion"/>
    <skos:definition xml:lang="en">The relative portion of a matter portion</skos:definition>
    <skos:prefLabel xml:lang="en">portion</skos:prefLabel>
    <nen2660:hasQuantityKind rdf:resource="http://qudt.org/vocab/quantitykind/DimensionlessRatio"/>
  </rdf:Description>
  <rdf:Description rdf:nodeID="n29315767620c4c949118ed89a344f3a5b37">
    <rdf:first rdf:resource="https://w3id.org/nen2660/def#RealObject"/>
    <rdf:rest rdf:nodeID="n29315767620c4c949118ed89a344f3a5b38"/>
  </rdf:Description>
  <rdf:Description rdf:about="https://w3id.org/nen2660/def#begins">
    <rdf:type rdf:resource="http://www.w3.org/1999/02/22-rdf-syntax-ns#Property"/>
    <rdf:type rdf:resource="http://www.w3.org/2002/07/owl#ObjectProperty"/>
    <rdfs:domain rdf:resource="https://w3id.org/nen2660/def#Event"/>
    <rdfs:range rdf:resource="https://w3id.org/nen2660/def#State"/>
    <rdfs:seeAlso rdf:resource="https://w3id.org/nen2660/term#begins"/>
    <skos:definition xml:lang="en">The state that is started by an event</skos:definition>
    <skos:prefLabel xml:lang="en">begins</skos:prefLabel>
  </rdf:Description>
  <rdf:Description rdf:about="https://w3id.org/nen2660/term#RequirementTopicType">
    <rdf:type rdf:resource="http://www.w3.org/2004/02/skos/core#Concept"/>
    <skos:broader rdf:resource="https://w3id.org/nen2660/term#EnumerationType"/>
    <skos:definition xml:lang="nl">Het entiteitsaspect waarop een eis van toepassing is</skos:definition>
    <skos:definition xml:lang="en">The entity aspect a requirement applies to</skos:definition>
    <skos:prefLabel xml:lang="nl">Eis onderwerp type</skos:prefLabel>
    <skos:prefLabel xml:lang="en">Requirement topic type</skos:prefLabel>
  </rdf:Description>
  <rdf:Description rdf:about="https://w3id.org/nen2660/def#Representation">
    <rdf:type rdf:resource="http://www.w3.org/2000/01/rdf-schema#Class"/>
    <rdf:type rdf:resource="http://www.w3.org/2002/07/owl#Class"/>
    <rdfs:seeAlso rdf:resource="https://w3id.org/nen2660/term#Representation"/>
    <rdfs:subClassOf rdf:resource="https://w3id.org/nen2660/def#InformationObject"/>
    <skos:definition xml:lang="en">That which represents something else</skos:definition>
    <skos:prefLabel xml:lang="en">Representation</skos:prefLabel>
  </rdf:Description>
  <rdf:Description rdf:about="https://w3id.org/nen2660/def#hasQuantityKindShape">
    <rdf:type rdf:resource="http://www.w3.org/ns/shacl#NodeShape"/>
    <sh:class rdf:resource="http://qudt.org/schema/qudt/QuantityKind"/>
    <sh:targetObjectsOf rdf:resource="https://w3id.org/nen2660/def#hasQuantityKind"/>
  </rdf:Description>
  <rdf:Description rdf:about="https://w3id.org/nen2660/term#ConcreteConcept">
    <rdf:type rdf:resource="http://www.w3.org/2004/02/skos/core#Concept"/>
    <skos:broader rdf:resource="https://w3id.org/nen2660/term#TopConcept"/>
    <skos:definition xml:lang="nl">Concept dat een manifestatie en een afbakening vormt in een concrete ruimte-tijd. Een concreet concept heeft een levenscyclus</skos:definition>
    <skos:definition xml:lang="en">Concept that forms a manifestation and a demarcation in a concrete space-time. A concrete concept has a life cycle</skos:definition>
    <skos:prefLabel xml:lang="nl">Concreet concept</skos:prefLabel>
    <skos:prefLabel xml:lang="en">Concrete concept</skos:prefLabel>
  </rdf:Description>
  <rdf:Description rdf:nodeID="n87801b7bffed4f059b3dda9335adfc9ab77">
    <sh:path rdf:resource="https://w3id.org/nen2660/def#hasBoundary"/>
    <sh:class rdf:resource="https://w3id.org/nen2660/def#GeometricEntity"/>
  </rdf:Description>
  <rdf:Description rdf:about="https://w3id.org/nen2660/term#AggregationStateType">
    <rdf:type rdf:resource="http://www.w3.org/2004/02/skos/core#Concept"/>
    <skos:broader rdf:resource="https://w3id.org/nen2660/term#EnumerationType"/>
    <skos:definition xml:lang="nl">Een van de vier fundamentele toestanden van materie zijnde een vaste stof, vloeistof, gas of plasma</skos:definition>
    <skos:definition xml:lang="en">One of the four fundamental states of matter being a solid, liquid, gas or plasma</skos:definition>
    <skos:prefLabel xml:lang="nl">Aggregatietoestandtype</skos:prefLabel>
    <skos:prefLabel xml:lang="en">Aggregation state type</skos:prefLabel>
  </rdf:Description>
  <rdf:Description rdf:about="https://w3id.org/nen2660/term#Event">
    <rdf:type rdf:resource="http://www.w3.org/2004/02/skos/core#Concept"/>
    <skos:broader rdf:resource="https://w3id.org/nen2660/term#ConcreteConcept"/>
    <skos:definition xml:lang="nl">Overgang tussen twee opeenvolgende toestanden van een entiteit (object of activiteit). Een gebeurtenis wordt getriggerd in een toestand</skos:definition>
    <skos:definition xml:lang="en">Transition between two successive states of an entity (object or activity). An event is triggered in a state</skos:definition>
    <skos:prefLabel xml:lang="en">Event</skos:prefLabel>
    <skos:prefLabel xml:lang="nl">Gebeurtenis</skos:prefLabel>
  </rdf:Description>
  <rdf:Description rdf:about="https://w3id.org/nen2660/term#transferType">
    <rdf:type rdf:resource="http://www.w3.org/2004/02/skos/core#Concept"/>
    <skos:definition xml:lang="nl">Het hebben van een overdrachtstype door een interactie</skos:definition>
    <skos:definition xml:lang="en">The possession of a transfer type by an interaction</skos:definition>
    <skos:prefLabel xml:lang="nl">overdrachtstype</skos:prefLabel>
    <skos:prefLabel xml:lang="en">transfer type</skos:prefLabel>
  </rdf:Description>
  <rdf:Description rdf:nodeID="n29315767620c4c949118ed89a344f3a5b19">
    <rdf:type rdf:resource="http://www.w3.org/2002/07/owl#Restriction"/>
    <owl:cardinality rdf:datatype="http://www.w3.org/2001/XMLSchema#nonNegativeInteger">1</owl:cardinality>
    <owl:onProperty rdf:resource="https://w3id.org/nen2660/def#portion"/>
  </rdf:Description>
  <rdf:Description rdf:about="https://w3id.org/nen2660/term#TransferType">
    <rdf:type rdf:resource="http://www.w3.org/2004/02/skos/core#Concept"/>
    <skos:broader rdf:resource="https://w3id.org/nen2660/term#EnumerationType"/>
    <skos:definition xml:lang="nl">Het soort ding dat wordt overgedragen, hier: materiaal, informatie, energie of kracht</skos:definition>
    <skos:definition xml:lang="en">The type of thing being transferred, here: material, information, energy or force</skos:definition>
    <skos:prefLabel xml:lang="nl">Overdrachtstype</skos:prefLabel>
    <skos:prefLabel xml:lang="en">Transfer type</skos:prefLabel>
  </rdf:Description>
  <rdf:Description rdf:about="https://w3id.org/nen2660/def#consistsOf">
    <rdf:type rdf:resource="http://www.w3.org/1999/02/22-rdf-syntax-ns#Property"/>
    <rdf:type rdf:resource="http://www.w3.org/2002/07/owl#ObjectProperty"/>
    <rdfs:seeAlso rdf:resource="https://w3id.org/nen2660/term#consistsOf"/>
    <skos:definition xml:lang="en">The matter a real object or mixture is made of</skos:definition>
    <skos:prefLabel xml:lang="en">consists of</skos:prefLabel>
    <rdfs:domain rdf:nodeID="n29315767620c4c949118ed89a344f3a5b58"/>
    <rdfs:range rdf:nodeID="n29315767620c4c949118ed89a344f3a5b61"/>
  </rdf:Description>
  <rdf:Description rdf:about="https://w3id.org/nen2660/term#Gas">
    <rdf:type rdf:resource="http://www.w3.org/2004/02/skos/core#Concept"/>
    <skos:broader rdf:resource="https://w3id.org/nen2660/term#AggregationStateType"/>
    <skos:definition xml:lang="nl">Materie in een tussentoestand tussen vloeistof en plasma die alleen kan worden ingesloten als deze volledig is omgeven door een vaste stof (of in een bel van vloeistof) (of bij elkaar wordt gehouden door zwaartekracht); het kan condenseren tot een vloeistof, of kan (zelden) direct een vaste stof worden door afzetting</skos:definition>
    <skos:definition xml:lang="en">Matter in an intermediate state between liquid and plasma that can be contained only if it is fully surrounded by a solid (or in a bubble of liquid) (or held together by gravitational pull); it can condense into a liquid, or can (rarely) become a solid directly by deposition</skos:definition>
    <skos:prefLabel xml:lang="en">Gas</skos:prefLabel>
    <skos:prefLabel xml:lang="nl">Gas</skos:prefLabel>
  </rdf:Description>
  <rdf:Description rdf:about="https://w3id.org/nen2660/def#Mixture">
    <rdf:type rdf:resource="http://www.w3.org/2000/01/rdf-schema#Class"/>
    <rdf:type rdf:resource="http://www.w3.org/ns/shacl#NodeShape"/>
    <rdf:type rdf:resource="http://www.w3.org/2002/07/owl#Class"/>
    <rdfs:seeAlso rdf:resource="https://w3id.org/nen2660/term#Mixture"/>
    <rdfs:subClassOf rdf:resource="https://w3id.org/nen2660/def#Matter"/>
    <skos:definition xml:lang="en">The combination of two or more different pure substances without the molecules losing their identity</skos:definition>
    <skos:prefLabel xml:lang="en">Mixture</skos:prefLabel>
    <sh:property rdf:nodeID="n87801b7bffed4f059b3dda9335adfc9ab33"/>
  </rdf:Description>
  <rdf:Description rdf:nodeID="n29315767620c4c949118ed89a344f3a5b47">
    <rdf:type rdf:resource="http://www.w3.org/2002/07/owl#Restriction"/>
    <owl:allValuesFrom rdf:resource="https://w3id.org/nen2660/def#Entity"/>
    <owl:onProperty rdf:resource="https://w3id.org/nen2660/def#hasPart"/>
  </rdf:Description>
  <rdf:Description rdf:about="https://w3id.org/nen2660/def#Object">
    <rdf:type rdf:resource="http://www.w3.org/2000/01/rdf-schema#Class"/>
    <rdf:type rdf:resource="http://www.w3.org/ns/shacl#NodeShape"/>
    <rdf:type rdf:resource="http://www.w3.org/2002/07/owl#Class"/>
    <rdfs:seeAlso rdf:resource="https://w3id.org/nen2660/term#Object"/>
    <rdfs:subClassOf rdf:resource="https://w3id.org/nen2660/def#Entity"/>
    <rdfs:subClassOf rdf:nodeID="n29315767620c4c949118ed89a344f3a5b21"/>
    <skos:definition xml:lang="en">Entity that exists or can exist within a concrete space-time. An object executes an activity, and is transformed by an activity</skos:definition>
    <skos:prefLabel xml:lang="en">Object</skos:prefLabel>
    <sh:property rdf:nodeID="n87801b7bffed4f059b3dda9335adfc9ab38"/>
  </rdf:Description>
  <rdf:Description rdf:nodeID="n29315767620c4c949118ed89a344f3a5b54">
    <rdf:first rdf:resource="https://w3id.org/nen2660/def#Interface"/>
    <rdf:rest rdf:resource="http://www.w3.org/1999/02/22-rdf-syntax-ns#nil"/>
  </rdf:Description>
  <rdf:Description rdf:nodeID="n87801b7bffed4f059b3dda9335adfc9ab66">
    <sh:path rdf:resource="http://www.w3.org/1999/02/22-rdf-syntax-ns#value"/>
    <sh:datatype rdf:resource="http://www.w3.org/2001/XMLSchema#string"/>
    <sh:maxCount rdf:datatype="http://www.w3.org/2001/XMLSchema#integer">1</sh:maxCount>
    <sh:minCount rdf:datatype="http://www.w3.org/2001/XMLSchema#integer">1</sh:minCount>
  </rdf:Description>
  <rdf:Description rdf:nodeID="n87801b7bffed4f059b3dda9335adfc9ab27">
    <sh:path rdf:resource="https://w3id.org/nen2660/def#transferType"/>
    <sh:class rdf:resource="https://w3id.org/nen2660/def#TransferType"/>
  </rdf:Description>
  <rdf:Description rdf:nodeID="n87801b7bffed4f059b3dda9335adfc9ab32">
    <sh:path rdf:resource="https://w3id.org/nen2660/def#portion"/>
    <sh:class rdf:resource="https://w3id.org/nen2660/def#QuantityValue"/>
    <sh:maxCount rdf:datatype="http://www.w3.org/2001/XMLSchema#integer">1</sh:maxCount>
    <sh:minCount rdf:datatype="http://www.w3.org/2001/XMLSchema#integer">1</sh:minCount>
  </rdf:Description>
  <rdf:Description rdf:about="https://w3id.org/nen2660/def#QualityValue">
    <rdf:type rdf:resource="http://www.w3.org/2000/01/rdf-schema#Class"/>
    <rdf:type rdf:resource="http://www.w3.org/ns/shacl#NodeShape"/>
    <rdf:type rdf:resource="http://www.w3.org/2002/07/owl#Class"/>
    <rdfs:seeAlso rdf:resource="https://w3id.org/nen2660/term#QualityValue"/>
    <rdfs:subClassOf rdf:resource="https://w3id.org/nen2660/def#Objectification"/>
    <rdfs:subClassOf rdf:nodeID="n29315767620c4c949118ed89a344f3a5b24"/>
    <skos:definition xml:lang="en">The objectification of a value of a quality having a complex value like a simple value sec combined with other metadata or just a combination of simple values</skos:definition>
    <skos:prefLabel xml:lang="en">Quality value</skos:prefLabel>
    <sh:property rdf:nodeID="n87801b7bffed4f059b3dda9335adfc9ab46"/>
  </rdf:Description>
  <rdf:Description rdf:about="https://w3id.org/nen2660/def#ChemicalElement">
    <rdf:type rdf:resource="http://www.w3.org/2000/01/rdf-schema#Class"/>
    <rdf:type rdf:resource="http://www.w3.org/2002/07/owl#Class"/>
    <rdfs:seeAlso rdf:resource="https://w3id.org/nen2660/term#ChemicalElement"/>
    <rdfs:subClassOf rdf:resource="https://w3id.org/nen2660/def#PureSubstance"/>
    <skos:definition xml:lang="en">Pure substance that is made up of atoms with the same atomic number. A chemical element cannot be decomposed through chemical reactions</skos:definition>
    <skos:prefLabel xml:lang="en">Chemical element</skos:prefLabel>
  </rdf:Description>
  <rdf:Description rdf:about="https://w3id.org/nen2660/term#MatterPortion">
    <rdf:type rdf:resource="http://www.w3.org/2004/02/skos/core#Concept"/>
    <skos:broader rdf:resource="https://w3id.org/nen2660/term#RelationReference"/>
    <skos:definition xml:lang="en">An objectified relation reference for the consists of relation</skos:definition>
    <skos:definition xml:lang="nl">Een geobjectiveerde relatiereferentie voor de bestaat uit relatie</skos:definition>
    <skos:prefLabel xml:lang="nl">Materie-aandeel</skos:prefLabel>
    <skos:prefLabel xml:lang="en">Matter portion</skos:prefLabel>
  </rdf:Description>
  <rdf:Description rdf:nodeID="n87801b7bffed4f059b3dda9335adfc9ab22">
    <sh:path rdf:resource="https://w3id.org/nen2660/def#hasPart"/>
    <sh:class rdf:resource="https://w3id.org/nen2660/def#Entity"/>
  </rdf:Description>
  <rdf:Description rdf:about="https://w3id.org/nen2660/term#FunctionalEntity">
    <rdf:type rdf:resource="http://www.w3.org/2004/02/skos/core#Concept"/>
    <skos:broader rdf:resource="https://w3id.org/nen2660/term#Entity"/>
    <skos:definition xml:lang="en">An entity involving the external behavior where the output contributes to stakeholder objectives implemented/played by one or more technical entities</skos:definition>
    <skos:definition xml:lang="nl">Een entiteit waarbij het gaat om het externe gedrag waarbij de uitvoer bijdraagt aan doelstellingen van belanghebbenden geïmplementeerd/gespeeld door een of meer technische entiteiten</skos:definition>
    <skos:prefLabel xml:lang="en">Functional entity</skos:prefLabel>
    <skos:prefLabel xml:lang="nl">Functionele entiteit</skos:prefLabel>
  </rdf:Description>
  <rdf:Description rdf:about="https://w3id.org/nen2660/def#AggregationStateType">
    <rdf:type rdf:resource="http://www.w3.org/2000/01/rdf-schema#Class"/>
    <rdf:type rdf:resource="https://w3id.org/nen2660/def#EnumerationType"/>
    <rdf:type rdf:resource="http://www.w3.org/ns/shacl#NodeShape"/>
    <rdf:type rdf:resource="http://www.w3.org/2002/07/owl#Class"/>
    <rdfs:seeAlso rdf:resource="https://w3id.org/nen2660/term#AggregationStateType"/>
    <skos:definition xml:lang="en">One of the four fundamental states of matter being a solid, liquid, gas or plasma</skos:definition>
    <skos:prefLabel xml:lang="en">Aggregation state type</skos:prefLabel>
    <sh:in rdf:nodeID="n87801b7bffed4f059b3dda9335adfc9ab6"/>
    <owl:oneOf rdf:nodeID="n29315767620c4c949118ed89a344f3a5b2"/>
  </rdf:Description>
  <rdf:Description rdf:about="https://w3id.org/nen2660/def#Port">
    <rdf:type rdf:resource="http://www.w3.org/2000/01/rdf-schema#Class"/>
    <rdf:type rdf:resource="http://www.w3.org/2002/07/owl#Class"/>
    <rdfs:seeAlso rdf:resource="https://w3id.org/nen2660/term#Port"/>
    <rdfs:subClassOf rdf:resource="https://w3id.org/nen2660/def#PhysicalObject"/>
    <skos:definition xml:lang="en">A physical or logical point of interaction as part of a physical object where, through a connection or interface, an interaction can take place</skos:definition>
    <skos:prefLabel xml:lang="en">Port</skos:prefLabel>
  </rdf:Description>
  <rdf:Description rdf:about="https://w3id.org/nen2660/def#hasTemporalEntity">
    <rdf:type rdf:resource="http://www.w3.org/1999/02/22-rdf-syntax-ns#Property"/>
    <rdf:type rdf:resource="http://www.w3.org/2002/07/owl#ObjectProperty"/>
    <rdfs:domain rdf:resource="https://w3id.org/nen2660/def#ConcreteConcept"/>
    <rdfs:range rdf:resource="http://www.w3.org/2006/time#TemporalEntity"/>
    <rdfs:seeAlso rdf:resource="https://w3id.org/nen2660/term#hasTemporalEntity"/>
    <skos:definition xml:lang="en">The abstract temporal entity representing a concrete concept in time</skos:definition>
    <skos:prefLabel xml:lang="en">has temporal entity</skos:prefLabel>
  </rdf:Description>
  <rdf:Description rdf:about="https://w3id.org/nen2660/term#TopConcept">
    <rdf:type rdf:resource="http://www.w3.org/2004/02/skos/core#Concept"/>
    <skos:definition xml:lang="nl">Het meest generieke concept</skos:definition>
    <skos:definition xml:lang="en">The most generic concept</skos:definition>
    <skos:prefLabel xml:lang="en">Top concept</skos:prefLabel>
    <skos:prefLabel xml:lang="nl">Top concept</skos:prefLabel>
  </rdf:Description>
  <rdf:Description rdf:about="https://w3id.org/nen2660/term#MaterialFlow">
    <rdf:type rdf:resource="http://www.w3.org/2004/02/skos/core#Concept"/>
    <skos:broader rdf:resource="https://w3id.org/nen2660/term#TransferType"/>
    <skos:definition xml:lang="nl">De beweging van een hoeveelheid materiaal</skos:definition>
    <skos:definition xml:lang="en">The movement of an amount of material</skos:definition>
    <skos:prefLabel xml:lang="nl">Materiaalstroom</skos:prefLabel>
    <skos:prefLabel xml:lang="en">Material flow</skos:prefLabel>
  </rdf:Description>
  <rdf:Description rdf:nodeID="n29315767620c4c949118ed89a344f3a5b40">
    <rdf:type rdf:resource="http://www.w3.org/2002/07/owl#Restriction"/>
    <owl:allValuesFrom rdf:resource="http://www.w3.org/2001/XMLSchema#anyURI"/>
    <owl:onProperty rdf:resource="http://www.w3.org/1999/02/22-rdf-syntax-ns#value"/>
  </rdf:Description>
  <rdf:Description rdf:nodeID="n29315767620c4c949118ed89a344f3a5b52">
    <rdf:type rdf:resource="http://www.w3.org/2002/07/owl#Class"/>
    <owl:unionOf rdf:nodeID="n29315767620c4c949118ed89a344f3a5b53"/>
  </rdf:Description>
  <rdf:Description rdf:about="https://w3id.org/nen2660/def#hasPartsGroup">
    <rdf:type rdf:resource="http://www.w3.org/1999/02/22-rdf-syntax-ns#Property"/>
    <rdf:type rdf:resource="http://www.w3.org/2002/07/owl#ObjectProperty"/>
    <rdfs:domain rdf:resource="https://w3id.org/nen2660/def#ConcreteConcept"/>
    <rdfs:range rdf:resource="http://www.w3.org/2000/01/rdf-schema#Container"/>
    <rdfs:seeAlso rdf:resource="https://w3id.org/nen2660/term#hasPart"/>
    <skos:definition xml:lang="en">The possession of an group of, potentially implicit, parts</skos:definition>
    <skos:prefLabel xml:lang="en">has parts group</skos:prefLabel>
  </rdf:Description>
  <rdf:Description rdf:about="https://w3id.org/nen2660/def#FunctionalEntity">
    <rdf:type rdf:resource="http://www.w3.org/2000/01/rdf-schema#Class"/>
    <rdf:type rdf:resource="http://www.w3.org/ns/shacl#NodeShape"/>
    <rdf:type rdf:resource="http://www.w3.org/2002/07/owl#Class"/>
    <rdfs:seeAlso rdf:resource="https://w3id.org/nen2660/term#FunctionalEntity"/>
    <rdfs:subClassOf rdf:resource="https://w3id.org/nen2660/def#Entity"/>
    <rdfs:subClassOf rdf:nodeID="n29315767620c4c949118ed89a344f3a5b18"/>
    <skos:definition xml:lang="en">An entity involving the external behavior where the output contributes to stakeholder objectives implemented/played by one or more technical entities</skos:definition>
    <skos:prefLabel xml:lang="en">Functional entity</skos:prefLabel>
    <sh:property rdf:nodeID="n87801b7bffed4f059b3dda9335adfc9ab22"/>
    <sh:property rdf:nodeID="n87801b7bffed4f059b3dda9335adfc9ab23"/>
    <sh:property rdf:nodeID="n87801b7bffed4f059b3dda9335adfc9ab24"/>
  </rdf:Description>
  <rdf:Description rdf:nodeID="n29315767620c4c949118ed89a344f3a5b59">
    <rdf:first rdf:resource="https://w3id.org/nen2660/def#RealObject"/>
    <rdf:rest rdf:nodeID="n29315767620c4c949118ed89a344f3a5b60"/>
  </rdf:Description>
  <rdf:Description rdf:about="https://w3id.org/nen2660/def#requirementTopicType">
    <rdf:type rdf:resource="http://www.w3.org/1999/02/22-rdf-syntax-ns#Property"/>
    <rdf:type rdf:resource="http://www.w3.org/2002/07/owl#ObjectProperty"/>
    <rdfs:domain rdf:resource="https://w3id.org/nen2660/def#Requirement"/>
    <rdfs:range rdf:resource="https://w3id.org/nen2660/def#RequirementTopicType"/>
    <rdfs:seeAlso rdf:resource="https://w3id.org/nen2660/term#requirementTopicType"/>
    <skos:definition xml:lang="en">The possession of a topic type by a requirement</skos:definition>
    <skos:prefLabel xml:lang="en">requirement topic type</skos:prefLabel>
  </rdf:Description>
  <rdf:Description rdf:nodeID="n87801b7bffed4f059b3dda9335adfc9ab94">
    <sh:in rdf:nodeID="n87801b7bffed4f059b3dda9335adfc9ab95"/>
  </rdf:Description>
  <rdf:Description rdf:nodeID="n87801b7bffed4f059b3dda9335adfc9ab18">
    <sh:path rdf:resource="https://w3id.org/nen2660/def#triggers"/>
    <sh:class rdf:resource="https://w3id.org/nen2660/def#Event"/>
  </rdf:Description>
  <rdf:Description rdf:about="https://w3id.org/nen2660/term#QuantityValue">
    <rdf:type rdf:resource="http://www.w3.org/2004/02/skos/core#Concept"/>
    <skos:broader rdf:resource="https://w3id.org/nen2660/term#Objectification"/>
    <skos:definition xml:lang="nl">De objectivering van een waarde van een hoeveelheid (typisch met een grootheid en een eenheid) met een complexe waarde zoals een eenvoudige waarde sec gecombineerd met andere metadata of alleen een combinatie van eenvoudige waarden</skos:definition>
    <skos:definition xml:lang="en">The objectification of a value of a quantity (typically involving a quantity kind and a unit) having a complex value like a simple value sec combined with other metadata or just a combination of simple values</skos:definition>
    <skos:prefLabel xml:lang="nl">Kwantiteitsoort</skos:prefLabel>
    <skos:prefLabel xml:lang="en">Quantity value</skos:prefLabel>
  </rdf:Description>
  <rdf:Description rdf:about="https://w3id.org/nen2660/term#hasBoundary">
    <rdf:type rdf:resource="http://www.w3.org/2004/02/skos/core#Concept"/>
    <skos:definition xml:lang="nl">De geometrische entiteit die de grens van een concreet concept vertegenwoordigt</skos:definition>
    <skos:definition xml:lang="en">The geometric entity representing the boundary of a concrete concept</skos:definition>
    <skos:prefLabel xml:lang="en">has boundary</skos:prefLabel>
    <skos:prefLabel xml:lang="nl">heeft begrenzing</skos:prefLabel>
  </rdf:Description>
  <rdf:Description rdf:nodeID="n87801b7bffed4f059b3dda9335adfc9ab23">
    <sh:path rdf:resource="https://w3id.org/nen2660/def#hasFunctionalPart"/>
    <sh:class rdf:resource="https://w3id.org/nen2660/def#FunctionalEntity"/>
  </rdf:Description>
  <rdf:Description rdf:about="https://w3id.org/nen2660/skos/term">
    <rdf:type rdf:resource="http://www.w3.org/2004/02/skos/core#ConceptScheme"/>
    <owl:imports rdf:resource="http://qudt.org/2.1/schema/qudt"/>
    <owl:imports rdf:resource="http://qudt.org/2.1/vocab/quantitykind"/>
    <owl:imports rdf:resource="http://qudt.org/2.1/vocab/unit"/>
    <owl:imports rdf:resource="http://www.w3.org/2004/02/skos/core"/>
    <owl:imports rdf:resource="http://www.w3.org/2006/time"/>
    <owl:imports rdf:resource="http://www.w3.org/ns/shacl"/>
    <skos:hasTopConcept rdf:resource="https://w3id.org/nen2660/term#TopConcept"/>
  </rdf:Description>
  <rdf:Description rdf:nodeID="n87801b7bffed4f059b3dda9335adfc9ab46">
    <sh:path rdf:resource="http://www.w3.org/1999/02/22-rdf-syntax-ns#value"/>
    <sh:datatype rdf:resource="http://www.w3.org/2001/XMLSchema#string"/>
  </rdf:Description>
  <rdf:Description rdf:about="https://w3id.org/nen2660/def#EnumerationType">
    <rdf:type rdf:resource="http://www.w3.org/2000/01/rdf-schema#Class"/>
    <rdf:type rdf:resource="http://www.w3.org/2002/07/owl#Class"/>
    <rdfs:seeAlso rdf:resource="https://w3id.org/nen2660/term#EnumerationType"/>
    <rdfs:subClassOf rdf:resource="http://www.w3.org/2000/01/rdf-schema#Container"/>
    <rdfs:subClassOf rdf:resource="https://w3id.org/nen2660/def#Type"/>
    <skos:definition xml:lang="en">A meta-concept having concepts as instances having no further attributes or relations (annotations only)</skos:definition>
    <skos:prefLabel xml:lang="en">Enumeration type</skos:prefLabel>
  </rdf:Description>
  <rdf:Description rdf:nodeID="n29315767620c4c949118ed89a344f3a5b41">
    <rdf:type rdf:resource="http://www.w3.org/2002/07/owl#Restriction"/>
    <owl:onClass rdf:resource="http://www.w3.org/2001/XMLSchema#string"/>
    <owl:onProperty rdf:resource="http://www.w3.org/1999/02/22-rdf-syntax-ns#value"/>
    <owl:qualifiedCardinality rdf:datatype="http://www.w3.org/2001/XMLSchema#nonNegativeInteger">1</owl:qualifiedCardinality>
  </rdf:Description>
  <rdf:Description rdf:about="https://w3id.org/nen2660/term#hasTechnicalPart">
    <rdf:type rdf:resource="http://www.w3.org/2004/02/skos/core#Concept"/>
    <skos:broader rdf:resource="https://w3id.org/nen2660/term#hasPart"/>
    <skos:definition xml:lang="en">A hasPart relation of a technical nature</skos:definition>
    <skos:definition xml:lang="nl">Een heeftDeel relatie van technische aard</skos:definition>
    <skos:prefLabel xml:lang="en">has technical part</skos:prefLabel>
    <skos:prefLabel xml:lang="nl">heeft technisch deel</skos:prefLabel>
  </rdf:Description>
  <rdf:Description rdf:about="https://w3id.org/nen2660/def#abbreviation">
    <rdf:type rdf:resource="http://www.w3.org/1999/02/22-rdf-syntax-ns#Property"/>
    <rdf:type rdf:resource="http://www.w3.org/2002/07/owl#AnnotationProperty"/>
    <rdfs:domain rdf:resource="https://w3id.org/nen2660/def#TopConcept"/>
    <rdfs:range rdf:resource="http://www.w3.org/2001/XMLSchema#string"/>
    <rdfs:seeAlso rdf:resource="https://w3id.org/nen2660/term#abbreviation"/>
    <rdfs:subPropertyOf rdf:resource="http://www.w3.org/2004/02/skos/core#altLabel"/>
    <skos:definition xml:lang="en">Acronym or initial word as special case of an external name</skos:definition>
    <skos:prefLabel xml:lang="en">abbreviation</skos:prefLabel>
  </rdf:Description>
  <rdf:Description rdf:nodeID="n29315767620c4c949118ed89a344f3a5b38">
    <rdf:first rdf:resource="https://w3id.org/nen2660/def#Port"/>
    <rdf:rest rdf:resource="http://www.w3.org/1999/02/22-rdf-syntax-ns#nil"/>
  </rdf:Description>
  <rdf:Description rdf:about="https://w3id.org/nen2660/def#AllDisjointClasses_3">
    <rdf:type rdf:resource="http://www.w3.org/2002/07/owl#AllDisjointClasses"/>
    <owl:members rdf:nodeID="n29315767620c4c949118ed89a344f3a5b13"/>
  </rdf:Description>
  <rdf:Description rdf:about="https://w3id.org/nen2660/term#isDescribedBy">
    <rdf:type rdf:resource="http://www.w3.org/2004/02/skos/core#Concept"/>
    <skos:definition xml:lang="nl">Het informatie object dat iets beschrijft</skos:definition>
    <skos:definition xml:lang="en">The information object that describes something</skos:definition>
    <skos:prefLabel xml:lang="nl">is beschreven door</skos:prefLabel>
    <skos:prefLabel xml:lang="en">is described by</skos:prefLabel>
  </rdf:Description>
  <rdf:Description rdf:about="https://w3id.org/nen2660/def#MaterialFlow">
    <rdf:type rdf:resource="https://w3id.org/nen2660/def#TransferType"/>
    <rdfs:seeAlso rdf:resource="https://w3id.org/nen2660/term#MaterialFlow"/>
    <skos:definition xml:lang="en">The movement of an amount of material</skos:definition>
    <skos:prefLabel xml:lang="en">Material flow</skos:prefLabel>
  </rdf:Description>
  <rdf:Description rdf:nodeID="n29315767620c4c949118ed89a344f3a5b46">
    <rdf:type rdf:resource="http://www.w3.org/2002/07/owl#Restriction"/>
    <owl:allValuesFrom rdf:resource="https://w3id.org/nen2660/def#State"/>
    <owl:onProperty rdf:resource="https://w3id.org/nen2660/def#hasPart"/>
  </rdf:Description>
  <rdf:Description rdf:about="https://w3id.org/nen2660/term#hasQuantityKind">
    <rdf:type rdf:resource="http://www.w3.org/2004/02/skos/core#Concept"/>
    <skos:definition xml:lang="nl">Het hebben van een grootheid</skos:definition>
    <skos:definition xml:lang="en">The possession of a quantity kind</skos:definition>
    <skos:prefLabel xml:lang="en">has quantity kind</skos:prefLabel>
    <skos:prefLabel xml:lang="nl">heeft kwantiteitsoort</skos:prefLabel>
  </rdf:Description>
  <rdf:Description rdf:nodeID="n29315767620c4c949118ed89a344f3a5b63">
    <rdf:first rdf:resource="https://w3id.org/nen2660/def#MatterPortion"/>
    <rdf:rest rdf:resource="http://www.w3.org/1999/02/22-rdf-syntax-ns#nil"/>
  </rdf:Description>
  <rdf:Description rdf:about="https://w3id.org/nen2660/def#hasTechnicalPart">
    <rdf:type rdf:resource="http://www.w3.org/1999/02/22-rdf-syntax-ns#Property"/>
    <rdf:type rdf:resource="http://www.w3.org/2002/07/owl#ObjectProperty"/>
    <rdfs:domain rdf:resource="https://w3id.org/nen2660/def#TechnicalEntity"/>
    <rdfs:range rdf:resource="https://w3id.org/nen2660/def#TechnicalEntity"/>
    <rdfs:seeAlso rdf:resource="https://w3id.org/nen2660/term#hasTechnicalPart"/>
    <rdfs:subPropertyOf rdf:resource="https://w3id.org/nen2660/def#hasPart"/>
    <skos:definition xml:lang="en">A hasPart relation of a technical nature</skos:definition>
    <skos:prefLabel xml:lang="en">has technical part</skos:prefLabel>
  </rdf:Description>
  <rdf:Description rdf:about="https://w3id.org/nen2660/term#EnumerationType">
    <rdf:type rdf:resource="http://www.w3.org/2004/02/skos/core#Concept"/>
    <skos:broader rdf:resource="https://w3id.org/nen2660/term#Type"/>
    <skos:definition xml:lang="en">A meta-concept having concepts as instances having no further attributes or relations (annotations only)</skos:definition>
    <skos:definition xml:lang="nl">Een meta-concept met concepten als instanties zonder verdere attributen of relaties (alleen annotaties)</skos:definition>
    <skos:prefLabel xml:lang="nl">Enumeratie type</skos:prefLabel>
    <skos:prefLabel xml:lang="en">Enumeration type</skos:prefLabel>
  </rdf:Description>
  <rdf:Description rdf:nodeID="n87801b7bffed4f059b3dda9335adfc9ab7">
    <rdf:first rdf:resource="https://w3id.org/nen2660/def#Liquid"/>
    <rdf:rest rdf:nodeID="n87801b7bffed4f059b3dda9335adfc9ab8"/>
  </rdf:Description>
  <rdf:Description rdf:about="https://w3id.org/nen2660/def#RealizedEntity">
    <rdf:type rdf:resource="http://www.w3.org/2000/01/rdf-schema#Class"/>
    <rdf:type rdf:resource="http://www.w3.org/ns/shacl#NodeShape"/>
    <rdf:type rdf:resource="http://www.w3.org/2002/07/owl#Class"/>
    <rdfs:seeAlso rdf:resource="https://w3id.org/nen2660/term#RealizedEntity"/>
    <rdfs:subClassOf rdf:resource="https://w3id.org/nen2660/def#Entity"/>
    <rdfs:subClassOf rdf:nodeID="n29315767620c4c949118ed89a344f3a5b39"/>
    <skos:definition xml:lang="en">An entity that exists or has existed in the physical reality</skos:definition>
    <skos:prefLabel xml:lang="en">Realized entity</skos:prefLabel>
    <sh:property rdf:nodeID="n87801b7bffed4f059b3dda9335adfc9ab64"/>
  </rdf:Description>
  <rdf:Description rdf:about="https://w3id.org/nen2660/term#ChemicalCompound">
    <rdf:type rdf:resource="http://www.w3.org/2004/02/skos/core#Concept"/>
    <skos:broader rdf:resource="https://w3id.org/nen2660/term#PureSubstance"/>
    <skos:definition xml:lang="en">Pure substance consisting of two or more chemical elements that have a chemical bond with each other. In a chemical compound, the elements occur in a fixed ratio. A compound can be broken down into simpler substances by means of chemical reactions</skos:definition>
    <skos:definition xml:lang="nl">Zuivere stof bestaande uit twee of meer chemische elementen die een chemische binding met elkaar hebben. In een chemische verbinding komen de elementen in een vaste verhouding voor. Een verbinding kan worden ontleed in eenvoudigere stoffen door middel van chemische reacties</skos:definition>
    <skos:prefLabel xml:lang="en">Chemical compound</skos:prefLabel>
    <skos:prefLabel xml:lang="nl">Chemische verbinding</skos:prefLabel>
  </rdf:Description>
  <rdf:Description rdf:about="https://w3id.org/nen2660/def#hasFunctionalPart">
    <rdf:type rdf:resource="http://www.w3.org/1999/02/22-rdf-syntax-ns#Property"/>
    <rdf:type rdf:resource="http://www.w3.org/2002/07/owl#ObjectProperty"/>
    <rdfs:domain rdf:resource="https://w3id.org/nen2660/def#FunctionalEntity"/>
    <rdfs:range rdf:resource="https://w3id.org/nen2660/def#FunctionalEntity"/>
    <rdfs:seeAlso rdf:resource="https://w3id.org/nen2660/term#hasFunctionalPart"/>
    <rdfs:subPropertyOf rdf:resource="https://w3id.org/nen2660/def#hasPart"/>
    <skos:definition xml:lang="en">The hasPart relation of a functional nature</skos:definition>
    <skos:prefLabel xml:lang="en">has functional part</skos:prefLabel>
  </rdf:Description>
  <rdf:Description rdf:about="https://w3id.org/nen2660/term#State">
    <rdf:type rdf:resource="http://www.w3.org/2004/02/skos/core#Concept"/>
    <skos:broader rdf:resource="https://w3id.org/nen2660/term#ConcreteConcept"/>
    <skos:definition xml:lang="en">Temporal part of an entity during a period between two events. A state is characterized by the properties and relations of the entity</skos:definition>
    <skos:definition xml:lang="nl">Temporeel deel van een entiteit gedurende een periode tussen twee gebeurtenissen. Een toestand wordt gekenmerkt door de eigenschappen en relaties van de entiteit</skos:definition>
    <skos:prefLabel xml:lang="en">State</skos:prefLabel>
    <skos:prefLabel xml:lang="nl">Toestand</skos:prefLabel>
  </rdf:Description>
  <rdf:Description rdf:about="https://w3id.org/nen2660/term#hasFunctionalPart">
    <rdf:type rdf:resource="http://www.w3.org/2004/02/skos/core#Concept"/>
    <skos:broader rdf:resource="https://w3id.org/nen2660/term#hasPart"/>
    <skos:definition xml:lang="nl">De heeftDeel relatie van functionele aard</skos:definition>
    <skos:definition xml:lang="en">The hasPart relation of a functional nature</skos:definition>
    <skos:prefLabel xml:lang="en">has functional part</skos:prefLabel>
    <skos:prefLabel xml:lang="nl">heeft functioneel deel</skos:prefLabel>
  </rdf:Description>
  <rdf:Description rdf:about="https://w3id.org/nen2660/term#participatesIn">
    <rdf:type rdf:resource="http://www.w3.org/2004/02/skos/core#Concept"/>
    <skos:definition xml:lang="nl">De interactie waaraan een fysiek object deelneemt</skos:definition>
    <skos:definition xml:lang="en">The interaction a physical object participates in</skos:definition>
    <skos:prefLabel xml:lang="en">participates in</skos:prefLabel>
    <skos:prefLabel xml:lang="nl">participeert in</skos:prefLabel>
  </rdf:Description>
  <rdf:Description rdf:nodeID="n87801b7bffed4f059b3dda9335adfc9ab86">
    <rdf:first rdf:resource="https://w3id.org/nen2660/def#MaterialFlow"/>
    <rdf:rest rdf:nodeID="n87801b7bffed4f059b3dda9335adfc9ab87"/>
  </rdf:Description>
  <rdf:Description rdf:nodeID="n29315767620c4c949118ed89a344f3a5b35">
    <rdf:type rdf:resource="http://www.w3.org/2002/07/owl#Restriction"/>
    <owl:allValuesFrom rdf:nodeID="n29315767620c4c949118ed89a344f3a5b36"/>
    <owl:onProperty rdf:resource="https://w3id.org/nen2660/def#hasPart"/>
  </rdf:Description>
  <rdf:Description rdf:about="http://qudt.org/schema/qudt/Unit">
    <rdf:type rdf:resource="https://w3id.org/nen2660/def#EnumerationType"/>
    <rdfs:seeAlso rdf:resource="https://w3id.org/nen2660/term#Unit"/>
    <skos:definition xml:lang="en">A particular quantity value that has been chosen as a scale for measuring other quantities the same kind</skos:definition>
    <skos:prefLabel xml:lang="en">Unit</skos:prefLabel>
  </rdf:Description>
  <rdf:Description rdf:about="https://w3id.org/nen2660/def#PlannedEntity">
    <rdf:type rdf:resource="http://www.w3.org/2000/01/rdf-schema#Class"/>
    <rdf:type rdf:resource="http://www.w3.org/ns/shacl#NodeShape"/>
    <rdf:type rdf:resource="http://www.w3.org/2002/07/owl#Class"/>
    <rdfs:seeAlso rdf:resource="https://w3id.org/nen2660/term#PlannedEntity"/>
    <rdfs:subClassOf rdf:resource="https://w3id.org/nen2660/def#Entity"/>
    <rdfs:subClassOf rdf:nodeID="n29315767620c4c949118ed89a344f3a5b23"/>
    <skos:definition xml:lang="en">An entity that does not yet exist in physical reality, but which exists in mental or conceptual reality</skos:definition>
    <skos:prefLabel xml:lang="en">Planned entity</skos:prefLabel>
    <sh:property rdf:nodeID="n87801b7bffed4f059b3dda9335adfc9ab44"/>
    <sh:property rdf:nodeID="n87801b7bffed4f059b3dda9335adfc9ab45"/>
  </rdf:Description>
  <rdf:Description rdf:about="https://w3id.org/nen2660/term#isImplementedBy">
    <rdf:type rdf:resource="http://www.w3.org/2004/02/skos/core#Concept"/>
    <skos:broader rdf:resource="https://w3id.org/nen2660/term#hasSolution"/>
    <skos:definition xml:lang="nl">De technische entiteit die een functionele entiteit implementeert</skos:definition>
    <skos:definition xml:lang="en">The technical entity that implements a functional entity</skos:definition>
    <skos:prefLabel xml:lang="nl">is geimplementeerd door</skos:prefLabel>
    <skos:prefLabel xml:lang="en">is implemented by</skos:prefLabel>
  </rdf:Description>
  <rdf:Description rdf:about="https://w3id.org/nen2660/term#triggers">
    <rdf:type rdf:resource="http://www.w3.org/2004/02/skos/core#Concept"/>
    <skos:definition xml:lang="nl">De gebeurtenis getriggerd door een entiteit</skos:definition>
    <skos:definition xml:lang="en">The event triggert by an entity</skos:definition>
    <skos:prefLabel xml:lang="en">triggers</skos:prefLabel>
    <skos:prefLabel xml:lang="nl">triggert</skos:prefLabel>
  </rdf:Description>
  <rdf:Description rdf:about="https://w3id.org/nen2660/def#RealObject">
    <rdf:type rdf:resource="http://www.w3.org/2000/01/rdf-schema#Class"/>
    <rdf:type rdf:resource="http://www.w3.org/ns/shacl#NodeShape"/>
    <rdf:type rdf:resource="http://www.w3.org/2002/07/owl#Class"/>
    <rdfs:seeAlso rdf:resource="https://w3id.org/nen2660/term#RealObject"/>
    <rdfs:subClassOf rdf:resource="https://w3id.org/nen2660/def#PhysicalObject"/>
    <rdfs:subClassOf rdf:nodeID="n29315767620c4c949118ed89a344f3a5b35"/>
    <skos:definition xml:lang="en">physical object (rigid or non-rigid) that is (or can be) tangible and visible in reality, man-made or naturally occurring</skos:definition>
    <skos:prefLabel xml:lang="en">Real object</skos:prefLabel>
    <sh:property rdf:nodeID="n87801b7bffed4f059b3dda9335adfc9ab54"/>
    <sh:property rdf:nodeID="n87801b7bffed4f059b3dda9335adfc9ab59"/>
  </rdf:Description>
  <rdf:Description rdf:about="https://w3id.org/nen2660/term#RequirementSourceType">
    <rdf:type rdf:resource="http://www.w3.org/2004/02/skos/core#Concept"/>
    <skos:broader rdf:resource="https://w3id.org/nen2660/term#EnumerationType"/>
    <skos:definition xml:lang="nl">Het type bron waaruit een behoefte voortkomt zoals een klant, per definitie, aanbevolen door de sector of vereist door wet/regelgeving</skos:definition>
    <skos:definition xml:lang="en">The type of source from which a requirement comes like a client, by definition, recommended by the sector or demanded by law/regulation</skos:definition>
    <skos:prefLabel xml:lang="nl">Eis bron type</skos:prefLabel>
    <skos:prefLabel xml:lang="en">Requirement source type</skos:prefLabel>
  </rdf:Description>
  <rdf:Description rdf:nodeID="n29315767620c4c949118ed89a344f3a5b26">
    <rdf:first rdf:resource="http://www.w3.org/2001/XMLSchema#string"/>
    <rdf:rest rdf:nodeID="n29315767620c4c949118ed89a344f3a5b27"/>
  </rdf:Description>
  <rdf:Description rdf:about="https://w3id.org/nen2660/term#DiscreteObject">
    <rdf:type rdf:resource="http://www.w3.org/2004/02/skos/core#Concept"/>
    <skos:broader rdf:resource="https://w3id.org/nen2660/term#RealObject"/>
    <skos:definition xml:lang="en">A real object consisting of a contiguous amount of form-retaining matter, held together primarily by internal forces (gravity or electromagnetic force)</skos:definition>
    <skos:definition xml:lang="nl">Een reëel object dat bestaat uit een aaneengesloten hoeveelheid vormvaste materie, primair bijeengehouden door interne krachten (zwaartekracht of elektromagnetische kracht)</skos:definition>
    <skos:prefLabel xml:lang="nl">Discreet object</skos:prefLabel>
    <skos:prefLabel xml:lang="en">Discrete object</skos:prefLabel>
  </rdf:Description>
  <rdf:Description rdf:about="http://www.w3.org/2006/time#TemporalEntity">
    <rdfs:seeAlso rdf:resource="https://w3id.org/nen2660/term#TemporalEntity"/>
    <rdfs:subClassOf rdf:resource="https://w3id.org/nen2660/def#Representation"/>
    <skos:definition xml:lang="en">A temporal interval or instant</skos:definition>
    <skos:prefLabel xml:lang="en">Temporal entity</skos:prefLabel>
  </rdf:Description>
  <rdf:Description rdf:nodeID="n29315767620c4c949118ed89a344f3a5b60">
    <rdf:first rdf:resource="https://w3id.org/nen2660/def#Mixture"/>
    <rdf:rest rdf:resource="http://www.w3.org/1999/02/22-rdf-syntax-ns#nil"/>
  </rdf:Description>
  <rdf:Description rdf:nodeID="n87801b7bffed4f059b3dda9335adfc9ab14">
    <sh:path rdf:resource="https://w3id.org/nen2660/def#hasPartsGroup"/>
    <sh:class rdf:resource="http://www.w3.org/2000/01/rdf-schema#Container"/>
  </rdf:Description>
  <rdf:Description rdf:nodeID="n87801b7bffed4f059b3dda9335adfc9ab84">
    <sh:path rdf:resource="https://w3id.org/nen2660/def#hasRequirement"/>
    <sh:class rdf:resource="https://w3id.org/nen2660/def#Requirement"/>
  </rdf:Description>
  <rdf:Description rdf:about="https://w3id.org/nen2660/term#InformationFlow">
    <rdf:type rdf:resource="http://www.w3.org/2004/02/skos/core#Concept"/>
    <skos:broader rdf:resource="https://w3id.org/nen2660/term#TransferType"/>
    <skos:definition xml:lang="nl">De beweging van informatie weergegeven in een of ander medium</skos:definition>
    <skos:definition xml:lang="en">The movement of information represented in some medium</skos:definition>
    <skos:prefLabel xml:lang="nl">Informatie stroom</skos:prefLabel>
    <skos:prefLabel xml:lang="en">Information flow</skos:prefLabel>
  </rdf:Description>
  <rdf:Description rdf:about="https://w3id.org/nen2660/term#Representation">
    <rdf:type rdf:resource="http://www.w3.org/2004/02/skos/core#Concept"/>
    <skos:broader rdf:resource="https://w3id.org/nen2660/term#InformationObject"/>
    <skos:definition xml:lang="nl">Dat wat iets anders vertegenwoordigt</skos:definition>
    <skos:definition xml:lang="en">That which represents something else</skos:definition>
    <skos:prefLabel xml:lang="nl">Representatie</skos:prefLabel>
    <skos:prefLabel xml:lang="en">Representation</skos:prefLabel>
  </rdf:Description>
  <rdf:Description rdf:about="https://w3id.org/nen2660/def#hasQuantityKind">
    <rdf:type rdf:resource="http://www.w3.org/1999/02/22-rdf-syntax-ns#Property"/>
    <rdf:type rdf:resource="http://www.w3.org/2002/07/owl#ObjectProperty"/>
    <rdfs:range rdf:resource="http://qudt.org/schema/qudt/QuantityKind"/>
    <rdfs:seeAlso rdf:resource="https://w3id.org/nen2660/term#hasQuantityKind"/>
    <skos:definition xml:lang="en">The possession of a quantity kind</skos:definition>
    <skos:prefLabel xml:lang="en">has quantity kind</skos:prefLabel>
  </rdf:Description>
  <rdf:Description rdf:about="https://w3id.org/nen2660/term#Objectification">
    <rdf:type rdf:resource="http://www.w3.org/2004/02/skos/core#Concept"/>
    <skos:broader rdf:resource="https://w3id.org/nen2660/term#AbstractConcept"/>
    <skos:definition xml:lang="en">An attribute (quality or quantity) or relation represented as an individual defined by a concept</skos:definition>
    <skos:definition xml:lang="nl">Een attribuut (kwaliteit of kwantiteit) of relatie voorgesteld als een individu gedefinieerd door een concept</skos:definition>
    <skos:prefLabel xml:lang="nl">Objectificatie</skos:prefLabel>
    <skos:prefLabel xml:lang="en">Objectification</skos:prefLabel>
  </rdf:Description>
  <rdf:Description rdf:nodeID="n87801b7bffed4f059b3dda9335adfc9ab37">
    <rdf:first rdf:nodeID="n87801b7bffed4f059b3dda9335adfc9ab35"/>
    <rdf:rest rdf:resource="http://www.w3.org/1999/02/22-rdf-syntax-ns#nil"/>
  </rdf:Description>
  <rdf:Description rdf:about="https://w3id.org/nen2660/def#Objectification">
    <rdf:type rdf:resource="http://www.w3.org/2000/01/rdf-schema#Class"/>
    <rdf:type rdf:resource="http://www.w3.org/ns/shacl#NodeShape"/>
    <rdf:type rdf:resource="http://www.w3.org/2002/07/owl#Class"/>
    <rdfs:seeAlso rdf:resource="https://w3id.org/nen2660/term#Objectification"/>
    <rdfs:subClassOf rdf:resource="https://w3id.org/nen2660/def#AbstractConcept"/>
    <rdfs:subClassOf rdf:nodeID="n29315767620c4c949118ed89a344f3a5b22"/>
    <skos:definition xml:lang="en">An attribute (quality or quantity) or relation represented as an individual defined by a concept</skos:definition>
    <skos:prefLabel xml:lang="en">Objectification</skos:prefLabel>
    <sh:property rdf:nodeID="n87801b7bffed4f059b3dda9335adfc9ab39"/>
  </rdf:Description>
  <rdf:Description rdf:about="https://w3id.org/nen2660/term#begins">
    <rdf:type rdf:resource="http://www.w3.org/2004/02/skos/core#Concept"/>
    <skos:definition xml:lang="nl">De toestand die gestart wordt door een gebeurtenis</skos:definition>
    <skos:definition xml:lang="en">The state that is started by an event</skos:definition>
    <skos:prefLabel xml:lang="en">begins</skos:prefLabel>
    <skos:prefLabel xml:lang="nl">begint</skos:prefLabel>
  </rdf:Description>
  <rdf:Description rdf:nodeID="n87801b7bffed4f059b3dda9335adfc9ab97">
    <rdf:first rdf:resource="https://w3id.org/nen2660/def#State"/>
    <rdf:rest rdf:nodeID="n87801b7bffed4f059b3dda9335adfc9ab98"/>
  </rdf:Description>
  <rdf:Description rdf:about="https://w3id.org/nen2660/def#RelationReference">
    <rdf:type rdf:resource="http://www.w3.org/2000/01/rdf-schema#Class"/>
    <rdf:type rdf:resource="http://www.w3.org/ns/shacl#NodeShape"/>
    <rdf:type rdf:resource="http://www.w3.org/2002/07/owl#Class"/>
    <rdfs:seeAlso rdf:resource="https://w3id.org/nen2660/term#RelationReference"/>
    <rdfs:subClassOf rdf:resource="https://w3id.org/nen2660/def#Objectification"/>
    <rdfs:subClassOf rdf:nodeID="n29315767620c4c949118ed89a344f3a5b40"/>
    <skos:definition xml:lang="en">The objectification of a reference for a relation having a complex value like a simple reference sec combined with other metadata or just a combination of simple references (n-ary relation)</skos:definition>
    <skos:prefLabel xml:lang="en">Relation reference</skos:prefLabel>
    <sh:property rdf:nodeID="n87801b7bffed4f059b3dda9335adfc9ab65"/>
  </rdf:Description>
  <rdf:Description rdf:about="https://w3id.org/nen2660/def#participatesIn">
    <rdf:type rdf:resource="http://www.w3.org/1999/02/22-rdf-syntax-ns#Property"/>
    <rdf:type rdf:resource="http://www.w3.org/2002/07/owl#ObjectProperty"/>
    <rdfs:domain rdf:resource="https://w3id.org/nen2660/def#PhysicalObject"/>
    <rdfs:range rdf:resource="https://w3id.org/nen2660/def#Interaction"/>
    <rdfs:seeAlso rdf:resource="https://w3id.org/nen2660/term#participatesIn"/>
    <skos:definition xml:lang="en">The interaction a physical object participates in</skos:definition>
    <skos:prefLabel xml:lang="en">participates in</skos:prefLabel>
  </rdf:Description>
  <rdf:Description rdf:about="https://w3id.org/nen2660/term#Type">
    <rdf:type rdf:resource="http://www.w3.org/2004/02/skos/core#Concept"/>
    <skos:broader rdf:resource="https://w3id.org/nen2660/term#AbstractConcept"/>
    <skos:definition xml:lang="en">A meta-concept which instances are concepts (not individuals)</skos:definition>
    <skos:definition xml:lang="nl">Een meta-concept waarvan instanties concepten zijn (geen individuen)</skos:definition>
    <skos:prefLabel xml:lang="en">Type</skos:prefLabel>
    <skos:prefLabel xml:lang="nl">Type</skos:prefLabel>
  </rdf:Description>
  <rdf:Description rdf:about="https://w3id.org/nen2660/term#ends">
    <rdf:type rdf:resource="http://www.w3.org/2004/02/skos/core#Concept"/>
    <skos:definition xml:lang="nl">De toestand die wordt beëindigd door een gebeurtenis</skos:definition>
    <skos:definition xml:lang="en">The state that is ended by an event</skos:definition>
    <skos:prefLabel xml:lang="nl">beeindigt</skos:prefLabel>
    <skos:prefLabel xml:lang="en">ends</skos:prefLabel>
  </rdf:Description>
  <rdf:Description rdf:about="https://w3id.org/nen2660/def#Interaction">
    <rdf:type rdf:resource="http://www.w3.org/2000/01/rdf-schema#Class"/>
    <rdf:type rdf:resource="http://www.w3.org/ns/shacl#NodeShape"/>
    <rdf:type rdf:resource="http://www.w3.org/2002/07/owl#Class"/>
    <rdfs:seeAlso rdf:resource="https://w3id.org/nen2660/term#Interaction"/>
    <rdfs:subClassOf rdf:resource="https://w3id.org/nen2660/def#Activity"/>
    <skos:definition xml:lang="en">The activity being a combination of sub-activities performed by physical objects between which a transfer of matter, information, energy or force takes place, typically over a connection or interface (directly or through ports)</skos:definition>
    <skos:prefLabel xml:lang="en">Interaction</skos:prefLabel>
    <sh:property rdf:nodeID="n87801b7bffed4f059b3dda9335adfc9ab25"/>
    <sh:property rdf:nodeID="n87801b7bffed4f059b3dda9335adfc9ab26"/>
    <sh:property rdf:nodeID="n87801b7bffed4f059b3dda9335adfc9ab27"/>
  </rdf:Description>
  <rdf:Description rdf:about="https://w3id.org/nen2660/def#ConcreteConcept">
    <rdf:type rdf:resource="http://www.w3.org/2000/01/rdf-schema#Class"/>
    <rdf:type rdf:resource="http://www.w3.org/ns/shacl#NodeShape"/>
    <rdf:type rdf:resource="http://www.w3.org/2002/07/owl#Class"/>
    <rdfs:seeAlso rdf:resource="https://w3id.org/nen2660/term#ConcreteConcept"/>
    <rdfs:subClassOf rdf:resource="https://w3id.org/nen2660/def#TopConcept"/>
    <skos:definition xml:lang="en">Concept that forms a manifestation and a demarcation in a concrete space-time. A concrete concept has a life cycle</skos:definition>
    <skos:prefLabel xml:lang="en">Concrete concept</skos:prefLabel>
    <sh:property rdf:nodeID="n87801b7bffed4f059b3dda9335adfc9ab10"/>
    <sh:property rdf:nodeID="n87801b7bffed4f059b3dda9335adfc9ab11"/>
    <sh:property rdf:nodeID="n87801b7bffed4f059b3dda9335adfc9ab12"/>
    <sh:property rdf:nodeID="n87801b7bffed4f059b3dda9335adfc9ab13"/>
    <sh:property rdf:nodeID="n87801b7bffed4f059b3dda9335adfc9ab14"/>
  </rdf:Description>
  <rdf:Description rdf:about="https://w3id.org/nen2660/def#HeterogeneousMixture">
    <rdf:type rdf:resource="http://www.w3.org/2000/01/rdf-schema#Class"/>
    <rdf:type rdf:resource="http://www.w3.org/2002/07/owl#Class"/>
    <rdfs:seeAlso rdf:resource="https://w3id.org/nen2660/term#HeterogeneousMixture"/>
    <rdfs:subClassOf rdf:resource="https://w3id.org/nen2660/def#Mixture"/>
    <skos:definition xml:lang="en">A mixture that is separated into different regions or phases that have different compositions or properties</skos:definition>
    <skos:prefLabel xml:lang="en">Heterogeneous mixture</skos:prefLabel>
  </rdf:Description>
  <rdf:Description rdf:about="https://w3id.org/nen2660/def#hasUnitShape">
    <rdf:type rdf:resource="http://www.w3.org/ns/shacl#NodeShape"/>
    <sh:class rdf:resource="http://qudt.org/schema/qudt/Unit"/>
    <sh:targetObjectsOf rdf:resource="https://w3id.org/nen2660/def#hasUnit"/>
  </rdf:Description>
  <rdf:Description rdf:about="https://w3id.org/nen2660/def#requirementSeverityType">
    <rdf:type rdf:resource="http://www.w3.org/1999/02/22-rdf-syntax-ns#Property"/>
    <rdf:type rdf:resource="http://www.w3.org/2002/07/owl#ObjectProperty"/>
    <rdfs:domain rdf:resource="https://w3id.org/nen2660/def#Requirement"/>
    <rdfs:range rdf:resource="https://w3id.org/nen2660/def#RequirementSeverityType"/>
    <rdfs:seeAlso rdf:resource="https://w3id.org/nen2660/term#requirementSeverityType"/>
    <skos:definition xml:lang="en">The possession of a severity type by a requirement</skos:definition>
    <skos:prefLabel xml:lang="en">requirement severity type</skos:prefLabel>
  </rdf:Description>
  <rdf:Description rdf:about="https://w3id.org/nen2660/term#Plasma">
    <rdf:type rdf:resource="http://www.w3.org/2004/02/skos/core#Concept"/>
    <skos:broader rdf:resource="https://w3id.org/nen2660/term#AggregationStateType"/>
    <skos:definition xml:lang="en">A phase in which the particles of a gaseous substance are ionised</skos:definition>
    <skos:definition xml:lang="nl">Een fase waarin de deeltjes van een gasvormige stof geïoniseerd zijn</skos:definition>
    <skos:prefLabel xml:lang="en">Plasma</skos:prefLabel>
    <skos:prefLabel xml:lang="nl">Plasma</skos:prefLabel>
  </rdf:Description>
  <rdf:Description rdf:about="https://w3id.org/nen2660/term#requirementSourceType">
    <rdf:type rdf:resource="http://www.w3.org/2004/02/skos/core#Concept"/>
    <skos:definition xml:lang="nl">Het hebben van een brontype door een eis</skos:definition>
    <skos:definition xml:lang="en">The possession of a source type by a requirement</skos:definition>
    <skos:prefLabel xml:lang="nl">eis bron type</skos:prefLabel>
    <skos:prefLabel xml:lang="en">requirement source type</skos:prefLabel>
  </rdf:Description>
  <rdf:Description rdf:about="https://w3id.org/nen2660/term#isPlanFor">
    <rdf:type rdf:resource="http://www.w3.org/2004/02/skos/core#Concept"/>
    <skos:definition xml:lang="en">A potentially realized entity according to this planned entity</skos:definition>
    <skos:definition xml:lang="nl">Een potentieel gerealiseerde entiteit volgens deze geplande entiteit</skos:definition>
    <skos:prefLabel xml:lang="en">is plan for</skos:prefLabel>
    <skos:prefLabel xml:lang="nl">is plan voor</skos:prefLabel>
  </rdf:Description>
  <rdf:Description rdf:nodeID="n29315767620c4c949118ed89a344f3a5b42">
    <rdf:type rdf:resource="http://www.w3.org/2002/07/owl#Restriction"/>
    <owl:allValuesFrom rdf:nodeID="n29315767620c4c949118ed89a344f3a5b43"/>
    <owl:onProperty rdf:resource="https://w3id.org/nen2660/def#hasPart"/>
  </rdf:Description>
  <rdf:Description rdf:about="https://w3id.org/nen2660/term#hasRequirement">
    <rdf:type rdf:resource="http://www.w3.org/2004/02/skos/core#Concept"/>
    <skos:definition xml:lang="nl">De (ongestructureerde) eis aan iets</skos:definition>
    <skos:definition xml:lang="en">The (unstructured) requirement for something</skos:definition>
    <skos:prefLabel xml:lang="en">has requirement</skos:prefLabel>
    <skos:prefLabel xml:lang="nl">heeft eis</skos:prefLabel>
  </rdf:Description>
  <rdf:Description rdf:about="https://w3id.org/nen2660/term#RelationReference">
    <rdf:type rdf:resource="http://www.w3.org/2004/02/skos/core#Concept"/>
    <skos:broader rdf:resource="https://w3id.org/nen2660/term#Objectification"/>
    <skos:definition xml:lang="nl">De objectivering van een referentie voor een relatie met een complexe waarde zoals een simpele referentie sec gecombineerd met andere metadata of alleen een combinatie van simpele referenties (n-ary relaties)</skos:definition>
    <skos:definition xml:lang="en">The objectification of a reference for a relation having a complex value like a simple reference sec combined with other metadata or just a combination of simple references (n-ary relation)</skos:definition>
    <skos:prefLabel xml:lang="nl">Relatie referentie</skos:prefLabel>
    <skos:prefLabel xml:lang="en">Relation reference</skos:prefLabel>
  </rdf:Description>
  <rdf:Description rdf:about="https://w3id.org/nen2660/def#requirementSourceType">
    <rdf:type rdf:resource="http://www.w3.org/1999/02/22-rdf-syntax-ns#Property"/>
    <rdf:type rdf:resource="http://www.w3.org/2002/07/owl#ObjectProperty"/>
    <rdfs:domain rdf:resource="https://w3id.org/nen2660/def#Requirement"/>
    <rdfs:range rdf:resource="https://w3id.org/nen2660/def#RequirementSourceType"/>
    <rdfs:seeAlso rdf:resource="https://w3id.org/nen2660/term#requirementSourceType"/>
    <skos:definition xml:lang="en">The possession of a source type by a requirement</skos:definition>
    <skos:prefLabel xml:lang="en">requirement source type</skos:prefLabel>
  </rdf:Description>
  <rdf:Description rdf:about="https://w3id.org/nen2660/term#Activity">
    <rdf:type rdf:resource="http://www.w3.org/2004/02/skos/core#Concept"/>
    <skos:broader rdf:resource="https://w3id.org/nen2660/term#Entity"/>
    <skos:definition xml:lang="nl">Entiteit die plaatsvindt of kan plaatsvinden in een concrete ruimte-tijd. Een activiteit transformeert objecten, en wordt uitgevoerd door een object</skos:definition>
    <skos:definition xml:lang="en">Entity that takes place or can take place in a concrete space-time. An activity transforms objects, and is executed by an object</skos:definition>
    <skos:prefLabel xml:lang="en">Activity</skos:prefLabel>
    <skos:prefLabel xml:lang="nl">Activiteit</skos:prefLabel>
  </rdf:Description>
  <rdf:Description rdf:nodeID="n29315767620c4c949118ed89a344f3a5b23">
    <rdf:type rdf:resource="http://www.w3.org/2002/07/owl#Restriction"/>
    <owl:allValuesFrom rdf:resource="https://w3id.org/nen2660/def#PlannedEntity"/>
    <owl:onProperty rdf:resource="https://w3id.org/nen2660/def#hasPart"/>
  </rdf:Description>
  <rdf:Description rdf:about="https://w3id.org/nen2660/def#Interface">
    <rdf:type rdf:resource="http://www.w3.org/2000/01/rdf-schema#Class"/>
    <rdf:type rdf:resource="http://www.w3.org/ns/shacl#NodeShape"/>
    <rdf:type rdf:resource="http://www.w3.org/2002/07/owl#Class"/>
    <rdfs:seeAlso rdf:resource="https://w3id.org/nen2660/term#Interface"/>
    <rdfs:subClassOf rdf:resource="https://w3id.org/nen2660/def#SpatialRegion"/>
    <skos:definition xml:lang="en">A spatial object, typically a thin 2D physical space (but also 0D or 1D) that connects two physical objects or ports of physical objects through which a static or dynamic interaction or interaction between those elements can take place</skos:definition>
    <skos:prefLabel xml:lang="en">Interface</skos:prefLabel>
    <sh:property rdf:nodeID="n87801b7bffed4f059b3dda9335adfc9ab28"/>
    <sh:property rdf:nodeID="n87801b7bffed4f059b3dda9335adfc9ab29"/>
  </rdf:Description>
  <rdf:Description rdf:about="https://w3id.org/nen2660/term#QuantityKind">
    <rdf:type rdf:resource="http://www.w3.org/2004/02/skos/core#Concept"/>
    <skos:definition xml:lang="en">Any observable property that can be measured and quantified numerically</skos:definition>
    <skos:definition xml:lang="nl">Elke waarneembare eigenschap die numeriek kan worden gemeten en gekwantificeerd</skos:definition>
    <skos:prefLabel xml:lang="nl">Kwantiteitsoort</skos:prefLabel>
    <skos:prefLabel xml:lang="en">Quantity kind</skos:prefLabel>
  </rdf:Description>
  <rdf:Description rdf:nodeID="n87801b7bffed4f059b3dda9335adfc9ab24">
    <sh:path rdf:resource="https://w3id.org/nen2660/def#hasSolution"/>
    <sh:class rdf:resource="https://w3id.org/nen2660/def#TechnicalEntity"/>
  </rdf:Description>
  <rdf:Description rdf:nodeID="n29315767620c4c949118ed89a344f3a5b15">
    <rdf:first rdf:resource="https://w3id.org/nen2660/def#PlannedEntity"/>
    <rdf:rest rdf:nodeID="n29315767620c4c949118ed89a344f3a5b16"/>
  </rdf:Description>
  <rdf:Description rdf:about="https://w3id.org/nen2660/def#Liquid">
    <rdf:type rdf:resource="https://w3id.org/nen2660/def#AggregationStateType"/>
    <rdfs:seeAlso rdf:resource="https://w3id.org/nen2660/term#Liquid"/>
    <skos:definition xml:lang="en">A liquid is a nearly incompressible fluid that conforms to the shape of its container but retains a (nearly) constant volume independent of pressure</skos:definition>
    <skos:prefLabel xml:lang="en">Liquid</skos:prefLabel>
  </rdf:Description>
  <rdf:Description rdf:about="https://w3id.org/nen2660/rdfs/def">
    <rdf:type rdf:resource="http://www.w3.org/2002/07/owl#Ontology"/>
    <owl:imports rdf:resource="http://qudt.org/2.1/schema/qudt"/>
    <owl:imports rdf:resource="http://qudt.org/2.1/vocab/quantitykind"/>
    <owl:imports rdf:resource="http://qudt.org/2.1/vocab/unit"/>
    <owl:imports rdf:resource="http://www.w3.org/2004/02/skos/core"/>
    <owl:imports rdf:resource="http://www.w3.org/2006/time"/>
    <owl:imports rdf:resource="http://www.w3.org/ns/shacl"/>
    <owl:imports rdf:resource="https://w3id.org/nen2660/skos/term"/>
  </rdf:Description>
  <rdf:Description rdf:about="https://w3id.org/nen2660/def#ends">
    <rdf:type rdf:resource="http://www.w3.org/1999/02/22-rdf-syntax-ns#Property"/>
    <rdf:type rdf:resource="http://www.w3.org/2002/07/owl#ObjectProperty"/>
    <rdfs:domain rdf:resource="https://w3id.org/nen2660/def#Event"/>
    <rdfs:range rdf:resource="https://w3id.org/nen2660/def#State"/>
    <rdfs:seeAlso rdf:resource="https://w3id.org/nen2660/term#ends"/>
    <skos:definition xml:lang="en">The state that is ended by an event</skos:definition>
    <skos:prefLabel xml:lang="en">ends</skos:prefLabel>
  </rdf:Description>
  <rdf:Description rdf:nodeID="n87801b7bffed4f059b3dda9335adfc9ab82">
    <sh:path rdf:resource="https://w3id.org/nen2660/def#hasTechnicalPart"/>
    <sh:class rdf:resource="https://w3id.org/nen2660/def#TechnicalEntity"/>
  </rdf:Description>
  <rdf:Description rdf:nodeID="n87801b7bffed4f059b3dda9335adfc9ab15">
    <sh:path rdf:resource="https://w3id.org/nen2660/def#connectsObject"/>
    <sh:class rdf:resource="https://w3id.org/nen2660/def#PhysicalObject"/>
  </rdf:Description>
  <rdf:Description rdf:nodeID="n29315767620c4c949118ed89a344f3a5b30">
    <rdf:type rdf:resource="http://www.w3.org/2002/07/owl#Class"/>
    <owl:unionOf rdf:nodeID="n29315767620c4c949118ed89a344f3a5b31"/>
  </rdf:Description>
  <rdf:Description rdf:about="https://w3id.org/nen2660/def#State">
    <rdf:type rdf:resource="http://www.w3.org/2000/01/rdf-schema#Class"/>
    <rdf:type rdf:resource="http://www.w3.org/ns/shacl#NodeShape"/>
    <rdf:type rdf:resource="http://www.w3.org/2002/07/owl#Class"/>
    <rdfs:seeAlso rdf:resource="https://w3id.org/nen2660/term#State"/>
    <rdfs:subClassOf rdf:resource="https://w3id.org/nen2660/def#ConcreteConcept"/>
    <rdfs:subClassOf rdf:nodeID="n29315767620c4c949118ed89a344f3a5b46"/>
    <skos:definition xml:lang="en">Temporal part of an entity during a period between two events. A state is characterized by the properties and relations of the entity</skos:definition>
    <skos:prefLabel xml:lang="en">State</skos:prefLabel>
    <sh:property rdf:nodeID="n87801b7bffed4f059b3dda9335adfc9ab77"/>
    <sh:property rdf:nodeID="n87801b7bffed4f059b3dda9335adfc9ab78"/>
    <sh:property rdf:nodeID="n87801b7bffed4f059b3dda9335adfc9ab79"/>
    <sh:property rdf:nodeID="n87801b7bffed4f059b3dda9335adfc9ab80"/>
  </rdf:Description>
  <rdf:Description rdf:about="https://w3id.org/nen2660/term#hasTemporalEntity">
    <rdf:type rdf:resource="http://www.w3.org/2004/02/skos/core#Concept"/>
    <skos:definition xml:lang="nl">De abstracte temporele entiteit die een concreet concept in de tijd vertegenwoordigt</skos:definition>
    <skos:definition xml:lang="en">The abstract temporal entity representing a concrete concept in time</skos:definition>
    <skos:prefLabel xml:lang="en">has temporal entity</skos:prefLabel>
    <skos:prefLabel xml:lang="nl">heeft temporele entiteit</skos:prefLabel>
  </rdf:Description>
  <rdf:Description rdf:about="https://w3id.org/nen2660/term#ConceptType">
    <rdf:type rdf:resource="http://www.w3.org/2004/02/skos/core#Concept"/>
    <skos:broader rdf:resource="https://w3id.org/nen2660/term#Type"/>
    <skos:definition xml:lang="en">A meta-concept having concepts as instances that can have attributes or relations</skos:definition>
    <skos:definition xml:lang="nl">Een meta-concept met concepten als instanties die attributen of relaties kunnen hebben</skos:definition>
    <skos:prefLabel xml:lang="en">Concept type</skos:prefLabel>
    <skos:prefLabel xml:lang="nl">Concept type</skos:prefLabel>
  </rdf:Description>
  <rdf:Description rdf:about="https://w3id.org/nen2660/def#RequirementTopicType">
    <rdf:type rdf:resource="http://www.w3.org/2000/01/rdf-schema#Class"/>
    <rdf:type rdf:resource="https://w3id.org/nen2660/def#EnumerationType"/>
    <rdf:type rdf:resource="http://www.w3.org/2002/07/owl#Class"/>
    <rdfs:seeAlso rdf:resource="https://w3id.org/nen2660/term#RequirementTopicType"/>
    <skos:definition xml:lang="en">The entity aspect a requirement applies to</skos:definition>
    <skos:prefLabel xml:lang="en">Requirement topic type</skos:prefLabel>
  </rdf:Description>
  <rdf:Description rdf:nodeID="n87801b7bffed4f059b3dda9335adfc9ab99">
    <rdf:first rdf:resource="https://w3id.org/nen2660/def#Activity"/>
    <rdf:rest rdf:resource="http://www.w3.org/1999/02/22-rdf-syntax-ns#nil"/>
  </rdf:Description>
  <rdf:Description rdf:about="https://w3id.org/nen2660/term#connectsObject">
    <rdf:type rdf:resource="http://www.w3.org/2004/02/skos/core#Concept"/>
    <skos:definition xml:lang="nl">De fysieke objecten verbonden door een verbinding of raakvlak</skos:definition>
    <skos:definition xml:lang="en">The physical objects connected by a connection or interface</skos:definition>
    <skos:prefLabel xml:lang="en">connects object</skos:prefLabel>
    <skos:prefLabel xml:lang="nl">verbindt object</skos:prefLabel>
  </rdf:Description>
  <rdf:Description rdf:nodeID="n29315767620c4c949118ed89a344f3a5b43">
    <rdf:type rdf:resource="http://www.w3.org/2002/07/owl#Class"/>
    <owl:unionOf rdf:nodeID="n29315767620c4c949118ed89a344f3a5b44"/>
  </rdf:Description>
  <rdf:Description rdf:about="https://w3id.org/nen2660/def#Plasma">
    <rdf:type rdf:resource="https://w3id.org/nen2660/def#AggregationStateType"/>
    <rdfs:seeAlso rdf:resource="https://w3id.org/nen2660/term#Plasma"/>
    <skos:definition xml:lang="en">A phase in which the particles of a gaseous substance are ionised</skos:definition>
    <skos:prefLabel xml:lang="en">Plasma</skos:prefLabel>
  </rdf:Description>
  <rdf:Description rdf:nodeID="n87801b7bffed4f059b3dda9335adfc9ab43">
    <sh:path rdf:resource="https://w3id.org/nen2660/def#executes"/>
    <sh:class rdf:resource="https://w3id.org/nen2660/def#Activity"/>
  </rdf:Description>
  <rdf:Description rdf:about="https://w3id.org/nen2660/def#Gas">
    <rdf:type rdf:resource="https://w3id.org/nen2660/def#AggregationStateType"/>
    <rdfs:seeAlso rdf:resource="https://w3id.org/nen2660/term#Gas"/>
    <skos:definition xml:lang="en">Matter in an intermediate state between liquid and plasma that can be contained only if it is fully surrounded by a solid (or in a bubble of liquid) (or held together by gravitational pull); it can condense into a liquid, or can (rarely) become a solid directly by deposition</skos:definition>
    <skos:prefLabel xml:lang="en">Gas</skos:prefLabel>
  </rdf:Description>
  <rdf:Description rdf:about="https://w3id.org/nen2660/term#PlannedEntity">
    <rdf:type rdf:resource="http://www.w3.org/2004/02/skos/core#Concept"/>
    <skos:broader rdf:resource="https://w3id.org/nen2660/term#Entity"/>
    <skos:definition xml:lang="en">An entity that does not yet exist in physical reality, but which exists in mental or conceptual reality</skos:definition>
    <skos:definition xml:lang="nl">Een entiteit die nog niet bestaat in de fysieke werkelijkheid, maar die in de mentale of conceptuele werkelijkheid voorkomt</skos:definition>
    <skos:prefLabel xml:lang="nl">Geplande entiteit</skos:prefLabel>
    <skos:prefLabel xml:lang="en">Planned entity</skos:prefLabel>
  </rdf:Description>
  <rdf:Description rdf:about="https://w3id.org/nen2660/term#Connection">
    <rdf:type rdf:resource="http://www.w3.org/2004/02/skos/core#Concept"/>
    <skos:broader rdf:resource="https://w3id.org/nen2660/term#PhysicalObject"/>
    <skos:definition xml:lang="en">A physical object (real object or spatial area) that connects two other physical objects and over which interaction takes place, namely the transfer of matter, energy, information or forces</skos:definition>
    <skos:definition xml:lang="nl">Een fysiek object (reëel object of ruimtelijk gebied) dat twee andere fysieke objecten verbindt en waarover interactie plaatsvindt namelijk de overdracht van materie, energie, informatie of krachten</skos:definition>
    <skos:prefLabel xml:lang="en">Connection</skos:prefLabel>
    <skos:prefLabel xml:lang="nl">Verbinding</skos:prefLabel>
  </rdf:Description>
  <rdf:Description rdf:about="https://w3id.org/nen2660/def#hasRequirement">
    <rdf:type rdf:resource="http://www.w3.org/1999/02/22-rdf-syntax-ns#Property"/>
    <rdf:type rdf:resource="http://www.w3.org/2002/07/owl#ObjectProperty"/>
    <rdfs:domain rdf:resource="https://w3id.org/nen2660/def#TopConcept"/>
    <rdfs:range rdf:resource="https://w3id.org/nen2660/def#Requirement"/>
    <rdfs:seeAlso rdf:resource="https://w3id.org/nen2660/term#hasRequirement"/>
    <skos:definition xml:lang="en">The (unstructured) requirement for something</skos:definition>
    <skos:prefLabel xml:lang="en">has requirement</skos:prefLabel>
  </rdf:Description>
  <rdf:Description rdf:nodeID="n29315767620c4c949118ed89a344f3a5b11">
    <rdf:first rdf:resource="https://w3id.org/nen2660/def#RealObject"/>
    <rdf:rest rdf:nodeID="n29315767620c4c949118ed89a344f3a5b12"/>
  </rdf:Description>
  <rdf:Description rdf:about="https://w3id.org/nen2660/term#HomogeneousMixture">
    <rdf:type rdf:resource="http://www.w3.org/2004/02/skos/core#Concept"/>
    <skos:broader rdf:resource="https://w3id.org/nen2660/term#Mixture"/>
    <skos:definition xml:lang="en">A mixture that is uniform throughout, and has only one phase</skos:definition>
    <skos:definition xml:lang="nl">Een mengsel dat overal uniform is en maar 1 fase heeft</skos:definition>
    <skos:prefLabel xml:lang="nl">Homogeen mengsel</skos:prefLabel>
    <skos:prefLabel xml:lang="en">Homogeneous mixture</skos:prefLabel>
  </rdf:Description>
  <rdf:Description rdf:nodeID="n87801b7bffed4f059b3dda9335adfc9ab116">
    <rdf:first rdf:resource="http://www.w3.org/1999/02/22-rdf-syntax-ns#type"/>
    <rdf:rest rdf:nodeID="n87801b7bffed4f059b3dda9335adfc9ab117"/>
  </rdf:Description>
  <rdf:Description rdf:about="https://w3id.org/nen2660/term#AbstractConcept">
    <rdf:type rdf:resource="http://www.w3.org/2004/02/skos/core#Concept"/>
    <skos:broader rdf:resource="https://w3id.org/nen2660/term#TopConcept"/>
    <skos:definition xml:lang="nl">Concept dat een manifestatie en een afbakening vormt in een abstracte ruimte. Een abstract concept heeft geen levenscyclus</skos:definition>
    <skos:definition xml:lang="en">Concept that forms a manifestation and demarcation in an abstract space. An abstract concept has no life cycle</skos:definition>
    <skos:prefLabel xml:lang="en">Abstract concept</skos:prefLabel>
    <skos:prefLabel xml:lang="nl">Abstract concept</skos:prefLabel>
  </rdf:Description>
  <rdf:Description rdf:nodeID="n29315767620c4c949118ed89a344f3a5b55">
    <rdf:type rdf:resource="http://www.w3.org/2002/07/owl#Class"/>
    <owl:unionOf rdf:nodeID="n29315767620c4c949118ed89a344f3a5b56"/>
  </rdf:Description>
  <rdf:Description rdf:about="https://w3id.org/nen2660/term#hasSolution">
    <rdf:type rdf:resource="http://www.w3.org/2004/02/skos/core#Concept"/>
    <skos:definition xml:lang="en">A technical entity that is a potential solution for a functional entity</skos:definition>
    <skos:definition xml:lang="nl">Een technische entiteit die een mogelijke oplossing is voor een functionele entiteit</skos:definition>
    <skos:prefLabel xml:lang="en">has solution</skos:prefLabel>
    <skos:prefLabel xml:lang="nl">heeft oplossing</skos:prefLabel>
  </rdf:Description>
  <rdf:Description rdf:about="https://w3id.org/nen2660/def#Force">
    <rdf:type rdf:resource="https://w3id.org/nen2660/def#TransferType"/>
    <rdfs:seeAlso rdf:resource="https://w3id.org/nen2660/term#Force"/>
    <skos:definition xml:lang="en">Physical quantity which, when exerted on a body, causes tension or pressure to arise therein, or which causes the body to change motion, accelerate</skos:definition>
    <skos:prefLabel xml:lang="en">Force</skos:prefLabel>
  </rdf:Description>
  <rdf:Description rdf:about="https://w3id.org/nen2660/def#GeometricEntity">
    <rdf:type rdf:resource="http://www.w3.org/2000/01/rdf-schema#Class"/>
    <rdf:type rdf:resource="http://www.w3.org/2002/07/owl#Class"/>
    <rdfs:seeAlso rdf:resource="https://w3id.org/nen2660/term#GeometricEntity"/>
    <rdfs:subClassOf rdf:resource="https://w3id.org/nen2660/def#Representation"/>
    <skos:definition xml:lang="en">Named concept, which forms an actual or virtual demarcation in a concrete (physical, three-dimensional) space, which we experience in reality</skos:definition>
    <skos:prefLabel xml:lang="en">Geometric entity</skos:prefLabel>
  </rdf:Description>
  <rdf:Description rdf:nodeID="n87801b7bffed4f059b3dda9335adfc9ab95">
    <rdf:first rdf:resource="https://w3id.org/nen2660/def#PhysicalObject"/>
    <rdf:rest rdf:nodeID="n87801b7bffed4f059b3dda9335adfc9ab96"/>
  </rdf:Description>
  <rdf:Description rdf:nodeID="n87801b7bffed4f059b3dda9335adfc9ab58">
    <rdf:first rdf:nodeID="n87801b7bffed4f059b3dda9335adfc9ab56"/>
    <rdf:rest rdf:resource="http://www.w3.org/1999/02/22-rdf-syntax-ns#nil"/>
  </rdf:Description>
  <rdf:Description rdf:nodeID="n87801b7bffed4f059b3dda9335adfc9ab71">
    <sh:path rdf:resource="https://w3id.org/nen2660/def#hasPart"/>
    <sh:or rdf:nodeID="n87801b7bffed4f059b3dda9335adfc9ab74"/>
  </rdf:Description>
  <rdf:Description rdf:nodeID="n29315767620c4c949118ed89a344f3a5b12">
    <rdf:first rdf:resource="https://w3id.org/nen2660/def#SpatialRegion"/>
    <rdf:rest rdf:resource="http://www.w3.org/1999/02/22-rdf-syntax-ns#nil"/>
  </rdf:Description>
  <rdf:Description rdf:about="https://w3id.org/nen2660/def#RequirementSeverityType">
    <rdf:type rdf:resource="http://www.w3.org/2000/01/rdf-schema#Class"/>
    <rdf:type rdf:resource="https://w3id.org/nen2660/def#EnumerationType"/>
    <rdf:type rdf:resource="http://www.w3.org/2002/07/owl#Class"/>
    <rdfs:seeAlso rdf:resource="https://w3id.org/nen2660/term#RequirementSeverityType"/>
    <skos:definition xml:lang="en">The seriousness of a requirement like demanded or wished</skos:definition>
    <skos:prefLabel xml:lang="en">Requirement severity type</skos:prefLabel>
  </rdf:Description>
  <rdf:Description rdf:about="https://w3id.org/nen2660/def#chemicalFormula">
    <rdf:type rdf:resource="http://www.w3.org/1999/02/22-rdf-syntax-ns#Property"/>
    <rdf:type rdf:resource="http://www.w3.org/2002/07/owl#DatatypeProperty"/>
    <rdfs:domain rdf:resource="https://w3id.org/nen2660/def#Matter"/>
    <rdfs:range rdf:resource="http://www.w3.org/2001/XMLSchema#string"/>
    <rdfs:seeAlso rdf:resource="https://w3id.org/nen2660/term#chemicalFormula"/>
    <skos:definition xml:lang="en">The possession of information about the chemical proportions of atoms that constitute a particular chemical compound</skos:definition>
    <skos:prefLabel xml:lang="en">chemical formula</skos:prefLabel>
  </rdf:Description>
  <rdf:Description rdf:nodeID="n87801b7bffed4f059b3dda9335adfc9ab17">
    <sh:path rdf:resource="https://w3id.org/nen2660/def#hasState"/>
    <sh:class rdf:resource="https://w3id.org/nen2660/def#State"/>
  </rdf:Description>
  <rdf:Description rdf:about="https://w3id.org/nen2660/term#RealObject">
    <rdf:type rdf:resource="http://www.w3.org/2004/02/skos/core#Concept"/>
    <skos:altLabel xml:lang="en">Amount of matter</skos:altLabel>
    <skos:broader rdf:resource="https://w3id.org/nen2660/term#PhysicalObject"/>
    <skos:definition xml:lang="nl">Een fysiek object (vormvast of niet-vormvast) dat in de werkelijkheid tastbaar en zichtbaar is (of kan zijn), door de mens gemaakt of natuurlijk ontstaan</skos:definition>
    <skos:definition xml:lang="en">physical object (rigid or non-rigid) that is (or can be) tangible and visible in reality, man-made or naturally occurring</skos:definition>
    <skos:prefLabel xml:lang="en">Real object</skos:prefLabel>
    <skos:prefLabel xml:lang="nl">Reeel object</skos:prefLabel>
  </rdf:Description>
  <rdf:Description rdf:nodeID="n29315767620c4c949118ed89a344f3a5b17">
    <rdf:type rdf:resource="http://www.w3.org/2002/07/owl#Restriction"/>
    <owl:allValuesFrom rdf:resource="https://w3id.org/nen2660/def#Event"/>
    <owl:onProperty rdf:resource="https://w3id.org/nen2660/def#hasPart"/>
  </rdf:Description>
  <rdf:Description rdf:about="https://w3id.org/nen2660/def#Requirement">
    <rdf:type rdf:resource="http://www.w3.org/2000/01/rdf-schema#Class"/>
    <rdf:type rdf:resource="http://www.w3.org/ns/shacl#NodeShape"/>
    <rdf:type rdf:resource="http://www.w3.org/2002/07/owl#Class"/>
    <rdfs:seeAlso rdf:resource="https://w3id.org/nen2660/term#Requirement"/>
    <rdfs:subClassOf rdf:resource="https://w3id.org/nen2660/def#InformationObject"/>
    <rdfs:subClassOf rdf:nodeID="n29315767620c4c949118ed89a344f3a5b41"/>
    <skos:definition>A rule that should hold for something, defined via its attributes or relations</skos:definition>
    <skos:prefLabel xml:lang="en">Requirement</skos:prefLabel>
    <sh:property rdf:nodeID="n87801b7bffed4f059b3dda9335adfc9ab66"/>
    <sh:property rdf:nodeID="n87801b7bffed4f059b3dda9335adfc9ab67"/>
    <sh:property rdf:nodeID="n87801b7bffed4f059b3dda9335adfc9ab68"/>
    <sh:property rdf:nodeID="n87801b7bffed4f059b3dda9335adfc9ab69"/>
  </rdf:Description>
  <rdf:Description rdf:about="https://w3id.org/nen2660/def#TopConcept">
    <rdf:type rdf:resource="http://www.w3.org/2000/01/rdf-schema#Class"/>
    <rdf:type rdf:resource="http://www.w3.org/ns/shacl#NodeShape"/>
    <rdf:type rdf:resource="http://www.w3.org/2002/07/owl#Class"/>
    <rdfs:seeAlso rdf:resource="https://w3id.org/nen2660/term#TopConcept"/>
    <skos:definition xml:lang="en">The most generic concept</skos:definition>
    <skos:prefLabel xml:lang="en">Top concept</skos:prefLabel>
    <sh:property rdf:nodeID="n87801b7bffed4f059b3dda9335adfc9ab83"/>
    <sh:property rdf:nodeID="n87801b7bffed4f059b3dda9335adfc9ab84"/>
    <sh:property rdf:nodeID="n87801b7bffed4f059b3dda9335adfc9ab85"/>
  </rdf:Description>
  <rdf:Description rdf:about="https://w3id.org/nen2660/def#isConnectedTo">
    <rdf:type rdf:resource="http://www.w3.org/1999/02/22-rdf-syntax-ns#Property"/>
    <rdf:type rdf:resource="http://www.w3.org/2002/07/owl#ObjectProperty"/>
    <rdfs:domain rdf:resource="https://w3id.org/nen2660/def#PhysicalObject"/>
    <rdfs:range rdf:resource="https://w3id.org/nen2660/def#PhysicalObject"/>
    <rdfs:seeAlso rdf:resource="https://w3id.org/nen2660/term#isConnectedTo"/>
    <skos:definition xml:lang="en">The topological relationship between physical objects</skos:definition>
    <skos:prefLabel xml:lang="en">is connected to</skos:prefLabel>
  </rdf:Description>
  <rdf:Description rdf:nodeID="n87801b7bffed4f059b3dda9335adfc9ab60">
    <sh:class rdf:resource="https://w3id.org/nen2660/def#RealObject"/>
  </rdf:Description>
  <rdf:Description rdf:about="https://w3id.org/nen2660/term#isBoundBy">
    <rdf:type rdf:resource="http://www.w3.org/2004/02/skos/core#Concept"/>
    <skos:definition xml:lang="nl">Het fysieke object dat een ruimtelijk gebied begrensd</skos:definition>
    <skos:definition xml:lang="en">The physical object that bounds a spatial region</skos:definition>
    <skos:prefLabel xml:lang="nl">is begrensd door</skos:prefLabel>
    <skos:prefLabel xml:lang="en">is bound by</skos:prefLabel>
  </rdf:Description>
  <rdf:Description rdf:nodeID="n87801b7bffed4f059b3dda9335adfc9ab38">
    <sh:path rdf:resource="https://w3id.org/nen2660/def#hasPart"/>
    <sh:class rdf:resource="https://w3id.org/nen2660/def#Object"/>
  </rdf:Description>
  <rdf:Description rdf:nodeID="n87801b7bffed4f059b3dda9335adfc9ab81">
    <sh:path rdf:resource="https://w3id.org/nen2660/def#hasPart"/>
    <sh:class rdf:resource="https://w3id.org/nen2660/def#Entity"/>
  </rdf:Description>
  <rdf:Description rdf:nodeID="n29315767620c4c949118ed89a344f3a5b2">
    <rdf:first rdf:resource="https://w3id.org/nen2660/def#Solid"/>
    <rdf:rest rdf:nodeID="n29315767620c4c949118ed89a344f3a5b3"/>
  </rdf:Description>
  <rdf:Description rdf:about="https://w3id.org/nen2660/term#Interface">
    <rdf:type rdf:resource="http://www.w3.org/2004/02/skos/core#Concept"/>
    <skos:broader rdf:resource="https://w3id.org/nen2660/term#SpatialRegion"/>
    <skos:definition xml:lang="en">A spatial object, typically a thin 2D physical space (but also 0D or 1D) that connects two physical objects or ports of physical objects through which a static or dynamic interaction or interaction between those elements can take place</skos:definition>
    <skos:definition xml:lang="nl">Een ruimtelijk object, typisch een dunne 2D fysieke ruimte (maar 0D of 1D kan ook) dat de verbinding legt tussen twee fysieke objecten of poorten van fysieke objecten waarlangs een statische of dynamische wisselwerking of interactie tussen die elementen kan plaatsvinden</skos:definition>
    <skos:prefLabel xml:lang="en">Interface</skos:prefLabel>
    <skos:prefLabel xml:lang="nl">Raakvlak</skos:prefLabel>
  </rdf:Description>
  <rdf:Description rdf:about="https://w3id.org/nen2660/term#overConnection">
    <rdf:type rdf:resource="http://www.w3.org/2004/02/skos/core#Concept"/>
    <skos:definition xml:lang="nl">De verbinding waarover een interactie tussen fysieke objecten plaatsvindt</skos:definition>
    <skos:definition xml:lang="en">The connection over which an interaction between physical objects takes place</skos:definition>
    <skos:prefLabel xml:lang="en">over connection</skos:prefLabel>
    <skos:prefLabel xml:lang="nl">over verbinding</skos:prefLabel>
  </rdf:Description>
  <rdf:Description rdf:about="https://w3id.org/nen2660/term#hasPartsGroup">
    <rdf:type rdf:resource="http://www.w3.org/2004/02/skos/core#Concept"/>
    <skos:definition xml:lang="nl">Het hebben van een groep, eventueel impliciete, onderdelen</skos:definition>
    <skos:definition xml:lang="en">The possession of an group of, potentially implicit, parts</skos:definition>
    <skos:prefLabel xml:lang="en">has parts group</skos:prefLabel>
    <skos:prefLabel xml:lang="nl">heeft delen groep</skos:prefLabel>
  </rdf:Description>
  <rdf:Description rdf:nodeID="n87801b7bffed4f059b3dda9335adfc9ab109">
    <rdf:first rdf:resource="http://www.w3.org/1999/02/22-rdf-syntax-ns#type"/>
    <rdf:rest rdf:nodeID="n87801b7bffed4f059b3dda9335adfc9ab110"/>
  </rdf:Description>
  <rdf:Description rdf:nodeID="n87801b7bffed4f059b3dda9335adfc9ab40">
    <sh:path rdf:resource="https://w3id.org/nen2660/def#isConnectedTo"/>
    <sh:class rdf:resource="https://w3id.org/nen2660/def#PhysicalObject"/>
  </rdf:Description>
  <rdf:Description rdf:nodeID="n87801b7bffed4f059b3dda9335adfc9ab117">
    <rdf:first rdf:nodeID="n87801b7bffed4f059b3dda9335adfc9ab115"/>
    <rdf:rest rdf:resource="http://www.w3.org/1999/02/22-rdf-syntax-ns#nil"/>
  </rdf:Description>
  <rdf:Description rdf:about="https://w3id.org/nen2660/def#hasSolution">
    <rdf:type rdf:resource="http://www.w3.org/1999/02/22-rdf-syntax-ns#Property"/>
    <rdf:type rdf:resource="http://www.w3.org/2002/07/owl#ObjectProperty"/>
    <rdfs:domain rdf:resource="https://w3id.org/nen2660/def#FunctionalEntity"/>
    <rdfs:range rdf:resource="https://w3id.org/nen2660/def#TechnicalEntity"/>
    <rdfs:seeAlso rdf:resource="https://w3id.org/nen2660/term#hasSolution"/>
    <skos:definition xml:lang="en">A technical entity that is a potential solution for a functional entity</skos:definition>
    <skos:prefLabel xml:lang="en">has solution</skos:prefLabel>
  </rdf:Description>
  <rdf:Description rdf:nodeID="n87801b7bffed4f059b3dda9335adfc9ab26">
    <sh:path rdf:resource="https://w3id.org/nen2660/def#overInterface"/>
    <sh:class rdf:resource="https://w3id.org/nen2660/def#Interface"/>
  </rdf:Description>
  <rdf:Description rdf:about="https://w3id.org/nen2660/term#EnergyFlow">
    <rdf:type rdf:resource="http://www.w3.org/2004/02/skos/core#Concept"/>
    <skos:broader rdf:resource="https://w3id.org/nen2660/term#TransferType"/>
    <skos:definition xml:lang="nl">De beweging van een hoeveelheid energie (als capaciteit om arbeid te verrichten)</skos:definition>
    <skos:definition xml:lang="en">The movement of an amount of energy (as capacity to do work)</skos:definition>
    <skos:prefLabel xml:lang="nl">Energie stroom</skos:prefLabel>
    <skos:prefLabel xml:lang="en">Energy flow</skos:prefLabel>
  </rdf:Description>
  <rdf:Description rdf:nodeID="n87801b7bffed4f059b3dda9335adfc9ab10">
    <sh:path rdf:resource="https://w3id.org/nen2660/def#hasBoundary"/>
    <sh:class rdf:resource="https://w3id.org/nen2660/def#GeometricEntity"/>
  </rdf:Description>
  <rdf:Description rdf:nodeID="n87801b7bffed4f059b3dda9335adfc9ab39">
    <sh:path rdf:resource="http://www.w3.org/1999/02/22-rdf-syntax-ns#value"/>
    <sh:maxCount rdf:datatype="http://www.w3.org/2001/XMLSchema#integer">1</sh:maxCount>
  </rdf:Description>
  <rdf:Description rdf:nodeID="n29315767620c4c949118ed89a344f3a5b1">
    <rdf:type rdf:resource="http://www.w3.org/2002/07/owl#Restriction"/>
    <owl:allValuesFrom rdf:resource="https://w3id.org/nen2660/def#Activity"/>
    <owl:onProperty rdf:resource="https://w3id.org/nen2660/def#hasPart"/>
  </rdf:Description>
  <rdf:Description rdf:nodeID="n87801b7bffed4f059b3dda9335adfc9ab98">
    <rdf:first rdf:resource="https://w3id.org/nen2660/def#Event"/>
    <rdf:rest rdf:nodeID="n87801b7bffed4f059b3dda9335adfc9ab99"/>
  </rdf:Description>
  <rdf:Description rdf:nodeID="n87801b7bffed4f059b3dda9335adfc9ab51">
    <rdf:first rdf:nodeID="n87801b7bffed4f059b3dda9335adfc9ab48"/>
    <rdf:rest rdf:nodeID="n87801b7bffed4f059b3dda9335adfc9ab52"/>
  </rdf:Description>
  <rdf:Description rdf:about="https://w3id.org/nen2660/term#consistsOf">
    <rdf:type rdf:resource="http://www.w3.org/2004/02/skos/core#Concept"/>
    <skos:definition xml:lang="nl">De materie waarvan een reëel object of mengsel is gemaakt</skos:definition>
    <skos:definition xml:lang="en">The matter a real object or mixture is made of</skos:definition>
    <skos:prefLabel xml:lang="nl">bestaat uit</skos:prefLabel>
    <skos:prefLabel xml:lang="en">consists of</skos:prefLabel>
  </rdf:Description>
  <rdf:Description rdf:about="https://w3id.org/nen2660/def#PureSubstance">
    <rdf:type rdf:resource="http://www.w3.org/2000/01/rdf-schema#Class"/>
    <rdf:type rdf:resource="http://www.w3.org/2002/07/owl#Class"/>
    <rdfs:seeAlso rdf:resource="https://w3id.org/nen2660/term#PureSubstance"/>
    <rdfs:subClassOf rdf:resource="https://w3id.org/nen2660/def#Matter"/>
    <skos:definition xml:lang="en">Chemical matter that has an equal chemical composition and recognizable uniform and isotropic properties</skos:definition>
    <skos:prefLabel xml:lang="en">Pure substance</skos:prefLabel>
  </rdf:Description>
  <rdf:Description rdf:about="https://w3id.org/nen2660/def#TechnicalEntity">
    <rdf:type rdf:resource="http://www.w3.org/2000/01/rdf-schema#Class"/>
    <rdf:type rdf:resource="http://www.w3.org/ns/shacl#NodeShape"/>
    <rdf:type rdf:resource="http://www.w3.org/2002/07/owl#Class"/>
    <rdfs:seeAlso rdf:resource="https://w3id.org/nen2660/term#TechnicalEntity"/>
    <rdfs:subClassOf rdf:resource="https://w3id.org/nen2660/def#Entity"/>
    <rdfs:subClassOf rdf:nodeID="n29315767620c4c949118ed89a344f3a5b47"/>
    <skos:definition xml:lang="en">An entity concerned with technical properties and relations that implements or plays functional entities</skos:definition>
    <skos:prefLabel xml:lang="en">Technical entity</skos:prefLabel>
    <sh:property rdf:nodeID="n87801b7bffed4f059b3dda9335adfc9ab81"/>
    <sh:property rdf:nodeID="n87801b7bffed4f059b3dda9335adfc9ab82"/>
  </rdf:Description>
  <rdf:Description rdf:about="https://w3id.org/nen2660/term#Requirement">
    <rdf:type rdf:resource="http://www.w3.org/2004/02/skos/core#Concept"/>
    <skos:broader rdf:resource="https://w3id.org/nen2660/term#InformationObject"/>
    <skos:definition xml:lang="en">A rule that should hold for something, defined via its attributes or relations</skos:definition>
    <skos:definition xml:lang="nl">Een regel die ergens voor moet gelden, gedefinieerd via zijn attributen of relaties</skos:definition>
    <skos:prefLabel xml:lang="nl">Eis</skos:prefLabel>
    <skos:prefLabel xml:lang="en">Requirement</skos:prefLabel>
  </rdf:Description>
  <rdf:Description rdf:about="https://w3id.org/nen2660/def#AmountOfBulkMatter">
    <rdf:type rdf:resource="http://www.w3.org/2000/01/rdf-schema#Class"/>
    <rdf:type rdf:resource="http://www.w3.org/2002/07/owl#Class"/>
    <rdfs:seeAlso rdf:resource="https://w3id.org/nen2660/term#AmountOfBulkMatter"/>
    <rdfs:subClassOf rdf:resource="https://w3id.org/nen2660/def#RealObject"/>
    <skos:definition xml:lang="en">A real object that consists of a continuous amount of non-rigid matter, held together primarily by external forces (gravity or confinement)</skos:definition>
    <skos:prefLabel xml:lang="en">Amount of bulk matter</skos:prefLabel>
  </rdf:Description>
  <rdf:Description rdf:about="https://w3id.org/nen2660/def#hasBoundary">
    <rdf:type rdf:resource="http://www.w3.org/1999/02/22-rdf-syntax-ns#Property"/>
    <rdf:type rdf:resource="http://www.w3.org/2002/07/owl#ObjectProperty"/>
    <rdfs:domain rdf:resource="https://w3id.org/nen2660/def#ConcreteConcept"/>
    <rdfs:range rdf:resource="https://w3id.org/nen2660/def#GeometricEntity"/>
    <rdfs:seeAlso rdf:resource="https://w3id.org/nen2660/term#hasBoundary"/>
    <skos:definition xml:lang="en">The geometric entity representing the boundary of a concrete concept</skos:definition>
    <skos:prefLabel xml:lang="en">has boundary</skos:prefLabel>
  </rdf:Description>
  <rdf:Description rdf:nodeID="n29315767620c4c949118ed89a344f3a5b13">
    <rdf:first rdf:resource="https://w3id.org/nen2660/def#FunctionalEntity"/>
    <rdf:rest rdf:nodeID="n29315767620c4c949118ed89a344f3a5b14"/>
  </rdf:Description>
  <rdf:Description rdf:about="https://w3id.org/nen2660/term#requirementTopicType">
    <rdf:type rdf:resource="http://www.w3.org/2004/02/skos/core#Concept"/>
    <skos:definition xml:lang="nl">Het hebben van een onderwerptype door een eis</skos:definition>
    <skos:definition xml:lang="en">The possession of a topic type by a requirement</skos:definition>
    <skos:prefLabel xml:lang="nl">eis onderwerp type</skos:prefLabel>
    <skos:prefLabel xml:lang="en">requirement topic type</skos:prefLabel>
  </rdf:Description>
  <rdf:Description rdf:about="https://w3id.org/nen2660/term#InformationObject">
    <rdf:type rdf:resource="http://www.w3.org/2004/02/skos/core#Concept"/>
    <skos:broader rdf:resource="https://w3id.org/nen2660/term#Object"/>
    <skos:definition xml:lang="nl">Object dat een beschrijving vormt van een ding in de werkelijkheid</skos:definition>
    <skos:definition xml:lang="en">Object which describes a thing in reality</skos:definition>
    <skos:prefLabel xml:lang="nl">Informatie object</skos:prefLabel>
    <skos:prefLabel xml:lang="en">Information object</skos:prefLabel>
  </rdf:Description>
  <rdf:Description rdf:about="https://w3id.org/nen2660/term#requirementSeverityType">
    <rdf:type rdf:resource="http://www.w3.org/2004/02/skos/core#Concept"/>
    <skos:definition xml:lang="nl">Het hebben van een ernsttype door een eis</skos:definition>
    <skos:definition xml:lang="en">The possession of a severity type by a requirement</skos:definition>
    <skos:prefLabel xml:lang="nl">eis ernst type</skos:prefLabel>
    <skos:prefLabel xml:lang="en">requirement severity type</skos:prefLabel>
  </rdf:Description>
  <rdf:Description rdf:nodeID="n87801b7bffed4f059b3dda9335adfc9ab72">
    <sh:class rdf:resource="https://w3id.org/nen2660/def#SpatialRegion"/>
  </rdf:Description>
  <rdf:Description rdf:about="https://w3id.org/nen2660/term#executes">
    <rdf:type rdf:resource="http://www.w3.org/2004/02/skos/core#Concept"/>
    <skos:definition xml:lang="nl">De activiteit uitgevoerd door een fysiek object</skos:definition>
    <skos:definition xml:lang="en">The activity executed by a physical object</skos:definition>
    <skos:prefLabel xml:lang="en">executes</skos:prefLabel>
    <skos:prefLabel xml:lang="nl">voert uit</skos:prefLabel>
  </rdf:Description>
  <rdf:Description rdf:about="https://w3id.org/nen2660/term#RealizedEntity">
    <rdf:type rdf:resource="http://www.w3.org/2004/02/skos/core#Concept"/>
    <skos:broader rdf:resource="https://w3id.org/nen2660/term#Entity"/>
    <skos:definition xml:lang="en">An entity that exists or has existed in the physical reality</skos:definition>
    <skos:definition xml:lang="nl">Een entiteit die bestaat of heeft bestaan in de fysieke werkelijkheid</skos:definition>
    <skos:prefLabel xml:lang="nl">Gerealiseerde entiteit</skos:prefLabel>
    <skos:prefLabel xml:lang="en">Realized entity</skos:prefLabel>
  </rdf:Description>
  <rdf:Description rdf:nodeID="n87801b7bffed4f059b3dda9335adfc9ab74">
    <rdf:first rdf:nodeID="n87801b7bffed4f059b3dda9335adfc9ab72"/>
    <rdf:rest rdf:nodeID="n87801b7bffed4f059b3dda9335adfc9ab75"/>
  </rdf:Description>
  <rdf:Description rdf:nodeID="n87801b7bffed4f059b3dda9335adfc9ab30">
    <sh:path rdf:resource="https://w3id.org/nen2660/def#aggregationStateType"/>
    <sh:class rdf:resource="https://w3id.org/nen2660/def#AggregationStateType"/>
  </rdf:Description>
  <rdf:Description rdf:nodeID="n87801b7bffed4f059b3dda9335adfc9ab45">
    <sh:path rdf:resource="https://w3id.org/nen2660/def#isPlanFor"/>
    <sh:class rdf:resource="https://w3id.org/nen2660/def#RealizedEntity"/>
  </rdf:Description>
  <rdf:Description rdf:nodeID="n87801b7bffed4f059b3dda9335adfc9ab36">
    <rdf:first rdf:nodeID="n87801b7bffed4f059b3dda9335adfc9ab34"/>
    <rdf:rest rdf:nodeID="n87801b7bffed4f059b3dda9335adfc9ab37"/>
  </rdf:Description>
  <rdf:Description rdf:about="https://w3id.org/nen2660/def#isBoundBy">
    <rdf:type rdf:resource="http://www.w3.org/1999/02/22-rdf-syntax-ns#Property"/>
    <rdf:type rdf:resource="http://www.w3.org/2002/07/owl#ObjectProperty"/>
    <rdfs:domain rdf:resource="https://w3id.org/nen2660/def#SpatialRegion"/>
    <rdfs:range rdf:resource="https://w3id.org/nen2660/def#PhysicalObject"/>
    <rdfs:seeAlso rdf:resource="https://w3id.org/nen2660/term#isBoundBy"/>
    <skos:definition xml:lang="en">The physical object that bounds a spatial region</skos:definition>
    <skos:prefLabel xml:lang="en">is bound by</skos:prefLabel>
  </rdf:Description>
  <rdf:Description rdf:nodeID="n29315767620c4c949118ed89a344f3a5b5">
    <rdf:first rdf:resource="https://w3id.org/nen2660/def#Plasma"/>
    <rdf:rest rdf:resource="http://www.w3.org/1999/02/22-rdf-syntax-ns#nil"/>
  </rdf:Description>
  <rdf:Description rdf:nodeID="n29315767620c4c949118ed89a344f3a5b39">
    <rdf:type rdf:resource="http://www.w3.org/2002/07/owl#Restriction"/>
    <owl:allValuesFrom rdf:resource="https://w3id.org/nen2660/def#RealizedEntity"/>
    <owl:onProperty rdf:resource="https://w3id.org/nen2660/def#hasPart"/>
  </rdf:Description>
  <rdf:Description rdf:about="https://w3id.org/nen2660/def#ChemicalCompound">
    <rdf:type rdf:resource="http://www.w3.org/2000/01/rdf-schema#Class"/>
    <rdf:type rdf:resource="http://www.w3.org/2002/07/owl#Class"/>
    <rdfs:seeAlso rdf:resource="https://w3id.org/nen2660/term#ChemicalBonding"/>
    <rdfs:subClassOf rdf:resource="https://w3id.org/nen2660/def#PureSubstance"/>
    <skos:definition xml:lang="en">Pure substance consisting of two or more chemical elements that have a chemical bond with each other. In a chemical compound, the elements occur in a fixed ratio. A compound can be broken down into simpler substances by means of chemical reactions</skos:definition>
    <skos:prefLabel xml:lang="en">Chemical compound</skos:prefLabel>
  </rdf:Description>
  <rdf:Description rdf:about="https://w3id.org/nen2660/term#Solid">
    <rdf:type rdf:resource="http://www.w3.org/2004/02/skos/core#Concept"/>
    <skos:broader rdf:resource="https://w3id.org/nen2660/term#AggregationStateType"/>
    <skos:definition xml:lang="nl">Materie die kan worden opgepakt of vastgehouden, een textuur heeft en meestal stevig is. In tegenstelling tot een vloeistof, gas of plasma</skos:definition>
    <skos:definition xml:lang="en">Matter that can be picked up or held, having a texture, and usually firm. Unlike a liquid, gas or plasma</skos:definition>
    <skos:prefLabel xml:lang="en">Solid</skos:prefLabel>
    <skos:prefLabel xml:lang="nl">Vaste stof</skos:prefLabel>
  </rdf:Description>
  <rdf:Description rdf:nodeID="n87801b7bffed4f059b3dda9335adfc9ab5">
    <sh:path rdf:resource="https://w3id.org/nen2660/def#transforms"/>
    <sh:class rdf:resource="https://w3id.org/nen2660/def#Object"/>
  </rdf:Description>
  <rdf:Description rdf:nodeID="n87801b7bffed4f059b3dda9335adfc9ab2">
    <sh:path rdf:resource="https://w3id.org/nen2660/def#hasInterior"/>
    <sh:class rdf:resource="https://w3id.org/nen2660/def#GeometricEntity"/>
  </rdf:Description>
  <rdf:Description rdf:nodeID="n29315767620c4c949118ed89a344f3a5b56">
    <rdf:first rdf:resource="https://w3id.org/nen2660/def#Connection"/>
    <rdf:rest rdf:nodeID="n29315767620c4c949118ed89a344f3a5b57"/>
  </rdf:Description>
  <rdf:Description rdf:nodeID="n87801b7bffed4f059b3dda9335adfc9ab83">
    <sh:path rdf:resource="https://w3id.org/nen2660/def#abbreviation"/>
    <sh:datatype rdf:resource="http://www.w3.org/2001/XMLSchema#string"/>
  </rdf:Description>
  <rdf:Description rdf:about="https://w3id.org/nen2660/def#Entity">
    <rdf:type rdf:resource="http://www.w3.org/2000/01/rdf-schema#Class"/>
    <rdf:type rdf:resource="http://www.w3.org/ns/shacl#NodeShape"/>
    <rdf:type rdf:resource="http://www.w3.org/2002/07/owl#Class"/>
    <rdfs:seeAlso rdf:resource="https://w3id.org/nen2660/term#Entity"/>
    <rdfs:subClassOf rdf:resource="https://w3id.org/nen2660/def#ConcreteConcept"/>
    <skos:definition xml:lang="en">Concept that forms a manifestation and a demarcation in a concrete space-time, and which has a certain state at any moment in time. An entity has a unique identity that remains constant throughout its life cycle. The life cycle of an entity is made up of the sequence of states of that entity, which follow each other in time. An entity is an object or an activity. An object exists, an activity takes place</skos:definition>
    <skos:prefLabel xml:lang="en">Entity</skos:prefLabel>
    <sh:property rdf:nodeID="n87801b7bffed4f059b3dda9335adfc9ab17"/>
    <sh:property rdf:nodeID="n87801b7bffed4f059b3dda9335adfc9ab18"/>
  </rdf:Description>
  <rdf:Description rdf:nodeID="n29315767620c4c949118ed89a344f3a5b22">
    <rdf:type rdf:resource="http://www.w3.org/2002/07/owl#Restriction"/>
    <owl:maxCardinality rdf:datatype="http://www.w3.org/2001/XMLSchema#nonNegativeInteger">1</owl:maxCardinality>
    <owl:onProperty rdf:resource="http://www.w3.org/1999/02/22-rdf-syntax-ns#value"/>
  </rdf:Description>
  <rdf:Description rdf:nodeID="n87801b7bffed4f059b3dda9335adfc9ab108">
    <sh:zeroOrMorePath rdf:resource="http://www.w3.org/2000/01/rdf-schema#subClassOf"/>
  </rdf:Description>
  <rdf:Description rdf:nodeID="n29315767620c4c949118ed89a344f3a5b49">
    <rdf:first rdf:resource="https://w3id.org/nen2660/def#EnergyFlow"/>
    <rdf:rest rdf:nodeID="n29315767620c4c949118ed89a344f3a5b50"/>
  </rdf:Description>
  <rdf:Description rdf:about="https://w3id.org/nen2660/def#hasInterior">
    <rdf:type rdf:resource="http://www.w3.org/1999/02/22-rdf-syntax-ns#Property"/>
    <rdf:type rdf:resource="http://www.w3.org/2002/07/owl#ObjectProperty"/>
    <rdfs:domain rdf:resource="https://w3id.org/nen2660/def#ConcreteConcept"/>
    <rdfs:range rdf:resource="https://w3id.org/nen2660/def#GeometricEntity"/>
    <rdfs:seeAlso rdf:resource="https://w3id.org/nen2660/term#hasInterior"/>
    <skos:definition xml:lang="en">The geometric entity representing the interior of a concrete concept</skos:definition>
    <skos:prefLabel xml:lang="en">has interior</skos:prefLabel>
  </rdf:Description>
  <rdf:Description rdf:about="https://w3id.org/nen2660/def#HomogeneousMixture">
    <rdf:type rdf:resource="http://www.w3.org/2000/01/rdf-schema#Class"/>
    <rdf:type rdf:resource="http://www.w3.org/2002/07/owl#Class"/>
    <rdfs:seeAlso rdf:resource="https://w3id.org/nen2660/term#HomogeneousMixture"/>
    <rdfs:subClassOf rdf:resource="https://w3id.org/nen2660/def#Mixture"/>
    <skos:definition xml:lang="en">A mixture that is uniform throughout, and has only one phase</skos:definition>
    <skos:prefLabel xml:lang="en">Homogeneous mixture</skos:prefLabel>
  </rdf:Description>
  <rdf:Description rdf:about="https://w3id.org/nen2660/def#EnergyFlow">
    <rdf:type rdf:resource="https://w3id.org/nen2660/def#TransferType"/>
    <rdfs:seeAlso rdf:resource="https://w3id.org/nen2660/term#EnergyFlow"/>
    <skos:definition xml:lang="en">The movement of an amount of energy (as capacity to do work)</skos:definition>
    <skos:prefLabel xml:lang="en">Energy flow</skos:prefLabel>
  </rdf:Description>
  <rdf:Description rdf:nodeID="n87801b7bffed4f059b3dda9335adfc9ab112">
    <rdf:first rdf:resource="https://w3id.org/nen2660/def#FunctionalEntity"/>
    <rdf:rest rdf:nodeID="n87801b7bffed4f059b3dda9335adfc9ab113"/>
  </rdf:Description>
  <rdf:Description rdf:nodeID="n87801b7bffed4f059b3dda9335adfc9ab87">
    <rdf:first rdf:resource="https://w3id.org/nen2660/def#EnergyFlow"/>
    <rdf:rest rdf:nodeID="n87801b7bffed4f059b3dda9335adfc9ab88"/>
  </rdf:Description>
  <rdf:Description rdf:about="https://w3id.org/nen2660/term#connectsPort">
    <rdf:type rdf:resource="http://www.w3.org/2004/02/skos/core#Concept"/>
    <skos:definition xml:lang="nl">De poorten (als onderdeel van fysieke objecten) verbonden door een verbinding of interface</skos:definition>
    <skos:definition xml:lang="en">The ports (as part of physical objects) connected by a connection or interface</skos:definition>
    <skos:prefLabel xml:lang="en">connects port</skos:prefLabel>
    <skos:prefLabel xml:lang="nl">verbindt poort</skos:prefLabel>
  </rdf:Description>
  <rdf:Description rdf:nodeID="n29315767620c4c949118ed89a344f3a5b28">
    <rdf:first rdf:resource="http://www.w3.org/2001/XMLSchema#anyURI"/>
    <rdf:rest rdf:resource="http://www.w3.org/1999/02/22-rdf-syntax-ns#nil"/>
  </rdf:Description>
  <rdf:Description rdf:about="https://w3id.org/nen2660/def#AllDisjointClasses_2">
    <rdf:type rdf:resource="http://www.w3.org/2002/07/owl#AllDisjointClasses"/>
    <owl:members rdf:nodeID="n29315767620c4c949118ed89a344f3a5b11"/>
  </rdf:Description>
  <rdf:Description rdf:nodeID="n29315767620c4c949118ed89a344f3a5b20">
    <rdf:type rdf:resource="http://www.w3.org/2002/07/owl#Restriction"/>
    <owl:onClass rdf:resource="https://w3id.org/nen2660/def#Matter"/>
    <owl:onProperty rdf:resource="http://www.w3.org/1999/02/22-rdf-syntax-ns#value"/>
    <owl:qualifiedCardinality rdf:datatype="http://www.w3.org/2001/XMLSchema#nonNegativeInteger">1</owl:qualifiedCardinality>
  </rdf:Description>
  <rdf:Description rdf:about="https://w3id.org/nen2660/term#contains">
    <rdf:type rdf:resource="http://www.w3.org/2004/02/skos/core#Concept"/>
    <skos:definition xml:lang="nl">De reële objecten die zich in een ruimtelijk gebied bevinden, meestal de gasvormige hoeveelheid bulkmaterie die in dat gebied aanwezig is</skos:definition>
    <skos:definition xml:lang="en">The real objects located in a spatial region, typically the gaseous amount of bulk matter present in that region</skos:definition>
    <skos:prefLabel xml:lang="nl">bevat</skos:prefLabel>
    <skos:prefLabel xml:lang="en">contains</skos:prefLabel>
  </rdf:Description>
  <rdf:Description rdf:nodeID="n87801b7bffed4f059b3dda9335adfc9ab44">
    <sh:path rdf:resource="https://w3id.org/nen2660/def#hasPart"/>
    <sh:class rdf:resource="https://w3id.org/nen2660/def#PlannedEntity"/>
  </rdf:Description>
  <rdf:Description rdf:about="https://w3id.org/nen2660/term#RequirementSeverityType">
    <rdf:type rdf:resource="http://www.w3.org/2004/02/skos/core#Concept"/>
    <skos:broader rdf:resource="https://w3id.org/nen2660/term#EnumerationType"/>
    <skos:definition xml:lang="nl">De ernst van een eis zoals gevraagd of gewenst</skos:definition>
    <skos:definition xml:lang="en">The seriousness of a requirement like demanded or wished</skos:definition>
    <skos:prefLabel xml:lang="nl">Eis ernst type</skos:prefLabel>
    <skos:prefLabel xml:lang="en">Requirement severity type</skos:prefLabel>
  </rdf:Description>
  <rdf:Description rdf:about="https://w3id.org/nen2660/term#isConnectedTo">
    <rdf:type rdf:resource="http://www.w3.org/2004/02/skos/core#Concept"/>
    <skos:definition xml:lang="nl">De topologische relatie tussen fysieke objecten</skos:definition>
    <skos:definition xml:lang="en">The topological relation between physical objects</skos:definition>
    <skos:prefLabel xml:lang="en">is connected to</skos:prefLabel>
    <skos:prefLabel xml:lang="nl">is verbonden met</skos:prefLabel>
  </rdf:Description>
  <rdf:Description rdf:nodeID="n87801b7bffed4f059b3dda9335adfc9ab70">
    <sh:path rdf:resource="https://w3id.org/nen2660/def#contains"/>
    <sh:class rdf:resource="https://w3id.org/nen2660/def#RealObject"/>
  </rdf:Description>
  <rdf:Description rdf:nodeID="n87801b7bffed4f059b3dda9335adfc9ab103">
    <rdf:first rdf:nodeID="n87801b7bffed4f059b3dda9335adfc9ab101"/>
    <rdf:rest rdf:resource="http://www.w3.org/1999/02/22-rdf-syntax-ns#nil"/>
  </rdf:Description>
  <rdf:Description rdf:about="https://w3id.org/nen2660/def#hasPart">
    <rdf:type rdf:resource="http://www.w3.org/1999/02/22-rdf-syntax-ns#Property"/>
    <rdf:type rdf:resource="http://www.w3.org/2002/07/owl#ObjectProperty"/>
    <rdfs:domain rdf:resource="https://w3id.org/nen2660/def#ConcreteConcept"/>
    <rdfs:range rdf:resource="https://w3id.org/nen2660/def#ConcreteConcept"/>
    <rdfs:seeAlso rdf:resource="https://w3id.org/nen2660/term#hasPart"/>
    <skos:definition xml:lang="en">A decomposition (hasPart) relation between concrete concepts</skos:definition>
    <skos:prefLabel xml:lang="en">has part</skos:prefLabel>
  </rdf:Description>
  <rdf:Description rdf:nodeID="n29315767620c4c949118ed89a344f3a5b14">
    <rdf:first rdf:resource="https://w3id.org/nen2660/def#TechnicalEntity"/>
    <rdf:rest rdf:resource="http://www.w3.org/1999/02/22-rdf-syntax-ns#nil"/>
  </rdf:Description>
  <rdf:Description rdf:nodeID="n87801b7bffed4f059b3dda9335adfc9ab106">
    <rdf:first rdf:resource="https://w3id.org/nen2660/def#SpatialRegion"/>
    <rdf:rest rdf:resource="http://www.w3.org/1999/02/22-rdf-syntax-ns#nil"/>
  </rdf:Description>
  <rdf:Description rdf:nodeID="n87801b7bffed4f059b3dda9335adfc9ab93">
    <rdf:first rdf:nodeID="n87801b7bffed4f059b3dda9335adfc9ab91"/>
    <rdf:rest rdf:resource="http://www.w3.org/1999/02/22-rdf-syntax-ns#nil"/>
  </rdf:Description>
  <rdf:Description rdf:nodeID="n29315767620c4c949118ed89a344f3a5b44">
    <rdf:first rdf:resource="https://w3id.org/nen2660/def#SpatialRegion"/>
    <rdf:rest rdf:nodeID="n29315767620c4c949118ed89a344f3a5b45"/>
  </rdf:Description>
  <rdf:Description rdf:nodeID="n87801b7bffed4f059b3dda9335adfc9ab6">
    <rdf:first rdf:resource="https://w3id.org/nen2660/def#Solid"/>
    <rdf:rest rdf:nodeID="n87801b7bffed4f059b3dda9335adfc9ab7"/>
  </rdf:Description>
  <rdf:Description rdf:about="https://w3id.org/nen2660/term#AmountOfBulkMatter">
    <rdf:type rdf:resource="http://www.w3.org/2004/02/skos/core#Concept"/>
    <skos:broader rdf:resource="https://w3id.org/nen2660/term#RealObject"/>
    <skos:definition xml:lang="en">A real object that consists of a continuous amount of non-rigid matter, held together primarily by external forces (gravity or confinement)</skos:definition>
    <skos:definition xml:lang="nl">Een reëel object dat bestaat uit een aaneengesloten hoeveelheid niet-vormvaste materie, primair bijeengehouden door externe krachten (zwaartekracht of opsluiting)</skos:definition>
    <skos:prefLabel xml:lang="en">Amount of bulk matter</skos:prefLabel>
    <skos:prefLabel xml:lang="nl">Hoeveelheid bulkmaterie</skos:prefLabel>
  </rdf:Description>
  <rdf:Description rdf:nodeID="n87801b7bffed4f059b3dda9335adfc9ab114">
    <sh:path rdf:nodeID="n87801b7bffed4f059b3dda9335adfc9ab116"/>
    <sh:qualifiedValueShape rdf:nodeID="n87801b7bffed4f059b3dda9335adfc9ab118"/>
    <sh:qualifiedMaxCount rdf:datatype="http://www.w3.org/2001/XMLSchema#integer">1</sh:qualifiedMaxCount>
  </rdf:Description>
  <rdf:Description rdf:about="https://w3id.org/nen2660/def#AbstractConcept">
    <rdf:type rdf:resource="http://www.w3.org/2000/01/rdf-schema#Class"/>
    <rdf:type rdf:resource="http://www.w3.org/2002/07/owl#Class"/>
    <rdfs:seeAlso rdf:resource="https://w3id.org/nen2660/term#AbstractConcept"/>
    <rdfs:subClassOf rdf:resource="https://w3id.org/nen2660/def#TopConcept"/>
    <skos:definition xml:lang="en">Concept that forms a manifestation and demarcation in an abstract space. An abstract concept has no life cycle</skos:definition>
    <skos:prefLabel xml:lang="en">Abstract concept</skos:prefLabel>
  </rdf:Description>
  <rdf:Description rdf:nodeID="n87801b7bffed4f059b3dda9335adfc9ab79">
    <sh:path rdf:resource="https://w3id.org/nen2660/def#hasPart"/>
    <sh:class rdf:resource="https://w3id.org/nen2660/def#State"/>
  </rdf:Description>
  <rdf:Description rdf:about="https://w3id.org/nen2660/term#chemicalFormula">
    <rdf:type rdf:resource="http://www.w3.org/2004/02/skos/core#Concept"/>
    <skos:definition xml:lang="nl">Het hebben van informatie over de chemische verhoudingen van atomen die een bepaalde chemische verbinding vormen</skos:definition>
    <skos:definition xml:lang="en">The possession of information about the chemical proportions of atoms that constitute a particular chemical compound</skos:definition>
    <skos:prefLabel xml:lang="en">chemical formula</skos:prefLabel>
    <skos:prefLabel xml:lang="nl">chemische formule</skos:prefLabel>
  </rdf:Description>
  <rdf:Description rdf:nodeID="n29315767620c4c949118ed89a344f3a5b21">
    <rdf:type rdf:resource="http://www.w3.org/2002/07/owl#Restriction"/>
    <owl:allValuesFrom rdf:resource="https://w3id.org/nen2660/def#Object"/>
    <owl:onProperty rdf:resource="https://w3id.org/nen2660/def#hasPart"/>
  </rdf:Description>
  <rdf:Description rdf:nodeID="n29315767620c4c949118ed89a344f3a5b62">
    <rdf:first rdf:resource="https://w3id.org/nen2660/def#Matter"/>
    <rdf:rest rdf:nodeID="n29315767620c4c949118ed89a344f3a5b63"/>
  </rdf:Description>
  <rdf:Description rdf:nodeID="n29315767620c4c949118ed89a344f3a5b32">
    <rdf:first rdf:resource="http://www.w3.org/2001/XMLSchema#float"/>
    <rdf:rest rdf:nodeID="n29315767620c4c949118ed89a344f3a5b33"/>
  </rdf:Description>
  <rdf:Description rdf:nodeID="n87801b7bffed4f059b3dda9335adfc9ab69">
    <sh:path rdf:resource="https://w3id.org/nen2660/def#requirementTopicType"/>
    <sh:class rdf:resource="https://w3id.org/nen2660/def#RequirementTopicType"/>
  </rdf:Description>
  <rdf:Description rdf:about="https://w3id.org/nen2660/def#InformationFlow">
    <rdf:type rdf:resource="https://w3id.org/nen2660/def#TransferType"/>
    <rdfs:seeAlso rdf:resource="https://w3id.org/nen2660/term#InformationFlow"/>
    <skos:definition xml:lang="en">The movement of information represented in some medium</skos:definition>
    <skos:prefLabel xml:lang="en">Information flow</skos:prefLabel>
  </rdf:Description>
  <rdf:Description rdf:nodeID="n87801b7bffed4f059b3dda9335adfc9ab89">
    <rdf:first rdf:resource="https://w3id.org/nen2660/def#Force"/>
    <rdf:rest rdf:resource="http://www.w3.org/1999/02/22-rdf-syntax-ns#nil"/>
  </rdf:Description>
  <rdf:Description rdf:nodeID="n87801b7bffed4f059b3dda9335adfc9ab57">
    <rdf:first rdf:nodeID="n87801b7bffed4f059b3dda9335adfc9ab55"/>
    <rdf:rest rdf:nodeID="n87801b7bffed4f059b3dda9335adfc9ab58"/>
  </rdf:Description>
  <rdf:Description rdf:nodeID="n87801b7bffed4f059b3dda9335adfc9ab107">
    <sh:path rdf:nodeID="n87801b7bffed4f059b3dda9335adfc9ab109"/>
    <sh:qualifiedValueShape rdf:nodeID="n87801b7bffed4f059b3dda9335adfc9ab111"/>
    <sh:qualifiedMaxCount rdf:datatype="http://www.w3.org/2001/XMLSchema#integer">1</sh:qualifiedMaxCount>
  </rdf:Description>
  <rdf:Description rdf:nodeID="n87801b7bffed4f059b3dda9335adfc9ab113">
    <rdf:first rdf:resource="https://w3id.org/nen2660/def#TechnicalEntity"/>
    <rdf:rest rdf:resource="http://www.w3.org/1999/02/22-rdf-syntax-ns#nil"/>
  </rdf:Description>
  <rdf:Description rdf:nodeID="n29315767620c4c949118ed89a344f3a5b45">
    <rdf:first rdf:resource="https://w3id.org/nen2660/def#Port"/>
    <rdf:rest rdf:resource="http://www.w3.org/1999/02/22-rdf-syntax-ns#nil"/>
  </rdf:Description>
  <rdf:Description rdf:nodeID="n87801b7bffed4f059b3dda9335adfc9ab104">
    <sh:in rdf:nodeID="n87801b7bffed4f059b3dda9335adfc9ab105"/>
  </rdf:Description>
  <rdf:Description rdf:about="https://w3id.org/nen2660/term#hasInterior">
    <rdf:type rdf:resource="http://www.w3.org/2004/02/skos/core#Concept"/>
    <skos:definition xml:lang="nl">De geometrische entiteit die het inwendige van een concreet concept vertegenwoordigt</skos:definition>
    <skos:definition xml:lang="en">The geometric entity representing the interior of a concrete concept</skos:definition>
    <skos:prefLabel xml:lang="en">has interior</skos:prefLabel>
    <skos:prefLabel xml:lang="nl">heeft inwendige</skos:prefLabel>
  </rdf:Description>
  <rdf:Description rdf:nodeID="n87801b7bffed4f059b3dda9335adfc9ab100">
    <sh:path rdf:nodeID="n87801b7bffed4f059b3dda9335adfc9ab102"/>
    <sh:qualifiedValueShape rdf:nodeID="n87801b7bffed4f059b3dda9335adfc9ab104"/>
    <sh:qualifiedMaxCount rdf:datatype="http://www.w3.org/2001/XMLSchema#integer">1</sh:qualifiedMaxCount>
  </rdf:Description>
  <rdf:Description rdf:nodeID="n87801b7bffed4f059b3dda9335adfc9ab63">
    <rdf:first rdf:nodeID="n87801b7bffed4f059b3dda9335adfc9ab61"/>
    <rdf:rest rdf:resource="http://www.w3.org/1999/02/22-rdf-syntax-ns#nil"/>
  </rdf:Description>
  <rdf:Description rdf:nodeID="n29315767620c4c949118ed89a344f3a5b4">
    <rdf:first rdf:resource="https://w3id.org/nen2660/def#Gas"/>
    <rdf:rest rdf:nodeID="n29315767620c4c949118ed89a344f3a5b5"/>
  </rdf:Description>
  <rdf:Description rdf:nodeID="n87801b7bffed4f059b3dda9335adfc9ab61">
    <sh:class rdf:resource="https://w3id.org/nen2660/def#Port"/>
  </rdf:Description>
  <rdf:Description rdf:nodeID="n87801b7bffed4f059b3dda9335adfc9ab75">
    <rdf:first rdf:nodeID="n87801b7bffed4f059b3dda9335adfc9ab73"/>
    <rdf:rest rdf:resource="http://www.w3.org/1999/02/22-rdf-syntax-ns#nil"/>
  </rdf:Description>
  <rdf:Description rdf:nodeID="n87801b7bffed4f059b3dda9335adfc9ab13">
    <sh:path rdf:resource="https://w3id.org/nen2660/def#hasPart"/>
    <sh:class rdf:resource="https://w3id.org/nen2660/def#ConcreteConcept"/>
  </rdf:Description>
  <rdf:Description rdf:nodeID="n29315767620c4c949118ed89a344f3a5b6">
    <rdf:first rdf:resource="https://w3id.org/nen2660/def#PhysicalObject"/>
    <rdf:rest rdf:nodeID="n29315767620c4c949118ed89a344f3a5b7"/>
  </rdf:Description>
  <rdf:Description rdf:nodeID="n87801b7bffed4f059b3dda9335adfc9ab110">
    <rdf:first rdf:nodeID="n87801b7bffed4f059b3dda9335adfc9ab108"/>
    <rdf:rest rdf:resource="http://www.w3.org/1999/02/22-rdf-syntax-ns#nil"/>
  </rdf:Description>
  <rdf:Description rdf:nodeID="n87801b7bffed4f059b3dda9335adfc9ab92">
    <rdf:first rdf:resource="http://www.w3.org/1999/02/22-rdf-syntax-ns#type"/>
    <rdf:rest rdf:nodeID="n87801b7bffed4f059b3dda9335adfc9ab93"/>
  </rdf:Description>
  <rdf:Description rdf:nodeID="n29315767620c4c949118ed89a344f3a5b36">
    <rdf:type rdf:resource="http://www.w3.org/2002/07/owl#Class"/>
    <owl:unionOf rdf:nodeID="n29315767620c4c949118ed89a344f3a5b37"/>
  </rdf:Description>
  <rdf:Description rdf:nodeID="n29315767620c4c949118ed89a344f3a5b16">
    <rdf:first rdf:resource="https://w3id.org/nen2660/def#RealizedEntity"/>
    <rdf:rest rdf:resource="http://www.w3.org/1999/02/22-rdf-syntax-ns#nil"/>
  </rdf:Description>
  <rdf:Description rdf:nodeID="n87801b7bffed4f059b3dda9335adfc9ab20">
    <sh:path rdf:resource="https://w3id.org/nen2660/def#ends"/>
    <sh:class rdf:resource="https://w3id.org/nen2660/def#State"/>
  </rdf:Description>
  <rdf:Description rdf:nodeID="n87801b7bffed4f059b3dda9335adfc9ab64">
    <sh:path rdf:resource="https://w3id.org/nen2660/def#hasPart"/>
    <sh:class rdf:resource="https://w3id.org/nen2660/def#RealizedEntity"/>
  </rdf:Description>
  <rdf:Description rdf:nodeID="n87801b7bffed4f059b3dda9335adfc9ab47">
    <sh:path rdf:resource="http://www.w3.org/1999/02/22-rdf-syntax-ns#value"/>
    <sh:or rdf:nodeID="n87801b7bffed4f059b3dda9335adfc9ab51"/>
  </rdf:Description>
  <rdf:Description rdf:nodeID="n87801b7bffed4f059b3dda9335adfc9ab41">
    <sh:path rdf:resource="https://w3id.org/nen2660/def#isDescribedBy"/>
    <sh:class rdf:resource="https://w3id.org/nen2660/def#InformationObject"/>
  </rdf:Description>
  <rdf:Description rdf:nodeID="n87801b7bffed4f059b3dda9335adfc9ab50">
    <sh:datatype rdf:resource="http://www.w3.org/2001/XMLSchema#double"/>
  </rdf:Description>
  <rdf:Description rdf:nodeID="n87801b7bffed4f059b3dda9335adfc9ab12">
    <sh:path rdf:resource="https://w3id.org/nen2660/def#hasTemporalEntity"/>
    <sh:class rdf:resource="http://www.w3.org/2006/time#TemporalEntity"/>
  </rdf:Description>
  <rdf:Description rdf:nodeID="n87801b7bffed4f059b3dda9335adfc9ab28">
    <sh:path rdf:resource="https://w3id.org/nen2660/def#connectsObject"/>
    <sh:class rdf:resource="https://w3id.org/nen2660/def#PhysicalObject"/>
  </rdf:Description>
  <rdf:Description rdf:nodeID="n87801b7bffed4f059b3dda9335adfc9ab34">
    <sh:class rdf:resource="https://w3id.org/nen2660/def#Matter"/>
  </rdf:Description>
  <rdf:Description rdf:nodeID="n29315767620c4c949118ed89a344f3a5b27">
    <rdf:first rdf:resource="http://www.w3.org/2001/XMLSchema#boolean"/>
    <rdf:rest rdf:nodeID="n29315767620c4c949118ed89a344f3a5b28"/>
  </rdf:Description>
  <rdf:Description rdf:nodeID="n87801b7bffed4f059b3dda9335adfc9ab31">
    <sh:path rdf:resource="https://w3id.org/nen2660/def#chemicalFormula"/>
    <sh:datatype rdf:resource="http://www.w3.org/2001/XMLSchema#string"/>
  </rdf:Description>
  <rdf:Description rdf:nodeID="n29315767620c4c949118ed89a344f3a5b57">
    <rdf:first rdf:resource="https://w3id.org/nen2660/def#Interface"/>
    <rdf:rest rdf:resource="http://www.w3.org/1999/02/22-rdf-syntax-ns#nil"/>
  </rdf:Description>
  <rdf:Description rdf:nodeID="n87801b7bffed4f059b3dda9335adfc9ab3">
    <sh:path rdf:resource="https://w3id.org/nen2660/def#hasPart"/>
    <sh:class rdf:resource="https://w3id.org/nen2660/def#Activity"/>
  </rdf:Description>
  <rdf:Description rdf:nodeID="n87801b7bffed4f059b3dda9335adfc9ab9">
    <rdf:first rdf:resource="https://w3id.org/nen2660/def#Plasma"/>
    <rdf:rest rdf:resource="http://www.w3.org/1999/02/22-rdf-syntax-ns#nil"/>
  </rdf:Description>
  <rdf:Description rdf:nodeID="n29315767620c4c949118ed89a344f3a5b3">
    <rdf:first rdf:resource="https://w3id.org/nen2660/def#Liquid"/>
    <rdf:rest rdf:nodeID="n29315767620c4c949118ed89a344f3a5b4"/>
  </rdf:Description>
  <rdf:Description rdf:nodeID="n87801b7bffed4f059b3dda9335adfc9ab90">
    <sh:path rdf:nodeID="n87801b7bffed4f059b3dda9335adfc9ab92"/>
    <sh:qualifiedValueShape rdf:nodeID="n87801b7bffed4f059b3dda9335adfc9ab94"/>
    <sh:qualifiedMaxCount rdf:datatype="http://www.w3.org/2001/XMLSchema#integer">1</sh:qualifiedMaxCount>
  </rdf:Description>
  <rdf:Description rdf:nodeID="n29315767620c4c949118ed89a344f3a5b61">
    <rdf:type rdf:resource="http://www.w3.org/2002/07/owl#Class"/>
    <owl:unionOf rdf:nodeID="n29315767620c4c949118ed89a344f3a5b62"/>
  </rdf:Description>
  <rdf:Description rdf:nodeID="n87801b7bffed4f059b3dda9335adfc9ab88">
    <rdf:first rdf:resource="https://w3id.org/nen2660/def#InformationFlow"/>
    <rdf:rest rdf:nodeID="n87801b7bffed4f059b3dda9335adfc9ab89"/>
  </rdf:Description>
  <rdf:Description rdf:nodeID="n87801b7bffed4f059b3dda9335adfc9ab120">
    <rdf:first rdf:resource="https://w3id.org/nen2660/def#RealizedEntity"/>
    <rdf:rest rdf:resource="http://www.w3.org/1999/02/22-rdf-syntax-ns#nil"/>
  </rdf:Description>
  <rdf:Description rdf:nodeID="n87801b7bffed4f059b3dda9335adfc9ab52">
    <rdf:first rdf:nodeID="n87801b7bffed4f059b3dda9335adfc9ab49"/>
    <rdf:rest rdf:nodeID="n87801b7bffed4f059b3dda9335adfc9ab53"/>
  </rdf:Description>
  <rdf:Description rdf:nodeID="n87801b7bffed4f059b3dda9335adfc9ab101">
    <sh:zeroOrMorePath rdf:resource="http://www.w3.org/2000/01/rdf-schema#subClassOf"/>
  </rdf:Description>
  <rdf:Description rdf:nodeID="n87801b7bffed4f059b3dda9335adfc9ab119">
    <rdf:first rdf:resource="https://w3id.org/nen2660/def#PlannedEntity"/>
    <rdf:rest rdf:nodeID="n87801b7bffed4f059b3dda9335adfc9ab120"/>
  </rdf:Description>
  <rdf:Description rdf:nodeID="n29315767620c4c949118ed89a344f3a5b24">
    <rdf:type rdf:resource="http://www.w3.org/2002/07/owl#Restriction"/>
    <owl:allValuesFrom rdf:nodeID="n29315767620c4c949118ed89a344f3a5b25"/>
    <owl:onProperty rdf:resource="http://www.w3.org/1999/02/22-rdf-syntax-ns#value"/>
  </rdf:Description>
  <rdf:Description rdf:nodeID="n87801b7bffed4f059b3dda9335adfc9ab16">
    <sh:path rdf:resource="https://w3id.org/nen2660/def#connectsPort"/>
    <sh:class rdf:resource="https://w3id.org/nen2660/def#Port"/>
  </rdf:Description>
  <rdf:Description rdf:nodeID="n87801b7bffed4f059b3dda9335adfc9ab1">
    <sh:path rdf:resource="https://w3id.org/nen2660/def#hasBoundary"/>
    <sh:class rdf:resource="https://w3id.org/nen2660/def#GeometricEntity"/>
  </rdf:Description>
  <rdf:Description rdf:nodeID="n87801b7bffed4f059b3dda9335adfc9ab80">
    <sh:path rdf:resource="https://w3id.org/nen2660/def#hasPeriod"/>
    <sh:class rdf:resource="http://www.w3.org/2006/time#TemporalEntity"/>
  </rdf:Description>
  <rdf:Description rdf:nodeID="n29315767620c4c949118ed89a344f3a5b7">
    <rdf:first rdf:resource="https://w3id.org/nen2660/def#InformationObject"/>
    <rdf:rest rdf:nodeID="n29315767620c4c949118ed89a344f3a5b8"/>
  </rdf:Description>
  <rdf:Description rdf:nodeID="n87801b7bffed4f059b3dda9335adfc9ab105">
    <rdf:first rdf:resource="https://w3id.org/nen2660/def#RealObject"/>
    <rdf:rest rdf:nodeID="n87801b7bffed4f059b3dda9335adfc9ab106"/>
  </rdf:Description>
  <rdf:Description rdf:nodeID="n87801b7bffed4f059b3dda9335adfc9ab65">
    <sh:path rdf:resource="http://www.w3.org/1999/02/22-rdf-syntax-ns#value"/>
    <sh:datatype rdf:resource="http://www.w3.org/2001/XMLSchema#anyURI"/>
  </rdf:Description>
  <rdf:Description rdf:nodeID="n87801b7bffed4f059b3dda9335adfc9ab33">
    <sh:path rdf:resource="https://w3id.org/nen2660/def#consistsOf"/>
    <sh:or rdf:nodeID="n87801b7bffed4f059b3dda9335adfc9ab36"/>
  </rdf:Description>
  <rdf:Description rdf:nodeID="n87801b7bffed4f059b3dda9335adfc9ab78">
    <sh:path rdf:resource="https://w3id.org/nen2660/def#hasInterior"/>
    <sh:class rdf:resource="https://w3id.org/nen2660/def#GeometricEntity"/>
  </rdf:Description>
  <rdf:Description rdf:nodeID="n29315767620c4c949118ed89a344f3a5b53">
    <rdf:first rdf:resource="https://w3id.org/nen2660/def#Connection"/>
    <rdf:rest rdf:nodeID="n29315767620c4c949118ed89a344f3a5b54"/>
  </rdf:Description>
  <rdf:Description rdf:nodeID="n87801b7bffed4f059b3dda9335adfc9ab96">
    <rdf:first rdf:resource="https://w3id.org/nen2660/def#InformationObject"/>
    <rdf:rest rdf:nodeID="n87801b7bffed4f059b3dda9335adfc9ab97"/>
  </rdf:Description>
  <rdf:Description rdf:about="https://w3id.org/nen2660/def#AllDisjointClasses_1">
    <rdf:type rdf:resource="http://www.w3.org/2002/07/owl#AllDisjointClasses"/>
    <owl:members rdf:nodeID="n29315767620c4c949118ed89a344f3a5b6"/>
  </rdf:Description>
  <rdf:Description rdf:nodeID="n87801b7bffed4f059b3dda9335adfc9ab19">
    <sh:path rdf:resource="https://w3id.org/nen2660/def#begins"/>
    <sh:class rdf:resource="https://w3id.org/nen2660/def#State"/>
  </rdf:Description>
  <rdf:Description rdf:nodeID="n29315767620c4c949118ed89a344f3a5b10">
    <rdf:first rdf:resource="https://w3id.org/nen2660/def#State"/>
    <rdf:rest rdf:resource="http://www.w3.org/1999/02/22-rdf-syntax-ns#nil"/>
  </rdf:Description>
  <rdf:Description rdf:nodeID="n87801b7bffed4f059b3dda9335adfc9ab62">
    <rdf:first rdf:nodeID="n87801b7bffed4f059b3dda9335adfc9ab60"/>
    <rdf:rest rdf:nodeID="n87801b7bffed4f059b3dda9335adfc9ab63"/>
  </rdf:Description>
  <rdf:Description rdf:nodeID="n29315767620c4c949118ed89a344f3a5b9">
    <rdf:first rdf:resource="https://w3id.org/nen2660/def#Event"/>
    <rdf:rest rdf:nodeID="n29315767620c4c949118ed89a344f3a5b10"/>
  </rdf:Description>
  <rdf:Description rdf:nodeID="n29315767620c4c949118ed89a344f3a5b48">
    <rdf:first rdf:resource="https://w3id.org/nen2660/def#MaterialFlow"/>
    <rdf:rest rdf:nodeID="n29315767620c4c949118ed89a344f3a5b49"/>
  </rdf:Description>
  <rdf:Description rdf:nodeID="n29315767620c4c949118ed89a344f3a5b8">
    <rdf:first rdf:resource="https://w3id.org/nen2660/def#Activity"/>
    <rdf:rest rdf:nodeID="n29315767620c4c949118ed89a344f3a5b9"/>
  </rdf:Description>
  <rdf:Description rdf:nodeID="n29315767620c4c949118ed89a344f3a5b58">
    <rdf:type rdf:resource="http://www.w3.org/2002/07/owl#Class"/>
    <owl:unionOf rdf:nodeID="n29315767620c4c949118ed89a344f3a5b59"/>
  </rdf:Description>
  <rdf:Description rdf:nodeID="n87801b7bffed4f059b3dda9335adfc9ab4">
    <sh:path rdf:resource="https://w3id.org/nen2660/def#hasPeriod"/>
    <sh:class rdf:resource="http://www.w3.org/2006/time#TemporalEntity"/>
  </rdf:Description>
  <rdf:Description rdf:nodeID="n87801b7bffed4f059b3dda9335adfc9ab11">
    <sh:path rdf:resource="https://w3id.org/nen2660/def#hasInterior"/>
    <sh:class rdf:resource="https://w3id.org/nen2660/def#GeometricEntity"/>
  </rdf:Description>
  <rdf:Description rdf:nodeID="n87801b7bffed4f059b3dda9335adfc9ab111">
    <sh:in rdf:nodeID="n87801b7bffed4f059b3dda9335adfc9ab112"/>
  </rdf:Description>
  <rdf:Description rdf:nodeID="n87801b7bffed4f059b3dda9335adfc9ab59">
    <sh:path rdf:resource="https://w3id.org/nen2660/def#hasPart"/>
    <sh:or rdf:nodeID="n87801b7bffed4f059b3dda9335adfc9ab62"/>
  </rdf:Description>
  <rdf:Description rdf:nodeID="n87801b7bffed4f059b3dda9335adfc9ab85">
    <sh:path rdf:resource="https://w3id.org/nen2660/def#isDescribedBy"/>
    <sh:class rdf:resource="https://w3id.org/nen2660/def#InformationObject"/>
  </rdf:Description>
  <rdf:Description rdf:about="https://w3id.org/nen2660/def#AllDisjointClasses_4">
    <rdf:type rdf:resource="http://www.w3.org/2002/07/owl#AllDisjointClasses"/>
    <owl:members rdf:nodeID="n29315767620c4c949118ed89a344f3a5b15"/>
  </rdf:Description>
  <rdf:Description rdf:nodeID="n87801b7bffed4f059b3dda9335adfc9ab118">
    <sh:in rdf:nodeID="n87801b7bffed4f059b3dda9335adfc9ab119"/>
  </rdf:Description>
  <rdf:Description rdf:nodeID="n87801b7bffed4f059b3dda9335adfc9ab35">
    <sh:class rdf:resource="https://w3id.org/nen2660/def#MatterPortion"/>
  </rdf:Description>
  <rdf:Description rdf:nodeID="n87801b7bffed4f059b3dda9335adfc9ab48">
    <sh:datatype rdf:resource="http://www.w3.org/2001/XMLSchema#decimal"/>
  </rdf:Description>
  <rdf:Description rdf:nodeID="n87801b7bffed4f059b3dda9335adfc9ab49">
    <sh:datatype rdf:resource="http://www.w3.org/2001/XMLSchema#float"/>
  </rdf:Description>
  <rdf:Description rdf:nodeID="n87801b7bffed4f059b3dda9335adfc9ab76">
    <sh:path rdf:resource="https://w3id.org/nen2660/def#isBoundBy"/>
    <sh:class rdf:resource="https://w3id.org/nen2660/def#PhysicalObject"/>
  </rdf:Description>
  <rdf:Description rdf:nodeID="n87801b7bffed4f059b3dda9335adfc9ab115">
    <sh:zeroOrMorePath rdf:resource="http://www.w3.org/2000/01/rdf-schema#subClassOf"/>
  </rdf:Description>
  <rdf:Description rdf:nodeID="n87801b7bffed4f059b3dda9335adfc9ab42">
    <sh:path rdf:resource="https://w3id.org/nen2660/def#participatesIn"/>
    <sh:class rdf:resource="https://w3id.org/nen2660/def#Interaction"/>
  </rdf:Description>
  <rdf:Description rdf:nodeID="n87801b7bffed4f059b3dda9335adfc9ab56">
    <sh:class rdf:resource="https://w3id.org/nen2660/def#MatterPortion"/>
  </rdf:Description>
  <rdf:Description rdf:nodeID="n87801b7bffed4f059b3dda9335adfc9ab73">
    <sh:class rdf:resource="https://w3id.org/nen2660/def#Port"/>
  </rdf:Description>
  <rdf:Description rdf:nodeID="n87801b7bffed4f059b3dda9335adfc9ab55">
    <sh:class rdf:resource="https://w3id.org/nen2660/def#Matter"/>
  </rdf:Description>
</rdf:RDF>
